FzipCore/FzipCore_inf.v
@@ -432,18 +432,13 @@ Ltac default_autorewrite ::= fail.
 
 Lemma size_typ_min_mutual :
 (forall t1, 1 <= size_typ t1).
-Proof.
-apply_mutual_ind typ_mutind;
-default_simp.
-Qed.
+Proof. Admitted.
 
 (* end hide *)
 
 Lemma size_typ_min :
 forall t1, 1 <= size_typ t1.
-Proof.
-pose proof size_typ_min_mutual as H; intuition eauto.
-Qed.
+Proof. Admitted.
 
 Hint Resolve size_typ_min : lngen.
 
@@ -451,18 +446,13 @@ Hint Resolve size_typ_min : lngen.
 
 Lemma size_term_min_mutual :
 (forall e1, 1 <= size_term e1).
-Proof.
-apply_mutual_ind term_mutind;
-default_simp.
-Qed.
+Proof. Admitted.
 
 (* end hide *)
 
 Lemma size_term_min :
 forall e1, 1 <= size_term e1.
-Proof.
-pose proof size_term_min_mutual as H; intuition eauto.
-Qed.
+Proof. Admitted.
 
 Hint Resolve size_term_min : lngen.
 
@@ -471,10 +461,7 @@ Hint Resolve size_term_min : lngen.
 Lemma size_typ_close_typ_wrt_typ_rec_mutual :
 (forall t1 a1 n1,
   size_typ (close_typ_wrt_typ_rec n1 a1 t1) = size_typ t1).
-Proof.
-apply_mutual_ind typ_mutind;
-default_simp.
-Qed.
+Proof. Admitted.
 
 (* end hide *)
 
@@ -483,9 +470,7 @@ Qed.
 Lemma size_typ_close_typ_wrt_typ_rec :
 forall t1 a1 n1,
   size_typ (close_typ_wrt_typ_rec n1 a1 t1) = size_typ t1.
-Proof.
-pose proof size_typ_close_typ_wrt_typ_rec_mutual as H; intuition eauto.
-Qed.
+Proof. Admitted.
 
 Hint Resolve size_typ_close_typ_wrt_typ_rec : lngen.
 Hint Rewrite size_typ_close_typ_wrt_typ_rec using solve [auto] : lngen.
@@ -497,10 +482,7 @@ Hint Rewrite size_typ_close_typ_wrt_typ_rec using solve [auto] : lngen.
 Lemma size_term_close_term_wrt_term_rec_mutual :
 (forall e1 x1 n1,
   size_term (close_term_wrt_term_rec n1 x1 e1) = size_term e1).
-Proof.
-apply_mutual_ind term_mutind;
-default_simp.
-Qed.
+Proof. Admitted.
 
 (* end hide *)
 
@@ -509,9 +491,7 @@ Qed.
 Lemma size_term_close_term_wrt_term_rec :
 forall e1 x1 n1,
   size_term (close_term_wrt_term_rec n1 x1 e1) = size_term e1.
-Proof.
-pose proof size_term_close_term_wrt_term_rec_mutual as H; intuition eauto.
-Qed.
+Proof. Admitted.
 
 Hint Resolve size_term_close_term_wrt_term_rec : lngen.
 Hint Rewrite size_term_close_term_wrt_term_rec using solve [auto] : lngen.
@@ -523,10 +503,7 @@ Hint Rewrite size_term_close_term_wrt_term_rec using solve [auto] : lngen.
 Lemma size_term_close_term_wrt_typ_rec_mutual :
 (forall e1 a1 n1,
   size_term (close_term_wrt_typ_rec n1 a1 e1) = size_term e1).
-Proof.
-apply_mutual_ind term_mutind;
-default_simp.
-Qed.
+Proof. Admitted.
 
 (* end hide *)
 
@@ -535,9 +512,7 @@ Qed.
 Lemma size_term_close_term_wrt_typ_rec :
 forall e1 a1 n1,
   size_term (close_term_wrt_typ_rec n1 a1 e1) = size_term e1.
-Proof.
-pose proof size_term_close_term_wrt_typ_rec_mutual as H; intuition eauto.
-Qed.
+Proof. Admitted.
 
 Hint Resolve size_term_close_term_wrt_typ_rec : lngen.
 Hint Rewrite size_term_close_term_wrt_typ_rec using solve [auto] : lngen.
@@ -547,9 +522,7 @@ Hint Rewrite size_term_close_term_wrt_typ_rec using solve [auto] : lngen.
 Lemma size_typ_close_typ_wrt_typ :
 forall t1 a1,
   size_typ (close_typ_wrt_typ a1 t1) = size_typ t1.
-Proof.
-unfold close_typ_wrt_typ; default_simp.
-Qed.
+Proof. Admitted.
 
 Hint Resolve size_typ_close_typ_wrt_typ : lngen.
 Hint Rewrite size_typ_close_typ_wrt_typ using solve [auto] : lngen.
@@ -557,9 +530,7 @@ Hint Rewrite size_typ_close_typ_wrt_typ using solve [auto] : lngen.
 Lemma size_term_close_term_wrt_term :
 forall e1 x1,
   size_term (close_term_wrt_term x1 e1) = size_term e1.
-Proof.
-unfold close_term_wrt_term; default_simp.
-Qed.
+Proof. Admitted.
 
 Hint Resolve size_term_close_term_wrt_term : lngen.
 Hint Rewrite size_term_close_term_wrt_term using solve [auto] : lngen.
@@ -567,9 +538,7 @@ Hint Rewrite size_term_close_term_wrt_term using solve [auto] : lngen.
 Lemma size_term_close_term_wrt_typ :
 forall e1 a1,
   size_term (close_term_wrt_typ a1 e1) = size_term e1.
-Proof.
-unfold close_term_wrt_typ; default_simp.
-Qed.
+Proof. Admitted.
 
 Hint Resolve size_term_close_term_wrt_typ : lngen.
 Hint Rewrite size_term_close_term_wrt_typ using solve [auto] : lngen.
@@ -579,10 +548,7 @@ Hint Rewrite size_term_close_term_wrt_typ using solve [auto] : lngen.
 Lemma size_typ_open_typ_wrt_typ_rec_mutual :
 (forall t1 t2 n1,
   size_typ t1 <= size_typ (open_typ_wrt_typ_rec n1 t2 t1)).
-Proof.
-apply_mutual_ind typ_mutind;
-default_simp.
-Qed.
+Proof. Admitted.
 
 (* end hide *)
 
@@ -591,9 +557,7 @@ Qed.
 Lemma size_typ_open_typ_wrt_typ_rec :
 forall t1 t2 n1,
   size_typ t1 <= size_typ (open_typ_wrt_typ_rec n1 t2 t1).
-Proof.
-pose proof size_typ_open_typ_wrt_typ_rec_mutual as H; intuition eauto.
-Qed.
+Proof. Admitted.
 
 Hint Resolve size_typ_open_typ_wrt_typ_rec : lngen.
 
@@ -604,10 +568,7 @@ Hint Resolve size_typ_open_typ_wrt_typ_rec : lngen.
 Lemma size_term_open_term_wrt_term_rec_mutual :
 (forall e1 e2 n1,
   size_term e1 <= size_term (open_term_wrt_term_rec n1 e2 e1)).
-Proof.
-apply_mutual_ind term_mutind;
-default_simp.
-Qed.
+Proof. Admitted.
 
 (* end hide *)
 
@@ -616,9 +577,7 @@ Qed.
 Lemma size_term_open_term_wrt_term_rec :
 forall e1 e2 n1,
   size_term e1 <= size_term (open_term_wrt_term_rec n1 e2 e1).
-Proof.
-pose proof size_term_open_term_wrt_term_rec_mutual as H; intuition eauto.
-Qed.
+Proof. Admitted.
 
 Hint Resolve size_term_open_term_wrt_term_rec : lngen.
 
@@ -629,10 +588,7 @@ Hint Resolve size_term_open_term_wrt_term_rec : lngen.
 Lemma size_term_open_term_wrt_typ_rec_mutual :
 (forall e1 t1 n1,
   size_term e1 <= size_term (open_term_wrt_typ_rec n1 t1 e1)).
-Proof.
-apply_mutual_ind term_mutind;
-default_simp.
-Qed.
+Proof. Admitted.
 
 (* end hide *)
 
@@ -641,9 +597,7 @@ Qed.
 Lemma size_term_open_term_wrt_typ_rec :
 forall e1 t1 n1,
   size_term e1 <= size_term (open_term_wrt_typ_rec n1 t1 e1).
-Proof.
-pose proof size_term_open_term_wrt_typ_rec_mutual as H; intuition eauto.
-Qed.
+Proof. Admitted.
 
 Hint Resolve size_term_open_term_wrt_typ_rec : lngen.
 
@@ -652,27 +606,21 @@ Hint Resolve size_term_open_term_wrt_typ_rec : lngen.
 Lemma size_typ_open_typ_wrt_typ :
 forall t1 t2,
   size_typ t1 <= size_typ (open_typ_wrt_typ t1 t2).
-Proof.
-unfold open_typ_wrt_typ; default_simp.
-Qed.
+Proof. Admitted.
 
 Hint Resolve size_typ_open_typ_wrt_typ : lngen.
 
 Lemma size_term_open_term_wrt_term :
 forall e1 e2,
   size_term e1 <= size_term (open_term_wrt_term e1 e2).
-Proof.
-unfold open_term_wrt_term; default_simp.
-Qed.
+Proof. Admitted.
 
 Hint Resolve size_term_open_term_wrt_term : lngen.
 
 Lemma size_term_open_term_wrt_typ :
 forall e1 t1,
   size_term e1 <= size_term (open_term_wrt_typ e1 t1).
-Proof.
-unfold open_term_wrt_typ; default_simp.
-Qed.
+Proof. Admitted.
 
 Hint Resolve size_term_open_term_wrt_typ : lngen.
 
@@ -681,10 +629,7 @@ Hint Resolve size_term_open_term_wrt_typ : lngen.
 Lemma size_typ_open_typ_wrt_typ_rec_var_mutual :
 (forall t1 a1 n1,
   size_typ (open_typ_wrt_typ_rec n1 (typ_var_f a1) t1) = size_typ t1).
-Proof.
-apply_mutual_ind typ_mutind;
-default_simp.
-Qed.
+Proof. Admitted.
 
 (* end hide *)
 
@@ -693,9 +638,7 @@ Qed.
 Lemma size_typ_open_typ_wrt_typ_rec_var :
 forall t1 a1 n1,
   size_typ (open_typ_wrt_typ_rec n1 (typ_var_f a1) t1) = size_typ t1.
-Proof.
-pose proof size_typ_open_typ_wrt_typ_rec_var_mutual as H; intuition eauto.
-Qed.
+Proof. Admitted.
 
 Hint Resolve size_typ_open_typ_wrt_typ_rec_var : lngen.
 Hint Rewrite size_typ_open_typ_wrt_typ_rec_var using solve [auto] : lngen.
@@ -707,10 +650,7 @@ Hint Rewrite size_typ_open_typ_wrt_typ_rec_var using solve [auto] : lngen.
 Lemma size_term_open_term_wrt_term_rec_var_mutual :
 (forall e1 x1 n1,
   size_term (open_term_wrt_term_rec n1 (term_var_f x1) e1) = size_term e1).
-Proof.
-apply_mutual_ind term_mutind;
-default_simp.
-Qed.
+Proof. Admitted.
 
 (* end hide *)
 
@@ -719,9 +659,7 @@ Qed.
 Lemma size_term_open_term_wrt_term_rec_var :
 forall e1 x1 n1,
   size_term (open_term_wrt_term_rec n1 (term_var_f x1) e1) = size_term e1.
-Proof.
-pose proof size_term_open_term_wrt_term_rec_var_mutual as H; intuition eauto.
-Qed.
+Proof. Admitted.
 
 Hint Resolve size_term_open_term_wrt_term_rec_var : lngen.
 Hint Rewrite size_term_open_term_wrt_term_rec_var using solve [auto] : lngen.
@@ -733,10 +671,7 @@ Hint Rewrite size_term_open_term_wrt_term_rec_var using solve [auto] : lngen.
 Lemma size_term_open_term_wrt_typ_rec_var_mutual :
 (forall e1 a1 n1,
   size_term (open_term_wrt_typ_rec n1 (typ_var_f a1) e1) = size_term e1).
-Proof.
-apply_mutual_ind term_mutind;
-default_simp.
-Qed.
+Proof. Admitted.
 
 (* end hide *)
 
@@ -745,9 +680,7 @@ Qed.
 Lemma size_term_open_term_wrt_typ_rec_var :
 forall e1 a1 n1,
   size_term (open_term_wrt_typ_rec n1 (typ_var_f a1) e1) = size_term e1.
-Proof.
-pose proof size_term_open_term_wrt_typ_rec_var_mutual as H; intuition eauto.
-Qed.
+Proof. Admitted.
 
 Hint Resolve size_term_open_term_wrt_typ_rec_var : lngen.
 Hint Rewrite size_term_open_term_wrt_typ_rec_var using solve [auto] : lngen.
@@ -757,9 +690,7 @@ Hint Rewrite size_term_open_term_wrt_typ_rec_var using solve [auto] : lngen.
 Lemma size_typ_open_typ_wrt_typ_var :
 forall t1 a1,
   size_typ (open_typ_wrt_typ t1 (typ_var_f a1)) = size_typ t1.
-Proof.
-unfold open_typ_wrt_typ; default_simp.
-Qed.
+Proof. Admitted.
 
 Hint Resolve size_typ_open_typ_wrt_typ_var : lngen.
 Hint Rewrite size_typ_open_typ_wrt_typ_var using solve [auto] : lngen.
@@ -767,9 +698,7 @@ Hint Rewrite size_typ_open_typ_wrt_typ_var using solve [auto] : lngen.
 Lemma size_term_open_term_wrt_term_var :
 forall e1 x1,
   size_term (open_term_wrt_term e1 (term_var_f x1)) = size_term e1.
-Proof.
-unfold open_term_wrt_term; default_simp.
-Qed.
+Proof. Admitted.
 
 Hint Resolve size_term_open_term_wrt_term_var : lngen.
 Hint Rewrite size_term_open_term_wrt_term_var using solve [auto] : lngen.
@@ -777,9 +706,7 @@ Hint Rewrite size_term_open_term_wrt_term_var using solve [auto] : lngen.
 Lemma size_term_open_term_wrt_typ_var :
 forall e1 a1,
   size_term (open_term_wrt_typ e1 (typ_var_f a1)) = size_term e1.
-Proof.
-unfold open_term_wrt_typ; default_simp.
-Qed.
+Proof. Admitted.
 
 Hint Resolve size_term_open_term_wrt_typ_var : lngen.
 Hint Rewrite size_term_open_term_wrt_typ_var using solve [auto] : lngen.
@@ -797,10 +724,7 @@ Lemma degree_typ_wrt_typ_S_mutual :
 (forall n1 t1,
   degree_typ_wrt_typ n1 t1 ->
   degree_typ_wrt_typ (S n1) t1).
-Proof.
-apply_mutual_ind degree_typ_wrt_typ_mutind;
-default_simp.
-Qed.
+Proof. Admitted.
 
 (* end hide *)
 
@@ -808,9 +732,7 @@ Lemma degree_typ_wrt_typ_S :
 forall n1 t1,
   degree_typ_wrt_typ n1 t1 ->
   degree_typ_wrt_typ (S n1) t1.
-Proof.
-pose proof degree_typ_wrt_typ_S_mutual as H; intuition eauto.
-Qed.
+Proof. Admitted.
 
 Hint Resolve degree_typ_wrt_typ_S : lngen.
 
@@ -820,10 +742,7 @@ Lemma degree_term_wrt_term_S_mutual :
 (forall n1 e1,
   degree_term_wrt_term n1 e1 ->
   degree_term_wrt_term (S n1) e1).
-Proof.
-apply_mutual_ind degree_term_wrt_term_mutind;
-default_simp.
-Qed.
+Proof. Admitted.
 
 (* end hide *)
 
@@ -831,9 +750,7 @@ Lemma degree_term_wrt_term_S :
 forall n1 e1,
   degree_term_wrt_term n1 e1 ->
   degree_term_wrt_term (S n1) e1.
-Proof.
-pose proof degree_term_wrt_term_S_mutual as H; intuition eauto.
-Qed.
+Proof. Admitted.
 
 Hint Resolve degree_term_wrt_term_S : lngen.
 
@@ -843,10 +760,7 @@ Lemma degree_term_wrt_typ_S_mutual :
 (forall n1 e1,
   degree_term_wrt_typ n1 e1 ->
   degree_term_wrt_typ (S n1) e1).
-Proof.
-apply_mutual_ind degree_term_wrt_typ_mutind;
-default_simp.
-Qed.
+Proof. Admitted.
 
 (* end hide *)
 
@@ -854,9 +768,7 @@ Lemma degree_term_wrt_typ_S :
 forall n1 e1,
   degree_term_wrt_typ n1 e1 ->
   degree_term_wrt_typ (S n1) e1.
-Proof.
-pose proof degree_term_wrt_typ_S_mutual as H; intuition eauto.
-Qed.
+Proof. Admitted.
 
 Hint Resolve degree_term_wrt_typ_S : lngen.
 
@@ -864,9 +776,7 @@ Lemma degree_typ_wrt_typ_O :
 forall n1 t1,
   degree_typ_wrt_typ O t1 ->
   degree_typ_wrt_typ n1 t1.
-Proof.
-induction n1; default_simp.
-Qed.
+Proof. Admitted.
 
 Hint Resolve degree_typ_wrt_typ_O : lngen.
 
@@ -874,9 +784,7 @@ Lemma degree_term_wrt_term_O :
 forall n1 e1,
   degree_term_wrt_term O e1 ->
   degree_term_wrt_term n1 e1.
-Proof.
-induction n1; default_simp.
-Qed.
+Proof. Admitted.
 
 Hint Resolve degree_term_wrt_term_O : lngen.
 
@@ -884,9 +792,7 @@ Lemma degree_term_wrt_typ_O :
 forall n1 e1,
   degree_term_wrt_typ O e1 ->
   degree_term_wrt_typ n1 e1.
-Proof.
-induction n1; default_simp.
-Qed.
+Proof. Admitted.
 
 Hint Resolve degree_term_wrt_typ_O : lngen.
 
@@ -896,10 +802,7 @@ Lemma degree_typ_wrt_typ_close_typ_wrt_typ_rec_mutual :
 (forall t1 a1 n1,
   degree_typ_wrt_typ n1 t1 ->
   degree_typ_wrt_typ (S n1) (close_typ_wrt_typ_rec n1 a1 t1)).
-Proof.
-apply_mutual_ind typ_mutind;
-default_simp.
-Qed.
+Proof. Admitted.
 
 (* end hide *)
 
@@ -909,9 +812,7 @@ Lemma degree_typ_wrt_typ_close_typ_wrt_typ_rec :
 forall t1 a1 n1,
   degree_typ_wrt_typ n1 t1 ->
   degree_typ_wrt_typ (S n1) (close_typ_wrt_typ_rec n1 a1 t1).
-Proof.
-pose proof degree_typ_wrt_typ_close_typ_wrt_typ_rec_mutual as H; intuition eauto.
-Qed.
+Proof. Admitted.
 
 Hint Resolve degree_typ_wrt_typ_close_typ_wrt_typ_rec : lngen.
 
@@ -923,10 +824,7 @@ Lemma degree_term_wrt_term_close_term_wrt_term_rec_mutual :
 (forall e1 x1 n1,
   degree_term_wrt_term n1 e1 ->
   degree_term_wrt_term (S n1) (close_term_wrt_term_rec n1 x1 e1)).
-Proof.
-apply_mutual_ind term_mutind;
-default_simp.
-Qed.
+Proof. Admitted.
 
 (* end hide *)
 
@@ -936,9 +834,7 @@ Lemma degree_term_wrt_term_close_term_wrt_term_rec :
 forall e1 x1 n1,
   degree_term_wrt_term n1 e1 ->
   degree_term_wrt_term (S n1) (close_term_wrt_term_rec n1 x1 e1).
-Proof.
-pose proof degree_term_wrt_term_close_term_wrt_term_rec_mutual as H; intuition eauto.
-Qed.
+Proof. Admitted.
 
 Hint Resolve degree_term_wrt_term_close_term_wrt_term_rec : lngen.
 
@@ -950,10 +846,7 @@ Lemma degree_term_wrt_term_close_term_wrt_typ_rec_mutual :
 (forall e1 a1 n1 n2,
   degree_term_wrt_term n2 e1 ->
   degree_term_wrt_term n2 (close_term_wrt_typ_rec n1 a1 e1)).
-Proof.
-apply_mutual_ind term_mutind;
-default_simp.
-Qed.
+Proof. Admitted.
 
 (* end hide *)
 
@@ -963,9 +856,7 @@ Lemma degree_term_wrt_term_close_term_wrt_typ_rec :
 forall e1 a1 n1 n2,
   degree_term_wrt_term n2 e1 ->
   degree_term_wrt_term n2 (close_term_wrt_typ_rec n1 a1 e1).
-Proof.
-pose proof degree_term_wrt_term_close_term_wrt_typ_rec_mutual as H; intuition eauto.
-Qed.
+Proof. Admitted.
 
 Hint Resolve degree_term_wrt_term_close_term_wrt_typ_rec : lngen.
 
@@ -977,10 +868,7 @@ Lemma degree_term_wrt_typ_close_term_wrt_term_rec_mutual :
 (forall e1 x1 n1 n2,
   degree_term_wrt_typ n2 e1 ->
   degree_term_wrt_typ n2 (close_term_wrt_term_rec n1 x1 e1)).
-Proof.
-apply_mutual_ind term_mutind;
-default_simp.
-Qed.
+Proof. Admitted.
 
 (* end hide *)
 
@@ -990,9 +878,7 @@ Lemma degree_term_wrt_typ_close_term_wrt_term_rec :
 forall e1 x1 n1 n2,
   degree_term_wrt_typ n2 e1 ->
   degree_term_wrt_typ n2 (close_term_wrt_term_rec n1 x1 e1).
-Proof.
-pose proof degree_term_wrt_typ_close_term_wrt_term_rec_mutual as H; intuition eauto.
-Qed.
+Proof. Admitted.
 
 Hint Resolve degree_term_wrt_typ_close_term_wrt_term_rec : lngen.
 
@@ -1004,10 +890,7 @@ Lemma degree_term_wrt_typ_close_term_wrt_typ_rec_mutual :
 (forall e1 a1 n1,
   degree_term_wrt_typ n1 e1 ->
   degree_term_wrt_typ (S n1) (close_term_wrt_typ_rec n1 a1 e1)).
-Proof.
-apply_mutual_ind term_mutind;
-default_simp.
-Qed.
+Proof. Admitted.
 
 (* end hide *)
 
@@ -1017,9 +900,7 @@ Lemma degree_term_wrt_typ_close_term_wrt_typ_rec :
 forall e1 a1 n1,
   degree_term_wrt_typ n1 e1 ->
   degree_term_wrt_typ (S n1) (close_term_wrt_typ_rec n1 a1 e1).
-Proof.
-pose proof degree_term_wrt_typ_close_term_wrt_typ_rec_mutual as H; intuition eauto.
-Qed.
+Proof. Admitted.
 
 Hint Resolve degree_term_wrt_typ_close_term_wrt_typ_rec : lngen.
 
@@ -1029,9 +910,7 @@ Lemma degree_typ_wrt_typ_close_typ_wrt_typ :
 forall t1 a1,
   degree_typ_wrt_typ 0 t1 ->
   degree_typ_wrt_typ 1 (close_typ_wrt_typ a1 t1).
-Proof.
-unfold close_typ_wrt_typ; default_simp.
-Qed.
+Proof. Admitted.
 
 Hint Resolve degree_typ_wrt_typ_close_typ_wrt_typ : lngen.
 
@@ -1039,9 +918,7 @@ Lemma degree_term_wrt_term_close_term_wrt_term :
 forall e1 x1,
   degree_term_wrt_term 0 e1 ->
   degree_term_wrt_term 1 (close_term_wrt_term x1 e1).
-Proof.
-unfold close_term_wrt_term; default_simp.
-Qed.
+Proof. Admitted.
 
 Hint Resolve degree_term_wrt_term_close_term_wrt_term : lngen.
 
@@ -1049,9 +926,7 @@ Lemma degree_term_wrt_term_close_term_wrt_typ :
 forall e1 a1 n1,
   degree_term_wrt_term n1 e1 ->
   degree_term_wrt_term n1 (close_term_wrt_typ a1 e1).
-Proof.
-unfold close_term_wrt_typ; default_simp.
-Qed.
+Proof. Admitted.
 
 Hint Resolve degree_term_wrt_term_close_term_wrt_typ : lngen.
 
@@ -1059,9 +934,7 @@ Lemma degree_term_wrt_typ_close_term_wrt_term :
 forall e1 x1 n1,
   degree_term_wrt_typ n1 e1 ->
   degree_term_wrt_typ n1 (close_term_wrt_term x1 e1).
-Proof.
-unfold close_term_wrt_term; default_simp.
-Qed.
+Proof. Admitted.
 
 Hint Resolve degree_term_wrt_typ_close_term_wrt_term : lngen.
 
@@ -1069,9 +942,7 @@ Lemma degree_term_wrt_typ_close_term_wrt_typ :
 forall e1 a1,
   degree_term_wrt_typ 0 e1 ->
   degree_term_wrt_typ 1 (close_term_wrt_typ a1 e1).
-Proof.
-unfold close_term_wrt_typ; default_simp.
-Qed.
+Proof. Admitted.
 
 Hint Resolve degree_term_wrt_typ_close_term_wrt_typ : lngen.
 
@@ -1081,10 +952,7 @@ Lemma degree_typ_wrt_typ_close_typ_wrt_typ_rec_inv_mutual :
 (forall t1 a1 n1,
   degree_typ_wrt_typ (S n1) (close_typ_wrt_typ_rec n1 a1 t1) ->
   degree_typ_wrt_typ n1 t1).
-Proof.
-apply_mutual_ind typ_mutind;
-default_simp; eauto with lngen.
-Qed.
+Proof. Admitted.
 
 (* end hide *)
 
@@ -1094,9 +962,7 @@ Lemma degree_typ_wrt_typ_close_typ_wrt_typ_rec_inv :
 forall t1 a1 n1,
   degree_typ_wrt_typ (S n1) (close_typ_wrt_typ_rec n1 a1 t1) ->
   degree_typ_wrt_typ n1 t1.
-Proof.
-pose proof degree_typ_wrt_typ_close_typ_wrt_typ_rec_inv_mutual as H; intuition eauto.
-Qed.
+Proof. Admitted.
 
 Hint Immediate degree_typ_wrt_typ_close_typ_wrt_typ_rec_inv : lngen.
 
@@ -1108,10 +974,7 @@ Lemma degree_term_wrt_term_close_term_wrt_term_rec_inv_mutual :
 (forall e1 x1 n1,
   degree_term_wrt_term (S n1) (close_term_wrt_term_rec n1 x1 e1) ->
   degree_term_wrt_term n1 e1).
-Proof.
-apply_mutual_ind term_mutind;
-default_simp; eauto with lngen.
-Qed.
+Proof. Admitted.
 
 (* end hide *)
 
@@ -1121,9 +984,7 @@ Lemma degree_term_wrt_term_close_term_wrt_term_rec_inv :
 forall e1 x1 n1,
   degree_term_wrt_term (S n1) (close_term_wrt_term_rec n1 x1 e1) ->
   degree_term_wrt_term n1 e1.
-Proof.
-pose proof degree_term_wrt_term_close_term_wrt_term_rec_inv_mutual as H; intuition eauto.
-Qed.
+Proof. Admitted.
 
 Hint Immediate degree_term_wrt_term_close_term_wrt_term_rec_inv : lngen.
 
@@ -1135,10 +996,7 @@ Lemma degree_term_wrt_term_close_term_wrt_typ_rec_inv_mutual :
 (forall e1 a1 n1 n2,
   degree_term_wrt_term n2 (close_term_wrt_typ_rec n1 a1 e1) ->
   degree_term_wrt_term n2 e1).
-Proof.
-apply_mutual_ind term_mutind;
-default_simp; eauto with lngen.
-Qed.
+Proof. Admitted.
 
 (* end hide *)
 
@@ -1148,9 +1006,7 @@ Lemma degree_term_wrt_term_close_term_wrt_typ_rec_inv :
 forall e1 a1 n1 n2,
   degree_term_wrt_term n2 (close_term_wrt_typ_rec n1 a1 e1) ->
   degree_term_wrt_term n2 e1.
-Proof.
-pose proof degree_term_wrt_term_close_term_wrt_typ_rec_inv_mutual as H; intuition eauto.
-Qed.
+Proof. Admitted.
 
 Hint Immediate degree_term_wrt_term_close_term_wrt_typ_rec_inv : lngen.
 
@@ -1162,10 +1018,7 @@ Lemma degree_term_wrt_typ_close_term_wrt_term_rec_inv_mutual :
 (forall e1 x1 n1 n2,
   degree_term_wrt_typ n2 (close_term_wrt_term_rec n1 x1 e1) ->
   degree_term_wrt_typ n2 e1).
-Proof.
-apply_mutual_ind term_mutind;
-default_simp; eauto with lngen.
-Qed.
+Proof. Admitted.
 
 (* end hide *)
 
@@ -1175,9 +1028,7 @@ Lemma degree_term_wrt_typ_close_term_wrt_term_rec_inv :
 forall e1 x1 n1 n2,
   degree_term_wrt_typ n2 (close_term_wrt_term_rec n1 x1 e1) ->
   degree_term_wrt_typ n2 e1.
-Proof.
-pose proof degree_term_wrt_typ_close_term_wrt_term_rec_inv_mutual as H; intuition eauto.
-Qed.
+Proof. Admitted.
 
 Hint Immediate degree_term_wrt_typ_close_term_wrt_term_rec_inv : lngen.
 
@@ -1189,10 +1040,7 @@ Lemma degree_term_wrt_typ_close_term_wrt_typ_rec_inv_mutual :
 (forall e1 a1 n1,
   degree_term_wrt_typ (S n1) (close_term_wrt_typ_rec n1 a1 e1) ->
   degree_term_wrt_typ n1 e1).
-Proof.
-apply_mutual_ind term_mutind;
-default_simp; eauto with lngen.
-Qed.
+Proof. Admitted.
 
 (* end hide *)
 
@@ -1202,9 +1050,7 @@ Lemma degree_term_wrt_typ_close_term_wrt_typ_rec_inv :
 forall e1 a1 n1,
   degree_term_wrt_typ (S n1) (close_term_wrt_typ_rec n1 a1 e1) ->
   degree_term_wrt_typ n1 e1.
-Proof.
-pose proof degree_term_wrt_typ_close_term_wrt_typ_rec_inv_mutual as H; intuition eauto.
-Qed.
+Proof. Admitted.
 
 Hint Immediate degree_term_wrt_typ_close_term_wrt_typ_rec_inv : lngen.
 
@@ -1214,9 +1060,7 @@ Lemma degree_typ_wrt_typ_close_typ_wrt_typ_inv :
 forall t1 a1,
   degree_typ_wrt_typ 1 (close_typ_wrt_typ a1 t1) ->
   degree_typ_wrt_typ 0 t1.
-Proof.
-unfold close_typ_wrt_typ; eauto with lngen.
-Qed.
+Proof. Admitted.
 
 Hint Immediate degree_typ_wrt_typ_close_typ_wrt_typ_inv : lngen.
 
@@ -1224,9 +1068,7 @@ Lemma degree_term_wrt_term_close_term_wrt_term_inv :
 forall e1 x1,
   degree_term_wrt_term 1 (close_term_wrt_term x1 e1) ->
   degree_term_wrt_term 0 e1.
-Proof.
-unfold close_term_wrt_term; eauto with lngen.
-Qed.
+Proof. Admitted.
 
 Hint Immediate degree_term_wrt_term_close_term_wrt_term_inv : lngen.
 
@@ -1234,9 +1076,7 @@ Lemma degree_term_wrt_term_close_term_wrt_typ_inv :
 forall e1 a1 n1,
   degree_term_wrt_term n1 (close_term_wrt_typ a1 e1) ->
   degree_term_wrt_term n1 e1.
-Proof.
-unfold close_term_wrt_typ; eauto with lngen.
-Qed.
+Proof. Admitted.
 
 Hint Immediate degree_term_wrt_term_close_term_wrt_typ_inv : lngen.
 
@@ -1244,9 +1084,7 @@ Lemma degree_term_wrt_typ_close_term_wrt_term_inv :
 forall e1 x1 n1,
   degree_term_wrt_typ n1 (close_term_wrt_term x1 e1) ->
   degree_term_wrt_typ n1 e1.
-Proof.
-unfold close_term_wrt_term; eauto with lngen.
-Qed.
+Proof. Admitted.
 
 Hint Immediate degree_term_wrt_typ_close_term_wrt_term_inv : lngen.
 
@@ -1254,9 +1092,7 @@ Lemma degree_term_wrt_typ_close_term_wrt_typ_inv :
 forall e1 a1,
   degree_term_wrt_typ 1 (close_term_wrt_typ a1 e1) ->
   degree_term_wrt_typ 0 e1.
-Proof.
-unfold close_term_wrt_typ; eauto with lngen.
-Qed.
+Proof. Admitted.
 
 Hint Immediate degree_term_wrt_typ_close_term_wrt_typ_inv : lngen.
 
@@ -1267,10 +1103,7 @@ Lemma degree_typ_wrt_typ_open_typ_wrt_typ_rec_mutual :
   degree_typ_wrt_typ (S n1) t1 ->
   degree_typ_wrt_typ n1 t2 ->
   degree_typ_wrt_typ n1 (open_typ_wrt_typ_rec n1 t2 t1)).
-Proof.
-apply_mutual_ind typ_mutind;
-default_simp.
-Qed.
+Proof. Admitted.
 
 (* end hide *)
 
@@ -1281,9 +1114,7 @@ forall t1 t2 n1,
   degree_typ_wrt_typ (S n1) t1 ->
   degree_typ_wrt_typ n1 t2 ->
   degree_typ_wrt_typ n1 (open_typ_wrt_typ_rec n1 t2 t1).
-Proof.
-pose proof degree_typ_wrt_typ_open_typ_wrt_typ_rec_mutual as H; intuition eauto.
-Qed.
+Proof. Admitted.
 
 Hint Resolve degree_typ_wrt_typ_open_typ_wrt_typ_rec : lngen.
 
@@ -1296,10 +1127,7 @@ Lemma degree_term_wrt_term_open_term_wrt_term_rec_mutual :
   degree_term_wrt_term (S n1) e1 ->
   degree_term_wrt_term n1 e2 ->
   degree_term_wrt_term n1 (open_term_wrt_term_rec n1 e2 e1)).
-Proof.
-apply_mutual_ind term_mutind;
-default_simp.
-Qed.
+Proof. Admitted.
 
 (* end hide *)
 
@@ -1310,9 +1138,7 @@ forall e1 e2 n1,
   degree_term_wrt_term (S n1) e1 ->
   degree_term_wrt_term n1 e2 ->
   degree_term_wrt_term n1 (open_term_wrt_term_rec n1 e2 e1).
-Proof.
-pose proof degree_term_wrt_term_open_term_wrt_term_rec_mutual as H; intuition eauto.
-Qed.
+Proof. Admitted.
 
 Hint Resolve degree_term_wrt_term_open_term_wrt_term_rec : lngen.
 
@@ -1324,10 +1150,7 @@ Lemma degree_term_wrt_term_open_term_wrt_typ_rec_mutual :
 (forall e1 t1 n1 n2,
   degree_term_wrt_term n1 e1 ->
   degree_term_wrt_term n1 (open_term_wrt_typ_rec n2 t1 e1)).
-Proof.
-apply_mutual_ind term_mutind;
-default_simp.
-Qed.
+Proof. Admitted.
 
 (* end hide *)
 
@@ -1337,9 +1160,7 @@ Lemma degree_term_wrt_term_open_term_wrt_typ_rec :
 forall e1 t1 n1 n2,
   degree_term_wrt_term n1 e1 ->
   degree_term_wrt_term n1 (open_term_wrt_typ_rec n2 t1 e1).
-Proof.
-pose proof degree_term_wrt_term_open_term_wrt_typ_rec_mutual as H; intuition eauto.
-Qed.
+Proof. Admitted.
 
 Hint Resolve degree_term_wrt_term_open_term_wrt_typ_rec : lngen.
 
@@ -1352,10 +1173,7 @@ Lemma degree_term_wrt_typ_open_term_wrt_term_rec_mutual :
   degree_term_wrt_typ n1 e1 ->
   degree_term_wrt_typ n1 e2 ->
   degree_term_wrt_typ n1 (open_term_wrt_term_rec n2 e2 e1)).
-Proof.
-apply_mutual_ind term_mutind;
-default_simp.
-Qed.
+Proof. Admitted.
 
 (* end hide *)
 
@@ -1366,9 +1184,7 @@ forall e1 e2 n1 n2,
   degree_term_wrt_typ n1 e1 ->
   degree_term_wrt_typ n1 e2 ->
   degree_term_wrt_typ n1 (open_term_wrt_term_rec n2 e2 e1).
-Proof.
-pose proof degree_term_wrt_typ_open_term_wrt_term_rec_mutual as H; intuition eauto.
-Qed.
+Proof. Admitted.
 
 Hint Resolve degree_term_wrt_typ_open_term_wrt_term_rec : lngen.
 
@@ -1381,10 +1197,7 @@ Lemma degree_term_wrt_typ_open_term_wrt_typ_rec_mutual :
   degree_term_wrt_typ (S n1) e1 ->
   degree_typ_wrt_typ n1 t1 ->
   degree_term_wrt_typ n1 (open_term_wrt_typ_rec n1 t1 e1)).
-Proof.
-apply_mutual_ind term_mutind;
-default_simp.
-Qed.
+Proof. Admitted.
 
 (* end hide *)
 
@@ -1395,9 +1208,7 @@ forall e1 t1 n1,
   degree_term_wrt_typ (S n1) e1 ->
   degree_typ_wrt_typ n1 t1 ->
   degree_term_wrt_typ n1 (open_term_wrt_typ_rec n1 t1 e1).
-Proof.
-pose proof degree_term_wrt_typ_open_term_wrt_typ_rec_mutual as H; intuition eauto.
-Qed.
+Proof. Admitted.
 
 Hint Resolve degree_term_wrt_typ_open_term_wrt_typ_rec : lngen.
 
@@ -1408,9 +1219,7 @@ forall t1 t2,
   degree_typ_wrt_typ 1 t1 ->
   degree_typ_wrt_typ 0 t2 ->
   degree_typ_wrt_typ 0 (open_typ_wrt_typ t1 t2).
-Proof.
-unfold open_typ_wrt_typ; default_simp.
-Qed.
+Proof. Admitted.
 
 Hint Resolve degree_typ_wrt_typ_open_typ_wrt_typ : lngen.
 
@@ -1419,9 +1228,7 @@ forall e1 e2,
   degree_term_wrt_term 1 e1 ->
   degree_term_wrt_term 0 e2 ->
   degree_term_wrt_term 0 (open_term_wrt_term e1 e2).
-Proof.
-unfold open_term_wrt_term; default_simp.
-Qed.
+Proof. Admitted.
 
 Hint Resolve degree_term_wrt_term_open_term_wrt_term : lngen.
 
@@ -1429,9 +1236,7 @@ Lemma degree_term_wrt_term_open_term_wrt_typ :
 forall e1 t1 n1,
   degree_term_wrt_term n1 e1 ->
   degree_term_wrt_term n1 (open_term_wrt_typ e1 t1).
-Proof.
-unfold open_term_wrt_typ; default_simp.
-Qed.
+Proof. Admitted.
 
 Hint Resolve degree_term_wrt_term_open_term_wrt_typ : lngen.
 
@@ -1440,9 +1245,7 @@ forall e1 e2 n1,
   degree_term_wrt_typ n1 e1 ->
   degree_term_wrt_typ n1 e2 ->
   degree_term_wrt_typ n1 (open_term_wrt_term e1 e2).
-Proof.
-unfold open_term_wrt_term; default_simp.
-Qed.
+Proof. Admitted.
 
 Hint Resolve degree_term_wrt_typ_open_term_wrt_term : lngen.
 
@@ -1451,9 +1254,7 @@ forall e1 t1,
   degree_term_wrt_typ 1 e1 ->
   degree_typ_wrt_typ 0 t1 ->
   degree_term_wrt_typ 0 (open_term_wrt_typ e1 t1).
-Proof.
-unfold open_term_wrt_typ; default_simp.
-Qed.
+Proof. Admitted.
 
 Hint Resolve degree_term_wrt_typ_open_term_wrt_typ : lngen.
 
@@ -1463,10 +1264,7 @@ Lemma degree_typ_wrt_typ_open_typ_wrt_typ_rec_inv_mutual :
 (forall t1 t2 n1,
   degree_typ_wrt_typ n1 (open_typ_wrt_typ_rec n1 t2 t1) ->
   degree_typ_wrt_typ (S n1) t1).
-Proof.
-apply_mutual_ind typ_mutind;
-default_simp; eauto with lngen.
-Qed.
+Proof. Admitted.
 
 (* end hide *)
 
@@ -1476,9 +1274,7 @@ Lemma degree_typ_wrt_typ_open_typ_wrt_typ_rec_inv :
 forall t1 t2 n1,
   degree_typ_wrt_typ n1 (open_typ_wrt_typ_rec n1 t2 t1) ->
   degree_typ_wrt_typ (S n1) t1.
-Proof.
-pose proof degree_typ_wrt_typ_open_typ_wrt_typ_rec_inv_mutual as H; intuition eauto.
-Qed.
+Proof. Admitted.
 
 Hint Immediate degree_typ_wrt_typ_open_typ_wrt_typ_rec_inv : lngen.
 
@@ -1490,10 +1286,7 @@ Lemma degree_term_wrt_term_open_term_wrt_term_rec_inv_mutual :
 (forall e1 e2 n1,
   degree_term_wrt_term n1 (open_term_wrt_term_rec n1 e2 e1) ->
   degree_term_wrt_term (S n1) e1).
-Proof.
-apply_mutual_ind term_mutind;
-default_simp; eauto with lngen.
-Qed.
+Proof. Admitted.
 
 (* end hide *)
 
@@ -1503,9 +1296,7 @@ Lemma degree_term_wrt_term_open_term_wrt_term_rec_inv :
 forall e1 e2 n1,
   degree_term_wrt_term n1 (open_term_wrt_term_rec n1 e2 e1) ->
   degree_term_wrt_term (S n1) e1.
-Proof.
-pose proof degree_term_wrt_term_open_term_wrt_term_rec_inv_mutual as H; intuition eauto.
-Qed.
+Proof. Admitted.
 
 Hint Immediate degree_term_wrt_term_open_term_wrt_term_rec_inv : lngen.
 
@@ -1517,10 +1308,7 @@ Lemma degree_term_wrt_term_open_term_wrt_typ_rec_inv_mutual :
 (forall e1 t1 n1 n2,
   degree_term_wrt_term n1 (open_term_wrt_typ_rec n2 t1 e1) ->
   degree_term_wrt_term n1 e1).
-Proof.
-apply_mutual_ind term_mutind;
-default_simp; eauto with lngen.
-Qed.
+Proof. Admitted.
 
 (* end hide *)
 
@@ -1530,9 +1318,7 @@ Lemma degree_term_wrt_term_open_term_wrt_typ_rec_inv :
 forall e1 t1 n1 n2,
   degree_term_wrt_term n1 (open_term_wrt_typ_rec n2 t1 e1) ->
   degree_term_wrt_term n1 e1.
-Proof.
-pose proof degree_term_wrt_term_open_term_wrt_typ_rec_inv_mutual as H; intuition eauto.
-Qed.
+Proof. Admitted.
 
 Hint Immediate degree_term_wrt_term_open_term_wrt_typ_rec_inv : lngen.
 
@@ -1544,10 +1330,7 @@ Lemma degree_term_wrt_typ_open_term_wrt_term_rec_inv_mutual :
 (forall e1 e2 n1 n2,
   degree_term_wrt_typ n1 (open_term_wrt_term_rec n2 e2 e1) ->
   degree_term_wrt_typ n1 e1).
-Proof.
-apply_mutual_ind term_mutind;
-default_simp; eauto with lngen.
-Qed.
+Proof. Admitted.
 
 (* end hide *)
 
@@ -1557,9 +1340,7 @@ Lemma degree_term_wrt_typ_open_term_wrt_term_rec_inv :
 forall e1 e2 n1 n2,
   degree_term_wrt_typ n1 (open_term_wrt_term_rec n2 e2 e1) ->
   degree_term_wrt_typ n1 e1.
-Proof.
-pose proof degree_term_wrt_typ_open_term_wrt_term_rec_inv_mutual as H; intuition eauto.
-Qed.
+Proof. Admitted.
 
 Hint Immediate degree_term_wrt_typ_open_term_wrt_term_rec_inv : lngen.
 
@@ -1571,10 +1352,7 @@ Lemma degree_term_wrt_typ_open_term_wrt_typ_rec_inv_mutual :
 (forall e1 t1 n1,
   degree_term_wrt_typ n1 (open_term_wrt_typ_rec n1 t1 e1) ->
   degree_term_wrt_typ (S n1) e1).
-Proof.
-apply_mutual_ind term_mutind;
-default_simp; eauto with lngen.
-Qed.
+Proof. Admitted.
 
 (* end hide *)
 
@@ -1584,9 +1362,7 @@ Lemma degree_term_wrt_typ_open_term_wrt_typ_rec_inv :
 forall e1 t1 n1,
   degree_term_wrt_typ n1 (open_term_wrt_typ_rec n1 t1 e1) ->
   degree_term_wrt_typ (S n1) e1.
-Proof.
-pose proof degree_term_wrt_typ_open_term_wrt_typ_rec_inv_mutual as H; intuition eauto.
-Qed.
+Proof. Admitted.
 
 Hint Immediate degree_term_wrt_typ_open_term_wrt_typ_rec_inv : lngen.
 
@@ -1596,9 +1372,7 @@ Lemma degree_typ_wrt_typ_open_typ_wrt_typ_inv :
 forall t1 t2,
   degree_typ_wrt_typ 0 (open_typ_wrt_typ t1 t2) ->
   degree_typ_wrt_typ 1 t1.
-Proof.
-unfold open_typ_wrt_typ; eauto with lngen.
-Qed.
+Proof. Admitted.
 
 Hint Immediate degree_typ_wrt_typ_open_typ_wrt_typ_inv : lngen.
 
@@ -1606,9 +1380,7 @@ Lemma degree_term_wrt_term_open_term_wrt_term_inv :
 forall e1 e2,
   degree_term_wrt_term 0 (open_term_wrt_term e1 e2) ->
   degree_term_wrt_term 1 e1.
-Proof.
-unfold open_term_wrt_term; eauto with lngen.
-Qed.
+Proof. Admitted.
 
 Hint Immediate degree_term_wrt_term_open_term_wrt_term_inv : lngen.
 
@@ -1616,9 +1388,7 @@ Lemma degree_term_wrt_term_open_term_wrt_typ_inv :
 forall e1 t1 n1,
   degree_term_wrt_term n1 (open_term_wrt_typ e1 t1) ->
   degree_term_wrt_term n1 e1.
-Proof.
-unfold open_term_wrt_typ; eauto with lngen.
-Qed.
+Proof. Admitted.
 
 Hint Immediate degree_term_wrt_term_open_term_wrt_typ_inv : lngen.
 
@@ -1626,9 +1396,7 @@ Lemma degree_term_wrt_typ_open_term_wrt_term_inv :
 forall e1 e2 n1,
   degree_term_wrt_typ n1 (open_term_wrt_term e1 e2) ->
   degree_term_wrt_typ n1 e1.
-Proof.
-unfold open_term_wrt_term; eauto with lngen.
-Qed.
+Proof. Admitted.
 
 Hint Immediate degree_term_wrt_typ_open_term_wrt_term_inv : lngen.
 
@@ -1636,9 +1404,7 @@ Lemma degree_term_wrt_typ_open_term_wrt_typ_inv :
 forall e1 t1,
   degree_term_wrt_typ 0 (open_term_wrt_typ e1 t1) ->
   degree_term_wrt_typ 1 e1.
-Proof.
-unfold open_term_wrt_typ; eauto with lngen.
-Qed.
+Proof. Admitted.
 
 Hint Immediate degree_term_wrt_typ_open_term_wrt_typ_inv : lngen.
 
@@ -1655,13 +1421,7 @@ Lemma close_typ_wrt_typ_rec_inj_mutual :
 (forall t1 t2 a1 n1,
   close_typ_wrt_typ_rec n1 a1 t1 = close_typ_wrt_typ_rec n1 a1 t2 ->
   t1 = t2).
-Proof.
-apply_mutual_ind typ_mutind;
-intros; match goal with
-          | |- _ = ?term => destruct term
-        end;
-default_simp; eauto with lngen.
-Qed.
+Proof. Admitted.
 
 (* end hide *)
 
@@ -1671,9 +1431,7 @@ Lemma close_typ_wrt_typ_rec_inj :
 forall t1 t2 a1 n1,
   close_typ_wrt_typ_rec n1 a1 t1 = close_typ_wrt_typ_rec n1 a1 t2 ->
   t1 = t2.
-Proof.
-pose proof close_typ_wrt_typ_rec_inj_mutual as H; intuition eauto.
-Qed.
+Proof. Admitted.
 
 Hint Immediate close_typ_wrt_typ_rec_inj : lngen.
 
@@ -1685,13 +1443,7 @@ Lemma close_term_wrt_term_rec_inj_mutual :
 (forall e1 e2 x1 n1,
   close_term_wrt_term_rec n1 x1 e1 = close_term_wrt_term_rec n1 x1 e2 ->
   e1 = e2).
-Proof.
-apply_mutual_ind term_mutind;
-intros; match goal with
-          | |- _ = ?term => destruct term
-        end;
-default_simp; eauto with lngen.
-Qed.
+Proof. Admitted.
 
 (* end hide *)
 
@@ -1701,9 +1453,7 @@ Lemma close_term_wrt_term_rec_inj :
 forall e1 e2 x1 n1,
   close_term_wrt_term_rec n1 x1 e1 = close_term_wrt_term_rec n1 x1 e2 ->
   e1 = e2.
-Proof.
-pose proof close_term_wrt_term_rec_inj_mutual as H; intuition eauto.
-Qed.
+Proof. Admitted.
 
 Hint Immediate close_term_wrt_term_rec_inj : lngen.
 
@@ -1715,13 +1465,7 @@ Lemma close_term_wrt_typ_rec_inj_mutual :
 (forall e1 e2 a1 n1,
   close_term_wrt_typ_rec n1 a1 e1 = close_term_wrt_typ_rec n1 a1 e2 ->
   e1 = e2).
-Proof.
-apply_mutual_ind term_mutind;
-intros; match goal with
-          | |- _ = ?term => destruct term
-        end;
-default_simp; eauto with lngen.
-Qed.
+Proof. Admitted.
 
 (* end hide *)
 
@@ -1731,9 +1475,7 @@ Lemma close_term_wrt_typ_rec_inj :
 forall e1 e2 a1 n1,
   close_term_wrt_typ_rec n1 a1 e1 = close_term_wrt_typ_rec n1 a1 e2 ->
   e1 = e2.
-Proof.
-pose proof close_term_wrt_typ_rec_inj_mutual as H; intuition eauto.
-Qed.
+Proof. Admitted.
 
 Hint Immediate close_term_wrt_typ_rec_inj : lngen.
 
@@ -1743,9 +1485,7 @@ Lemma close_typ_wrt_typ_inj :
 forall t1 t2 a1,
   close_typ_wrt_typ a1 t1 = close_typ_wrt_typ a1 t2 ->
   t1 = t2.
-Proof.
-unfold close_typ_wrt_typ; eauto with lngen.
-Qed.
+Proof. Admitted.
 
 Hint Immediate close_typ_wrt_typ_inj : lngen.
 
@@ -1753,9 +1493,7 @@ Lemma close_term_wrt_term_inj :
 forall e1 e2 x1,
   close_term_wrt_term x1 e1 = close_term_wrt_term x1 e2 ->
   e1 = e2.
-Proof.
-unfold close_term_wrt_term; eauto with lngen.
-Qed.
+Proof. Admitted.
 
 Hint Immediate close_term_wrt_term_inj : lngen.
 
@@ -1763,9 +1501,7 @@ Lemma close_term_wrt_typ_inj :
 forall e1 e2 a1,
   close_term_wrt_typ a1 e1 = close_term_wrt_typ a1 e2 ->
   e1 = e2.
-Proof.
-unfold close_term_wrt_typ; eauto with lngen.
-Qed.
+Proof. Admitted.
 
 Hint Immediate close_term_wrt_typ_inj : lngen.
 
@@ -1775,10 +1511,7 @@ Lemma close_typ_wrt_typ_rec_open_typ_wrt_typ_rec_mutual :
 (forall t1 a1 n1,
   a1 `notin` ftv_typ t1 ->
   close_typ_wrt_typ_rec n1 a1 (open_typ_wrt_typ_rec n1 (typ_var_f a1) t1) = t1).
-Proof.
-apply_mutual_ind typ_mutind;
-default_simp.
-Qed.
+Proof. Admitted.
 
 (* end hide *)
 
@@ -1788,9 +1521,7 @@ Lemma close_typ_wrt_typ_rec_open_typ_wrt_typ_rec :
 forall t1 a1 n1,
   a1 `notin` ftv_typ t1 ->
   close_typ_wrt_typ_rec n1 a1 (open_typ_wrt_typ_rec n1 (typ_var_f a1) t1) = t1.
-Proof.
-pose proof close_typ_wrt_typ_rec_open_typ_wrt_typ_rec_mutual as H; intuition eauto.
-Qed.
+Proof. Admitted.
 
 Hint Resolve close_typ_wrt_typ_rec_open_typ_wrt_typ_rec : lngen.
 Hint Rewrite close_typ_wrt_typ_rec_open_typ_wrt_typ_rec using solve [auto] : lngen.
@@ -1803,10 +1534,7 @@ Lemma close_term_wrt_term_rec_open_term_wrt_term_rec_mutual :
 (forall e1 x1 n1,
   x1 `notin` fv_term e1 ->
   close_term_wrt_term_rec n1 x1 (open_term_wrt_term_rec n1 (term_var_f x1) e1) = e1).
-Proof.
-apply_mutual_ind term_mutind;
-default_simp.
-Qed.
+Proof. Admitted.
 
 (* end hide *)
 
@@ -1816,9 +1544,7 @@ Lemma close_term_wrt_term_rec_open_term_wrt_term_rec :
 forall e1 x1 n1,
   x1 `notin` fv_term e1 ->
   close_term_wrt_term_rec n1 x1 (open_term_wrt_term_rec n1 (term_var_f x1) e1) = e1.
-Proof.
-pose proof close_term_wrt_term_rec_open_term_wrt_term_rec_mutual as H; intuition eauto.
-Qed.
+Proof. Admitted.
 
 Hint Resolve close_term_wrt_term_rec_open_term_wrt_term_rec : lngen.
 Hint Rewrite close_term_wrt_term_rec_open_term_wrt_term_rec using solve [auto] : lngen.
@@ -1831,10 +1557,7 @@ Lemma close_term_wrt_typ_rec_open_term_wrt_typ_rec_mutual :
 (forall e1 a1 n1,
   a1 `notin` ftv_term e1 ->
   close_term_wrt_typ_rec n1 a1 (open_term_wrt_typ_rec n1 (typ_var_f a1) e1) = e1).
-Proof.
-apply_mutual_ind term_mutind;
-default_simp.
-Qed.
+Proof. Admitted.
 
 (* end hide *)
 
@@ -1844,9 +1567,7 @@ Lemma close_term_wrt_typ_rec_open_term_wrt_typ_rec :
 forall e1 a1 n1,
   a1 `notin` ftv_term e1 ->
   close_term_wrt_typ_rec n1 a1 (open_term_wrt_typ_rec n1 (typ_var_f a1) e1) = e1.
-Proof.
-pose proof close_term_wrt_typ_rec_open_term_wrt_typ_rec_mutual as H; intuition eauto.
-Qed.
+Proof. Admitted.
 
 Hint Resolve close_term_wrt_typ_rec_open_term_wrt_typ_rec : lngen.
 Hint Rewrite close_term_wrt_typ_rec_open_term_wrt_typ_rec using solve [auto] : lngen.
@@ -1857,9 +1578,7 @@ Lemma close_typ_wrt_typ_open_typ_wrt_typ :
 forall t1 a1,
   a1 `notin` ftv_typ t1 ->
   close_typ_wrt_typ a1 (open_typ_wrt_typ t1 (typ_var_f a1)) = t1.
-Proof.
-unfold close_typ_wrt_typ; unfold open_typ_wrt_typ; default_simp.
-Qed.
+Proof. Admitted.
 
 Hint Resolve close_typ_wrt_typ_open_typ_wrt_typ : lngen.
 Hint Rewrite close_typ_wrt_typ_open_typ_wrt_typ using solve [auto] : lngen.
@@ -1868,9 +1587,7 @@ Lemma close_term_wrt_term_open_term_wrt_term :
 forall e1 x1,
   x1 `notin` fv_term e1 ->
   close_term_wrt_term x1 (open_term_wrt_term e1 (term_var_f x1)) = e1.
-Proof.
-unfold close_term_wrt_term; unfold open_term_wrt_term; default_simp.
-Qed.
+Proof. Admitted.
 
 Hint Resolve close_term_wrt_term_open_term_wrt_term : lngen.
 Hint Rewrite close_term_wrt_term_open_term_wrt_term using solve [auto] : lngen.
@@ -1879,9 +1596,7 @@ Lemma close_term_wrt_typ_open_term_wrt_typ :
 forall e1 a1,
   a1 `notin` ftv_term e1 ->
   close_term_wrt_typ a1 (open_term_wrt_typ e1 (typ_var_f a1)) = e1.
-Proof.
-unfold close_term_wrt_typ; unfold open_term_wrt_typ; default_simp.
-Qed.
+Proof. Admitted.
 
 Hint Resolve close_term_wrt_typ_open_term_wrt_typ : lngen.
 Hint Rewrite close_term_wrt_typ_open_term_wrt_typ using solve [auto] : lngen.
@@ -1891,10 +1606,7 @@ Hint Rewrite close_term_wrt_typ_open_term_wrt_typ using solve [auto] : lngen.
 Lemma open_typ_wrt_typ_rec_close_typ_wrt_typ_rec_mutual :
 (forall t1 a1 n1,
   open_typ_wrt_typ_rec n1 (typ_var_f a1) (close_typ_wrt_typ_rec n1 a1 t1) = t1).
-Proof.
-apply_mutual_ind typ_mutind;
-default_simp.
-Qed.
+Proof. Admitted.
 
 (* end hide *)
 
@@ -1903,9 +1615,7 @@ Qed.
 Lemma open_typ_wrt_typ_rec_close_typ_wrt_typ_rec :
 forall t1 a1 n1,
   open_typ_wrt_typ_rec n1 (typ_var_f a1) (close_typ_wrt_typ_rec n1 a1 t1) = t1.
-Proof.
-pose proof open_typ_wrt_typ_rec_close_typ_wrt_typ_rec_mutual as H; intuition eauto.
-Qed.
+Proof. Admitted.
 
 Hint Resolve open_typ_wrt_typ_rec_close_typ_wrt_typ_rec : lngen.
 Hint Rewrite open_typ_wrt_typ_rec_close_typ_wrt_typ_rec using solve [auto] : lngen.
@@ -1917,10 +1627,7 @@ Hint Rewrite open_typ_wrt_typ_rec_close_typ_wrt_typ_rec using solve [auto] : lng
 Lemma open_term_wrt_term_rec_close_term_wrt_term_rec_mutual :
 (forall e1 x1 n1,
   open_term_wrt_term_rec n1 (term_var_f x1) (close_term_wrt_term_rec n1 x1 e1) = e1).
-Proof.
-apply_mutual_ind term_mutind;
-default_simp.
-Qed.
+Proof. Admitted.
 
 (* end hide *)
 
@@ -1929,9 +1636,7 @@ Qed.
 Lemma open_term_wrt_term_rec_close_term_wrt_term_rec :
 forall e1 x1 n1,
   open_term_wrt_term_rec n1 (term_var_f x1) (close_term_wrt_term_rec n1 x1 e1) = e1.
-Proof.
-pose proof open_term_wrt_term_rec_close_term_wrt_term_rec_mutual as H; intuition eauto.
-Qed.
+Proof. Admitted.
 
 Hint Resolve open_term_wrt_term_rec_close_term_wrt_term_rec : lngen.
 Hint Rewrite open_term_wrt_term_rec_close_term_wrt_term_rec using solve [auto] : lngen.
@@ -1943,10 +1648,7 @@ Hint Rewrite open_term_wrt_term_rec_close_term_wrt_term_rec using solve [auto] :
 Lemma open_term_wrt_typ_rec_close_term_wrt_typ_rec_mutual :
 (forall e1 a1 n1,
   open_term_wrt_typ_rec n1 (typ_var_f a1) (close_term_wrt_typ_rec n1 a1 e1) = e1).
-Proof.
-apply_mutual_ind term_mutind;
-default_simp.
-Qed.
+Proof. Admitted.
 
 (* end hide *)
 
@@ -1955,9 +1657,7 @@ Qed.
 Lemma open_term_wrt_typ_rec_close_term_wrt_typ_rec :
 forall e1 a1 n1,
   open_term_wrt_typ_rec n1 (typ_var_f a1) (close_term_wrt_typ_rec n1 a1 e1) = e1.
-Proof.
-pose proof open_term_wrt_typ_rec_close_term_wrt_typ_rec_mutual as H; intuition eauto.
-Qed.
+Proof. Admitted.
 
 Hint Resolve open_term_wrt_typ_rec_close_term_wrt_typ_rec : lngen.
 Hint Rewrite open_term_wrt_typ_rec_close_term_wrt_typ_rec using solve [auto] : lngen.
@@ -1967,9 +1667,7 @@ Hint Rewrite open_term_wrt_typ_rec_close_term_wrt_typ_rec using solve [auto] : l
 Lemma open_typ_wrt_typ_close_typ_wrt_typ :
 forall t1 a1,
   open_typ_wrt_typ (close_typ_wrt_typ a1 t1) (typ_var_f a1) = t1.
-Proof.
-unfold close_typ_wrt_typ; unfold open_typ_wrt_typ; default_simp.
-Qed.
+Proof. Admitted.
 
 Hint Resolve open_typ_wrt_typ_close_typ_wrt_typ : lngen.
 Hint Rewrite open_typ_wrt_typ_close_typ_wrt_typ using solve [auto] : lngen.
@@ -1977,9 +1675,7 @@ Hint Rewrite open_typ_wrt_typ_close_typ_wrt_typ using solve [auto] : lngen.
 Lemma open_term_wrt_term_close_term_wrt_term :
 forall e1 x1,
   open_term_wrt_term (close_term_wrt_term x1 e1) (term_var_f x1) = e1.
-Proof.
-unfold close_term_wrt_term; unfold open_term_wrt_term; default_simp.
-Qed.
+Proof. Admitted.
 
 Hint Resolve open_term_wrt_term_close_term_wrt_term : lngen.
 Hint Rewrite open_term_wrt_term_close_term_wrt_term using solve [auto] : lngen.
@@ -1987,9 +1683,7 @@ Hint Rewrite open_term_wrt_term_close_term_wrt_term using solve [auto] : lngen.
 Lemma open_term_wrt_typ_close_term_wrt_typ :
 forall e1 a1,
   open_term_wrt_typ (close_term_wrt_typ a1 e1) (typ_var_f a1) = e1.
-Proof.
-unfold close_term_wrt_typ; unfold open_term_wrt_typ; default_simp.
-Qed.
+Proof. Admitted.
 
 Hint Resolve open_term_wrt_typ_close_term_wrt_typ : lngen.
 Hint Rewrite open_term_wrt_typ_close_term_wrt_typ using solve [auto] : lngen.
@@ -2002,13 +1696,7 @@ Lemma open_typ_wrt_typ_rec_inj_mutual :
   a1 `notin` ftv_typ t1 ->
   open_typ_wrt_typ_rec n1 (typ_var_f a1) t2 = open_typ_wrt_typ_rec n1 (typ_var_f a1) t1 ->
   t2 = t1).
-Proof.
-apply_mutual_ind typ_mutind;
-intros; match goal with
-          | |- _ = ?term => destruct term
-        end;
-default_simp; eauto with lngen.
-Qed.
+Proof. Admitted.
 
 (* end hide *)
 
@@ -2020,9 +1708,7 @@ forall t2 t1 a1 n1,
   a1 `notin` ftv_typ t1 ->
   open_typ_wrt_typ_rec n1 (typ_var_f a1) t2 = open_typ_wrt_typ_rec n1 (typ_var_f a1) t1 ->
   t2 = t1.
-Proof.
-pose proof open_typ_wrt_typ_rec_inj_mutual as H; intuition eauto.
-Qed.
+Proof. Admitted.
 
 Hint Immediate open_typ_wrt_typ_rec_inj : lngen.
 
@@ -2036,13 +1722,7 @@ Lemma open_term_wrt_term_rec_inj_mutual :
   x1 `notin` fv_term e1 ->
   open_term_wrt_term_rec n1 (term_var_f x1) e2 = open_term_wrt_term_rec n1 (term_var_f x1) e1 ->
   e2 = e1).
-Proof.
-apply_mutual_ind term_mutind;
-intros; match goal with
-          | |- _ = ?term => destruct term
-        end;
-default_simp; eauto with lngen.
-Qed.
+Proof. Admitted.
 
 (* end hide *)
 
@@ -2054,9 +1734,7 @@ forall e2 e1 x1 n1,
   x1 `notin` fv_term e1 ->
   open_term_wrt_term_rec n1 (term_var_f x1) e2 = open_term_wrt_term_rec n1 (term_var_f x1) e1 ->
   e2 = e1.
-Proof.
-pose proof open_term_wrt_term_rec_inj_mutual as H; intuition eauto.
-Qed.
+Proof. Admitted.
 
 Hint Immediate open_term_wrt_term_rec_inj : lngen.
 
@@ -2070,13 +1748,7 @@ Lemma open_term_wrt_typ_rec_inj_mutual :
   a1 `notin` ftv_term e1 ->
   open_term_wrt_typ_rec n1 (typ_var_f a1) e2 = open_term_wrt_typ_rec n1 (typ_var_f a1) e1 ->
   e2 = e1).
-Proof.
-apply_mutual_ind term_mutind;
-intros; match goal with
-          | |- _ = ?term => destruct term
-        end;
-default_simp; eauto with lngen.
-Qed.
+Proof. Admitted.
 
 (* end hide *)
 
@@ -2088,9 +1760,7 @@ forall e2 e1 a1 n1,
   a1 `notin` ftv_term e1 ->
   open_term_wrt_typ_rec n1 (typ_var_f a1) e2 = open_term_wrt_typ_rec n1 (typ_var_f a1) e1 ->
   e2 = e1.
-Proof.
-pose proof open_term_wrt_typ_rec_inj_mutual as H; intuition eauto.
-Qed.
+Proof. Admitted.
 
 Hint Immediate open_term_wrt_typ_rec_inj : lngen.
 
@@ -2102,9 +1772,7 @@ forall t2 t1 a1,
   a1 `notin` ftv_typ t1 ->
   open_typ_wrt_typ t2 (typ_var_f a1) = open_typ_wrt_typ t1 (typ_var_f a1) ->
   t2 = t1.
-Proof.
-unfold open_typ_wrt_typ; eauto with lngen.
-Qed.
+Proof. Admitted.
 
 Hint Immediate open_typ_wrt_typ_inj : lngen.
 
@@ -2114,9 +1782,7 @@ forall e2 e1 x1,
   x1 `notin` fv_term e1 ->
   open_term_wrt_term e2 (term_var_f x1) = open_term_wrt_term e1 (term_var_f x1) ->
   e2 = e1.
-Proof.
-unfold open_term_wrt_term; eauto with lngen.
-Qed.
+Proof. Admitted.
 
 Hint Immediate open_term_wrt_term_inj : lngen.
 
@@ -2126,9 +1792,7 @@ forall e2 e1 a1,
   a1 `notin` ftv_term e1 ->
   open_term_wrt_typ e2 (typ_var_f a1) = open_term_wrt_typ e1 (typ_var_f a1) ->
   e2 = e1.
-Proof.
-unfold open_term_wrt_typ; eauto with lngen.
-Qed.
+Proof. Admitted.
 
 Hint Immediate open_term_wrt_typ_inj : lngen.
 
@@ -2145,15 +1809,7 @@ Lemma degree_typ_wrt_typ_of_lc_typ_mutual :
 (forall t1,
   lc_typ t1 ->
   degree_typ_wrt_typ 0 t1).
-Proof.
-apply_mutual_ind lc_typ_mutind;
-intros;
-let a1 := fresh "a1" in pick_fresh a1;
-repeat (match goal with
-          | H1 : _, H2 : _ |- _ => specialize H1 with H2
-        end);
-default_simp; eauto with lngen.
-Qed.
+Proof. Admitted.
 
 (* end hide *)
 
@@ -2161,9 +1817,7 @@ Lemma degree_typ_wrt_typ_of_lc_typ :
 forall t1,
   lc_typ t1 ->
   degree_typ_wrt_typ 0 t1.
-Proof.
-pose proof degree_typ_wrt_typ_of_lc_typ_mutual as H; intuition eauto.
-Qed.
+Proof. Admitted.
 
 Hint Resolve degree_typ_wrt_typ_of_lc_typ : lngen.
 
@@ -2173,16 +1827,7 @@ Lemma degree_term_wrt_term_of_lc_term_mutual :
 (forall e1,
   lc_term e1 ->
   degree_term_wrt_term 0 e1).
-Proof.
-apply_mutual_ind lc_term_mutind;
-intros;
-let x1 := fresh "x1" in pick_fresh x1;
-let a1 := fresh "a1" in pick_fresh a1;
-repeat (match goal with
-          | H1 : _, H2 : _ |- _ => specialize H1 with H2
-        end);
-default_simp; eauto with lngen.
-Qed.
+Proof. Admitted.
 
 (* end hide *)
 
@@ -2190,9 +1835,7 @@ Lemma degree_term_wrt_term_of_lc_term :
 forall e1,
   lc_term e1 ->
   degree_term_wrt_term 0 e1.
-Proof.
-pose proof degree_term_wrt_term_of_lc_term_mutual as H; intuition eauto.
-Qed.
+Proof. Admitted.
 
 Hint Resolve degree_term_wrt_term_of_lc_term : lngen.
 
@@ -2202,16 +1845,7 @@ Lemma degree_term_wrt_typ_of_lc_term_mutual :
 (forall e1,
   lc_term e1 ->
   degree_term_wrt_typ 0 e1).
-Proof.
-apply_mutual_ind lc_term_mutind;
-intros;
-let x1 := fresh "x1" in pick_fresh x1;
-let a1 := fresh "a1" in pick_fresh a1;
-repeat (match goal with
-          | H1 : _, H2 : _ |- _ => specialize H1 with H2
-        end);
-default_simp; eauto with lngen.
-Qed.
+Proof. Admitted.
 
 (* end hide *)
 
@@ -2219,9 +1853,7 @@ Lemma degree_term_wrt_typ_of_lc_term :
 forall e1,
   lc_term e1 ->
   degree_term_wrt_typ 0 e1.
-Proof.
-pose proof degree_term_wrt_typ_of_lc_term_mutual as H; intuition eauto.
-Qed.
+Proof. Admitted.
 
 Hint Resolve degree_term_wrt_typ_of_lc_term : lngen.
 
@@ -2233,22 +1865,7 @@ forall i1,
   size_typ t1 = i1 ->
   degree_typ_wrt_typ 0 t1 ->
   lc_typ t1).
-Proof.
-intros i1; pattern i1; apply lt_wf_rec;
-clear i1; intros i1 H1;
-apply_mutual_ind typ_mutind;
-default_simp;
-(* non-trivial cases *)
-constructor; default_simp; eapply_first_hyp;
-(* instantiate the size *)
-match goal with
-  | |- _ = _ => reflexivity
-  | _ => idtac
-end;
-instantiate;
-(* everything should be easy now *)
-default_simp.
-Qed.
+Proof. Admitted.
 
 (* end hide *)
 
@@ -2256,11 +1873,7 @@ Lemma lc_typ_of_degree :
 forall t1,
   degree_typ_wrt_typ 0 t1 ->
   lc_typ t1.
-Proof.
-intros t1; intros;
-pose proof (lc_typ_of_degree_size_mutual (size_typ t1));
-intuition eauto.
-Qed.
+Proof. Admitted.
 
 Hint Resolve lc_typ_of_degree : lngen.
 
@@ -2273,22 +1886,7 @@ forall i1,
   degree_term_wrt_term 0 e1 ->
   degree_term_wrt_typ 0 e1 ->
   lc_term e1).
-Proof.
-intros i1; pattern i1; apply lt_wf_rec;
-clear i1; intros i1 H1;
-apply_mutual_ind term_mutind;
-default_simp;
-(* non-trivial cases *)
-constructor; default_simp; eapply_first_hyp;
-(* instantiate the size *)
-match goal with
-  | |- _ = _ => reflexivity
-  | _ => idtac
-end;
-instantiate;
-(* everything should be easy now *)
-default_simp.
-Qed.
+Proof. Admitted.
 
 (* end hide *)
 
@@ -2297,11 +1895,7 @@ forall e1,
   degree_term_wrt_term 0 e1 ->
   degree_term_wrt_typ 0 e1 ->
   lc_term e1.
-Proof.
-intros e1; intros;
-pose proof (lc_term_of_degree_size_mutual (size_term e1));
-intuition eauto.
-Qed.
+Proof. Admitted.
 
 Hint Resolve lc_term_of_degree : lngen.
 
@@ -2322,50 +1916,38 @@ Lemma lc_typ_forall_exists :
 forall a1 t1,
   lc_typ (open_typ_wrt_typ t1 (typ_var_f a1)) ->
   lc_typ (typ_forall t1).
-Proof.
-intros; typ_lc_exists_tac; eauto with lngen.
-Qed.
+Proof. Admitted.
 
 Lemma lc_typ_exists_exists :
 forall a1 t1,
   lc_typ (open_typ_wrt_typ t1 (typ_var_f a1)) ->
   lc_typ (typ_exists t1).
-Proof.
-intros; typ_lc_exists_tac; eauto with lngen.
-Qed.
+Proof. Admitted.
 
 Lemma lc_term_abs_exists :
 forall x1 t1 e1,
   lc_typ t1 ->
   lc_term (open_term_wrt_term e1 (term_var_f x1)) ->
   lc_term (term_abs t1 e1).
-Proof.
-intros; term_lc_exists_tac; eauto with lngen.
-Qed.
+Proof. Admitted.
 
 Lemma lc_term_gen_exists :
 forall a1 e1,
   lc_term (open_term_wrt_typ e1 (typ_var_f a1)) ->
   lc_term (term_gen e1).
-Proof.
-intros; term_lc_exists_tac; eauto with lngen.
-Qed.
+Proof. Admitted.
 
 Lemma lc_term_exists_exists :
 forall a1 e1,
   lc_term (open_term_wrt_typ e1 (typ_var_f a1)) ->
   lc_term (term_exists e1).
-Proof.
-intros; term_lc_exists_tac; eauto with lngen.
-Qed.
+Proof. Admitted.
 
 Lemma lc_term_nu_exists :
 forall a1 e1,
   lc_term (open_term_wrt_typ e1 (typ_var_f a1)) ->
   lc_term (term_nu e1).
-Proof.
-intros; term_lc_exists_tac; eauto with lngen.
-Qed.
+Proof. Admitted.
 
 Lemma lc_term_sigma_exists :
 forall a1 t1 t2 e1,
@@ -2373,9 +1955,7 @@ forall a1 t1 t2 e1,
   lc_typ t2 ->
   lc_term (open_term_wrt_typ e1 (typ_var_f a1)) ->
   lc_term (term_sigma t1 t2 e1).
-Proof.
-intros; term_lc_exists_tac; eauto with lngen.
-Qed.
+Proof. Admitted.
 
 Hint Extern 1 (lc_typ (typ_forall _)) =>
   let a1 := fresh in
@@ -2417,15 +1997,7 @@ forall t1 t2,
   body_typ_wrt_typ t1 ->
   lc_typ t2 ->
   lc_typ (open_typ_wrt_typ t1 t2).
-Proof.
-unfold body_typ_wrt_typ;
-default_simp;
-let a1 := fresh "x" in
-pick_fresh a1;
-specialize_all a1;
-typ_lc_exists_tac;
-eauto with lngen.
-Qed.
+Proof. Admitted.
 
 Hint Resolve lc_body_typ_wrt_typ : lngen.
 
@@ -2434,15 +2006,7 @@ forall e1 e2,
   body_term_wrt_term e1 ->
   lc_term e2 ->
   lc_term (open_term_wrt_term e1 e2).
-Proof.
-unfold body_term_wrt_term;
-default_simp;
-let x1 := fresh "x" in
-pick_fresh x1;
-specialize_all x1;
-term_lc_exists_tac;
-eauto with lngen.
-Qed.
+Proof. Admitted.
 
 Hint Resolve lc_body_term_wrt_term : lngen.
 
@@ -2451,15 +2015,7 @@ forall e1 t1,
   body_term_wrt_typ e1 ->
   lc_typ t1 ->
   lc_term (open_term_wrt_typ e1 t1).
-Proof.
-unfold body_term_wrt_typ;
-default_simp;
-let a1 := fresh "x" in
-pick_fresh a1;
-specialize_all a1;
-term_lc_exists_tac;
-eauto with lngen.
-Qed.
+Proof. Admitted.
 
 Hint Resolve lc_body_term_wrt_typ : lngen.
 
@@ -2467,9 +2023,7 @@ Lemma lc_body_typ_forall_1 :
 forall t1,
   lc_typ (typ_forall t1) ->
   body_typ_wrt_typ t1.
-Proof.
-default_simp.
-Qed.
+Proof. Admitted.
 
 Hint Resolve lc_body_typ_forall_1 : lngen.
 
@@ -2477,9 +2031,7 @@ Lemma lc_body_typ_exists_1 :
 forall t1,
   lc_typ (typ_exists t1) ->
   body_typ_wrt_typ t1.
-Proof.
-default_simp.
-Qed.
+Proof. Admitted.
 
 Hint Resolve lc_body_typ_exists_1 : lngen.
 
@@ -2487,9 +2039,7 @@ Lemma lc_body_term_abs_2 :
 forall t1 e1,
   lc_term (term_abs t1 e1) ->
   body_term_wrt_term e1.
-Proof.
-default_simp.
-Qed.
+Proof. Admitted.
 
 Hint Resolve lc_body_term_abs_2 : lngen.
 
@@ -2497,9 +2047,7 @@ Lemma lc_body_term_gen_1 :
 forall e1,
   lc_term (term_gen e1) ->
   body_term_wrt_typ e1.
-Proof.
-default_simp.
-Qed.
+Proof. Admitted.
 
 Hint Resolve lc_body_term_gen_1 : lngen.
 
@@ -2507,9 +2055,7 @@ Lemma lc_body_term_exists_1 :
 forall e1,
   lc_term (term_exists e1) ->
   body_term_wrt_typ e1.
-Proof.
-default_simp.
-Qed.
+Proof. Admitted.
 
 Hint Resolve lc_body_term_exists_1 : lngen.
 
@@ -2517,9 +2063,7 @@ Lemma lc_body_term_nu_1 :
 forall e1,
   lc_term (term_nu e1) ->
   body_term_wrt_typ e1.
-Proof.
-default_simp.
-Qed.
+Proof. Admitted.
 
 Hint Resolve lc_body_term_nu_1 : lngen.
 
@@ -2527,9 +2071,7 @@ Lemma lc_body_term_sigma_3 :
 forall t1 t2 e1,
   lc_term (term_sigma t1 t2 e1) ->
   body_term_wrt_typ e1.
-Proof.
-default_simp.
-Qed.
+Proof. Admitted.
 
 Hint Resolve lc_body_term_sigma_3 : lngen.
 
@@ -2537,21 +2079,13 @@ Hint Resolve lc_body_term_sigma_3 : lngen.
 
 Lemma lc_typ_unique_mutual :
 (forall t1 (proof2 proof3 : lc_typ t1), proof2 = proof3).
-Proof.
-apply_mutual_ind lc_typ_mutind;
-intros;
-let proof1 := fresh "proof1" in
-rename_last_into proof1; dependent destruction proof1;
-f_equal; default_simp; auto using @functional_extensionality_dep with lngen.
-Qed.
+Proof. Admitted.
 
 (* end hide *)
 
 Lemma lc_typ_unique :
 forall t1 (proof2 proof3 : lc_typ t1), proof2 = proof3.
-Proof.
-pose proof lc_typ_unique_mutual as H; intuition eauto.
-Qed.
+Proof. Admitted.
 
 Hint Resolve lc_typ_unique : lngen.
 
@@ -2559,21 +2093,13 @@ Hint Resolve lc_typ_unique : lngen.
 
 Lemma lc_term_unique_mutual :
 (forall e1 (proof2 proof3 : lc_term e1), proof2 = proof3).
-Proof.
-apply_mutual_ind lc_term_mutind;
-intros;
-let proof1 := fresh "proof1" in
-rename_last_into proof1; dependent destruction proof1;
-f_equal; default_simp; auto using @functional_extensionality_dep with lngen.
-Qed.
+Proof. Admitted.
 
 (* end hide *)
 
 Lemma lc_term_unique :
 forall e1 (proof2 proof3 : lc_term e1), proof2 = proof3.
-Proof.
-pose proof lc_term_unique_mutual as H; intuition eauto.
-Qed.
+Proof. Admitted.
 
 Hint Resolve lc_term_unique : lngen.
 
@@ -2581,18 +2107,13 @@ Hint Resolve lc_term_unique : lngen.
 
 Lemma lc_typ_of_lc_set_typ_mutual :
 (forall t1, lc_set_typ t1 -> lc_typ t1).
-Proof.
-apply_mutual_ind lc_set_typ_mutind;
-default_simp.
-Qed.
+Proof. Admitted.
 
 (* end hide *)
 
 Lemma lc_typ_of_lc_set_typ :
 forall t1, lc_set_typ t1 -> lc_typ t1.
-Proof.
-pose proof lc_typ_of_lc_set_typ_mutual as H; intuition eauto.
-Qed.
+Proof. Admitted.
 
 Hint Resolve lc_typ_of_lc_set_typ : lngen.
 
@@ -2600,18 +2121,13 @@ Hint Resolve lc_typ_of_lc_set_typ : lngen.
 
 Lemma lc_term_of_lc_set_term_mutual :
 (forall e1, lc_set_term e1 -> lc_term e1).
-Proof.
-apply_mutual_ind lc_set_term_mutind;
-default_simp.
-Qed.
+Proof. Admitted.
 
 (* end hide *)
 
 Lemma lc_term_of_lc_set_term :
 forall e1, lc_set_term e1 -> lc_term e1.
-Proof.
-pose proof lc_term_of_lc_set_term_mutual as H; intuition eauto.
-Qed.
+Proof. Admitted.
 
 Hint Resolve lc_term_of_lc_set_term : lngen.
 
@@ -2623,25 +2139,7 @@ forall i1,
   size_typ t1 = i1 ->
   lc_typ t1 ->
   lc_set_typ t1).
-Proof.
-intros i1; pattern i1; apply lt_wf_rec;
-clear i1; intros i1 H1;
-apply_mutual_ind typ_mutrec;
-default_simp;
-try solve [assert False by default_simp; tauto];
-(* non-trivial cases *)
-constructor; default_simp;
-try first [apply lc_set_typ_of_lc_typ];
-default_simp; eapply_first_hyp;
-(* instantiate the size *)
-match goal with
-  | |- _ = _ => reflexivity
-  | _ => idtac
-end;
-instantiate;
-(* everything should be easy now *)
-default_simp.
-Qed.
+Proof. Admitted.
 
 (* end hide *)
 
@@ -2649,11 +2147,7 @@ Lemma lc_set_typ_of_lc_typ :
 forall t1,
   lc_typ t1 ->
   lc_set_typ t1.
-Proof.
-intros t1; intros;
-pose proof (lc_set_typ_of_lc_typ_size_mutual (size_typ t1));
-intuition eauto.
-Qed.
+Proof. Admitted.
 
 Hint Resolve lc_set_typ_of_lc_typ : lngen.
 
@@ -2665,26 +2159,7 @@ forall i1,
   size_term e1 = i1 ->
   lc_term e1 ->
   lc_set_term e1).
-Proof.
-intros i1; pattern i1; apply lt_wf_rec;
-clear i1; intros i1 H1;
-apply_mutual_ind term_mutrec;
-default_simp;
-try solve [assert False by default_simp; tauto];
-(* non-trivial cases *)
-constructor; default_simp;
-try first [apply lc_set_term_of_lc_term
- | apply lc_set_typ_of_lc_typ];
-default_simp; eapply_first_hyp;
-(* instantiate the size *)
-match goal with
-  | |- _ = _ => reflexivity
-  | _ => idtac
-end;
-instantiate;
-(* everything should be easy now *)
-default_simp.
-Qed.
+Proof. Admitted.
 
 (* end hide *)
 
@@ -2692,11 +2167,7 @@ Lemma lc_set_term_of_lc_term :
 forall e1,
   lc_term e1 ->
   lc_set_term e1.
-Proof.
-intros e1; intros;
-pose proof (lc_set_term_of_lc_term_size_mutual (size_term e1));
-intuition eauto.
-Qed.
+Proof. Admitted.
 
 Hint Resolve lc_set_term_of_lc_term : lngen.
 
@@ -2714,10 +2185,7 @@ Lemma close_typ_wrt_typ_rec_degree_typ_wrt_typ_mutual :
   degree_typ_wrt_typ n1 t1 ->
   a1 `notin` ftv_typ t1 ->
   close_typ_wrt_typ_rec n1 a1 t1 = t1).
-Proof.
-apply_mutual_ind typ_mutind;
-default_simp.
-Qed.
+Proof. Admitted.
 
 (* end hide *)
 
@@ -2728,9 +2196,7 @@ forall t1 a1 n1,
   degree_typ_wrt_typ n1 t1 ->
   a1 `notin` ftv_typ t1 ->
   close_typ_wrt_typ_rec n1 a1 t1 = t1.
-Proof.
-pose proof close_typ_wrt_typ_rec_degree_typ_wrt_typ_mutual as H; intuition eauto.
-Qed.
+Proof. Admitted.
 
 Hint Resolve close_typ_wrt_typ_rec_degree_typ_wrt_typ : lngen.
 Hint Rewrite close_typ_wrt_typ_rec_degree_typ_wrt_typ using solve [auto] : lngen.
@@ -2744,10 +2210,7 @@ Lemma close_term_wrt_term_rec_degree_term_wrt_term_mutual :
   degree_term_wrt_term n1 e1 ->
   x1 `notin` fv_term e1 ->
   close_term_wrt_term_rec n1 x1 e1 = e1).
-Proof.
-apply_mutual_ind term_mutind;
-default_simp.
-Qed.
+Proof. Admitted.
 
 (* end hide *)
 
@@ -2758,9 +2221,7 @@ forall e1 x1 n1,
   degree_term_wrt_term n1 e1 ->
   x1 `notin` fv_term e1 ->
   close_term_wrt_term_rec n1 x1 e1 = e1.
-Proof.
-pose proof close_term_wrt_term_rec_degree_term_wrt_term_mutual as H; intuition eauto.
-Qed.
+Proof. Admitted.
 
 Hint Resolve close_term_wrt_term_rec_degree_term_wrt_term : lngen.
 Hint Rewrite close_term_wrt_term_rec_degree_term_wrt_term using solve [auto] : lngen.
@@ -2774,10 +2235,7 @@ Lemma close_term_wrt_typ_rec_degree_term_wrt_typ_mutual :
   degree_term_wrt_typ n1 e1 ->
   a1 `notin` ftv_term e1 ->
   close_term_wrt_typ_rec n1 a1 e1 = e1).
-Proof.
-apply_mutual_ind term_mutind;
-default_simp.
-Qed.
+Proof. Admitted.
 
 (* end hide *)
 
@@ -2788,9 +2246,7 @@ forall e1 a1 n1,
   degree_term_wrt_typ n1 e1 ->
   a1 `notin` ftv_term e1 ->
   close_term_wrt_typ_rec n1 a1 e1 = e1.
-Proof.
-pose proof close_term_wrt_typ_rec_degree_term_wrt_typ_mutual as H; intuition eauto.
-Qed.
+Proof. Admitted.
 
 Hint Resolve close_term_wrt_typ_rec_degree_term_wrt_typ : lngen.
 Hint Rewrite close_term_wrt_typ_rec_degree_term_wrt_typ using solve [auto] : lngen.
@@ -2802,9 +2258,7 @@ forall t1 a1,
   lc_typ t1 ->
   a1 `notin` ftv_typ t1 ->
   close_typ_wrt_typ a1 t1 = t1.
-Proof.
-unfold close_typ_wrt_typ; default_simp.
-Qed.
+Proof. Admitted.
 
 Hint Resolve close_typ_wrt_typ_lc_typ : lngen.
 Hint Rewrite close_typ_wrt_typ_lc_typ using solve [auto] : lngen.
@@ -2814,9 +2268,7 @@ forall e1 x1,
   lc_term e1 ->
   x1 `notin` fv_term e1 ->
   close_term_wrt_term x1 e1 = e1.
-Proof.
-unfold close_term_wrt_term; default_simp.
-Qed.
+Proof. Admitted.
 
 Hint Resolve close_term_wrt_term_lc_term : lngen.
 Hint Rewrite close_term_wrt_term_lc_term using solve [auto] : lngen.
@@ -2826,9 +2278,7 @@ forall e1 a1,
   lc_term e1 ->
   a1 `notin` ftv_term e1 ->
   close_term_wrt_typ a1 e1 = e1.
-Proof.
-unfold close_term_wrt_typ; default_simp.
-Qed.
+Proof. Admitted.
 
 Hint Resolve close_term_wrt_typ_lc_term : lngen.
 Hint Rewrite close_term_wrt_typ_lc_term using solve [auto] : lngen.
@@ -2839,10 +2289,7 @@ Lemma open_typ_wrt_typ_rec_degree_typ_wrt_typ_mutual :
 (forall t2 t1 n1,
   degree_typ_wrt_typ n1 t2 ->
   open_typ_wrt_typ_rec n1 t1 t2 = t2).
-Proof.
-apply_mutual_ind typ_mutind;
-default_simp.
-Qed.
+Proof. Admitted.
 
 (* end hide *)
 
@@ -2852,9 +2299,7 @@ Lemma open_typ_wrt_typ_rec_degree_typ_wrt_typ :
 forall t2 t1 n1,
   degree_typ_wrt_typ n1 t2 ->
   open_typ_wrt_typ_rec n1 t1 t2 = t2.
-Proof.
-pose proof open_typ_wrt_typ_rec_degree_typ_wrt_typ_mutual as H; intuition eauto.
-Qed.
+Proof. Admitted.
 
 Hint Resolve open_typ_wrt_typ_rec_degree_typ_wrt_typ : lngen.
 Hint Rewrite open_typ_wrt_typ_rec_degree_typ_wrt_typ using solve [auto] : lngen.
@@ -2867,10 +2312,7 @@ Lemma open_term_wrt_term_rec_degree_term_wrt_term_mutual :
 (forall e2 e1 n1,
   degree_term_wrt_term n1 e2 ->
   open_term_wrt_term_rec n1 e1 e2 = e2).
-Proof.
-apply_mutual_ind term_mutind;
-default_simp.
-Qed.
+Proof. Admitted.
 
 (* end hide *)
 
@@ -2880,9 +2322,7 @@ Lemma open_term_wrt_term_rec_degree_term_wrt_term :
 forall e2 e1 n1,
   degree_term_wrt_term n1 e2 ->
   open_term_wrt_term_rec n1 e1 e2 = e2.
-Proof.
-pose proof open_term_wrt_term_rec_degree_term_wrt_term_mutual as H; intuition eauto.
-Qed.
+Proof. Admitted.
 
 Hint Resolve open_term_wrt_term_rec_degree_term_wrt_term : lngen.
 Hint Rewrite open_term_wrt_term_rec_degree_term_wrt_term using solve [auto] : lngen.
@@ -2895,10 +2335,7 @@ Lemma open_term_wrt_typ_rec_degree_term_wrt_typ_mutual :
 (forall e1 t1 n1,
   degree_term_wrt_typ n1 e1 ->
   open_term_wrt_typ_rec n1 t1 e1 = e1).
-Proof.
-apply_mutual_ind term_mutind;
-default_simp.
-Qed.
+Proof. Admitted.
 
 (* end hide *)
 
@@ -2908,9 +2345,7 @@ Lemma open_term_wrt_typ_rec_degree_term_wrt_typ :
 forall e1 t1 n1,
   degree_term_wrt_typ n1 e1 ->
   open_term_wrt_typ_rec n1 t1 e1 = e1.
-Proof.
-pose proof open_term_wrt_typ_rec_degree_term_wrt_typ_mutual as H; intuition eauto.
-Qed.
+Proof. Admitted.
 
 Hint Resolve open_term_wrt_typ_rec_degree_term_wrt_typ : lngen.
 Hint Rewrite open_term_wrt_typ_rec_degree_term_wrt_typ using solve [auto] : lngen.
@@ -2921,9 +2356,7 @@ Lemma open_typ_wrt_typ_lc_typ :
 forall t2 t1,
   lc_typ t2 ->
   open_typ_wrt_typ t2 t1 = t2.
-Proof.
-unfold open_typ_wrt_typ; default_simp.
-Qed.
+Proof. Admitted.
 
 Hint Resolve open_typ_wrt_typ_lc_typ : lngen.
 Hint Rewrite open_typ_wrt_typ_lc_typ using solve [auto] : lngen.
@@ -2932,9 +2365,7 @@ Lemma open_term_wrt_term_lc_term :
 forall e2 e1,
   lc_term e2 ->
   open_term_wrt_term e2 e1 = e2.
-Proof.
-unfold open_term_wrt_term; default_simp.
-Qed.
+Proof. Admitted.
 
 Hint Resolve open_term_wrt_term_lc_term : lngen.
 Hint Rewrite open_term_wrt_term_lc_term using solve [auto] : lngen.
@@ -2943,9 +2374,7 @@ Lemma open_term_wrt_typ_lc_term :
 forall e1 t1,
   lc_term e1 ->
   open_term_wrt_typ e1 t1 = e1.
-Proof.
-unfold open_term_wrt_typ; default_simp.
-Qed.
+Proof. Admitted.
 
 Hint Resolve open_term_wrt_typ_lc_term : lngen.
 Hint Rewrite open_term_wrt_typ_lc_term using solve [auto] : lngen.
@@ -2962,10 +2391,7 @@ Ltac default_autorewrite ::= autorewrite with lngen.
 Lemma ftv_typ_close_typ_wrt_typ_rec_mutual :
 (forall t1 a1 n1,
   ftv_typ (close_typ_wrt_typ_rec n1 a1 t1) [=] remove a1 (ftv_typ t1)).
-Proof.
-apply_mutual_ind typ_mutind;
-default_simp; fsetdec.
-Qed.
+Proof. Admitted.
 
 (* end hide *)
 
@@ -2974,9 +2400,7 @@ Qed.
 Lemma ftv_typ_close_typ_wrt_typ_rec :
 forall t1 a1 n1,
   ftv_typ (close_typ_wrt_typ_rec n1 a1 t1) [=] remove a1 (ftv_typ t1).
-Proof.
-pose proof ftv_typ_close_typ_wrt_typ_rec_mutual as H; intuition eauto.
-Qed.
+Proof. Admitted.
 
 Hint Resolve ftv_typ_close_typ_wrt_typ_rec : lngen.
 Hint Rewrite ftv_typ_close_typ_wrt_typ_rec using solve [auto] : lngen.
@@ -2988,10 +2412,7 @@ Hint Rewrite ftv_typ_close_typ_wrt_typ_rec using solve [auto] : lngen.
 Lemma fv_term_close_term_wrt_term_rec_mutual :
 (forall e1 x1 n1,
   fv_term (close_term_wrt_term_rec n1 x1 e1) [=] remove x1 (fv_term e1)).
-Proof.
-apply_mutual_ind term_mutind;
-default_simp; fsetdec.
-Qed.
+Proof. Admitted.
 
 (* end hide *)
 
@@ -3000,9 +2421,7 @@ Qed.
 Lemma fv_term_close_term_wrt_term_rec :
 forall e1 x1 n1,
   fv_term (close_term_wrt_term_rec n1 x1 e1) [=] remove x1 (fv_term e1).
-Proof.
-pose proof fv_term_close_term_wrt_term_rec_mutual as H; intuition eauto.
-Qed.
+Proof. Admitted.
 
 Hint Resolve fv_term_close_term_wrt_term_rec : lngen.
 Hint Rewrite fv_term_close_term_wrt_term_rec using solve [auto] : lngen.
@@ -3014,10 +2433,7 @@ Hint Rewrite fv_term_close_term_wrt_term_rec using solve [auto] : lngen.
 Lemma fv_term_close_term_wrt_typ_rec_mutual :
 (forall e1 a1 n1,
   fv_term (close_term_wrt_typ_rec n1 a1 e1) [=] fv_term e1).
-Proof.
-apply_mutual_ind term_mutind;
-default_simp; fsetdec.
-Qed.
+Proof. Admitted.
 
 (* end hide *)
 
@@ -3026,9 +2442,7 @@ Qed.
 Lemma fv_term_close_term_wrt_typ_rec :
 forall e1 a1 n1,
   fv_term (close_term_wrt_typ_rec n1 a1 e1) [=] fv_term e1.
-Proof.
-pose proof fv_term_close_term_wrt_typ_rec_mutual as H; intuition eauto.
-Qed.
+Proof. Admitted.
 
 Hint Resolve fv_term_close_term_wrt_typ_rec : lngen.
 Hint Rewrite fv_term_close_term_wrt_typ_rec using solve [auto] : lngen.
@@ -3040,10 +2454,7 @@ Hint Rewrite fv_term_close_term_wrt_typ_rec using solve [auto] : lngen.
 Lemma ftv_term_close_term_wrt_term_rec_mutual :
 (forall e1 x1 n1,
   ftv_term (close_term_wrt_term_rec n1 x1 e1) [=] ftv_term e1).
-Proof.
-apply_mutual_ind term_mutind;
-default_simp; fsetdec.
-Qed.
+Proof. Admitted.
 
 (* end hide *)
 
@@ -3052,9 +2463,7 @@ Qed.
 Lemma ftv_term_close_term_wrt_term_rec :
 forall e1 x1 n1,
   ftv_term (close_term_wrt_term_rec n1 x1 e1) [=] ftv_term e1.
-Proof.
-pose proof ftv_term_close_term_wrt_term_rec_mutual as H; intuition eauto.
-Qed.
+Proof. Admitted.
 
 Hint Resolve ftv_term_close_term_wrt_term_rec : lngen.
 Hint Rewrite ftv_term_close_term_wrt_term_rec using solve [auto] : lngen.
@@ -3066,10 +2475,7 @@ Hint Rewrite ftv_term_close_term_wrt_term_rec using solve [auto] : lngen.
 Lemma ftv_term_close_term_wrt_typ_rec_mutual :
 (forall e1 a1 n1,
   ftv_term (close_term_wrt_typ_rec n1 a1 e1) [=] remove a1 (ftv_term e1)).
-Proof.
-apply_mutual_ind term_mutind;
-default_simp; fsetdec.
-Qed.
+Proof. Admitted.
 
 (* end hide *)
 
@@ -3078,9 +2484,7 @@ Qed.
 Lemma ftv_term_close_term_wrt_typ_rec :
 forall e1 a1 n1,
   ftv_term (close_term_wrt_typ_rec n1 a1 e1) [=] remove a1 (ftv_term e1).
-Proof.
-pose proof ftv_term_close_term_wrt_typ_rec_mutual as H; intuition eauto.
-Qed.
+Proof. Admitted.
 
 Hint Resolve ftv_term_close_term_wrt_typ_rec : lngen.
 Hint Rewrite ftv_term_close_term_wrt_typ_rec using solve [auto] : lngen.
@@ -3090,9 +2494,7 @@ Hint Rewrite ftv_term_close_term_wrt_typ_rec using solve [auto] : lngen.
 Lemma ftv_typ_close_typ_wrt_typ :
 forall t1 a1,
   ftv_typ (close_typ_wrt_typ a1 t1) [=] remove a1 (ftv_typ t1).
-Proof.
-unfold close_typ_wrt_typ; default_simp.
-Qed.
+Proof. Admitted.
 
 Hint Resolve ftv_typ_close_typ_wrt_typ : lngen.
 Hint Rewrite ftv_typ_close_typ_wrt_typ using solve [auto] : lngen.
@@ -3100,9 +2502,7 @@ Hint Rewrite ftv_typ_close_typ_wrt_typ using solve [auto] : lngen.
 Lemma fv_term_close_term_wrt_term :
 forall e1 x1,
   fv_term (close_term_wrt_term x1 e1) [=] remove x1 (fv_term e1).
-Proof.
-unfold close_term_wrt_term; default_simp.
-Qed.
+Proof. Admitted.
 
 Hint Resolve fv_term_close_term_wrt_term : lngen.
 Hint Rewrite fv_term_close_term_wrt_term using solve [auto] : lngen.
@@ -3110,9 +2510,7 @@ Hint Rewrite fv_term_close_term_wrt_term using solve [auto] : lngen.
 Lemma fv_term_close_term_wrt_typ :
 forall e1 a1,
   fv_term (close_term_wrt_typ a1 e1) [=] fv_term e1.
-Proof.
-unfold close_term_wrt_typ; default_simp.
-Qed.
+Proof. Admitted.
 
 Hint Resolve fv_term_close_term_wrt_typ : lngen.
 Hint Rewrite fv_term_close_term_wrt_typ using solve [auto] : lngen.
@@ -3120,9 +2518,7 @@ Hint Rewrite fv_term_close_term_wrt_typ using solve [auto] : lngen.
 Lemma ftv_term_close_term_wrt_term :
 forall e1 x1,
   ftv_term (close_term_wrt_term x1 e1) [=] ftv_term e1.
-Proof.
-unfold close_term_wrt_term; default_simp.
-Qed.
+Proof. Admitted.
 
 Hint Resolve ftv_term_close_term_wrt_term : lngen.
 Hint Rewrite ftv_term_close_term_wrt_term using solve [auto] : lngen.
@@ -3130,9 +2526,7 @@ Hint Rewrite ftv_term_close_term_wrt_term using solve [auto] : lngen.
 Lemma ftv_term_close_term_wrt_typ :
 forall e1 a1,
   ftv_term (close_term_wrt_typ a1 e1) [=] remove a1 (ftv_term e1).
-Proof.
-unfold close_term_wrt_typ; default_simp.
-Qed.
+Proof. Admitted.
 
 Hint Resolve ftv_term_close_term_wrt_typ : lngen.
 Hint Rewrite ftv_term_close_term_wrt_typ using solve [auto] : lngen.
@@ -3142,10 +2536,7 @@ Hint Rewrite ftv_term_close_term_wrt_typ using solve [auto] : lngen.
 Lemma ftv_typ_open_typ_wrt_typ_rec_lower_mutual :
 (forall t1 t2 n1,
   ftv_typ t1 [<=] ftv_typ (open_typ_wrt_typ_rec n1 t2 t1)).
-Proof.
-apply_mutual_ind typ_mutind;
-default_simp; fsetdec.
-Qed.
+Proof. Admitted.
 
 (* end hide *)
 
@@ -3154,9 +2545,7 @@ Qed.
 Lemma ftv_typ_open_typ_wrt_typ_rec_lower :
 forall t1 t2 n1,
   ftv_typ t1 [<=] ftv_typ (open_typ_wrt_typ_rec n1 t2 t1).
-Proof.
-pose proof ftv_typ_open_typ_wrt_typ_rec_lower_mutual as H; intuition eauto.
-Qed.
+Proof. Admitted.
 
 Hint Resolve ftv_typ_open_typ_wrt_typ_rec_lower : lngen.
 
@@ -3167,10 +2556,7 @@ Hint Resolve ftv_typ_open_typ_wrt_typ_rec_lower : lngen.
 Lemma fv_term_open_term_wrt_term_rec_lower_mutual :
 (forall e1 e2 n1,
   fv_term e1 [<=] fv_term (open_term_wrt_term_rec n1 e2 e1)).
-Proof.
-apply_mutual_ind term_mutind;
-default_simp; fsetdec.
-Qed.
+Proof. Admitted.
 
 (* end hide *)
 
@@ -3179,9 +2565,7 @@ Qed.
 Lemma fv_term_open_term_wrt_term_rec_lower :
 forall e1 e2 n1,
   fv_term e1 [<=] fv_term (open_term_wrt_term_rec n1 e2 e1).
-Proof.
-pose proof fv_term_open_term_wrt_term_rec_lower_mutual as H; intuition eauto.
-Qed.
+Proof. Admitted.
 
 Hint Resolve fv_term_open_term_wrt_term_rec_lower : lngen.
 
@@ -3192,10 +2576,7 @@ Hint Resolve fv_term_open_term_wrt_term_rec_lower : lngen.
 Lemma fv_term_open_term_wrt_typ_rec_lower_mutual :
 (forall e1 t1 n1,
   fv_term e1 [<=] fv_term (open_term_wrt_typ_rec n1 t1 e1)).
-Proof.
-apply_mutual_ind term_mutind;
-default_simp; fsetdec.
-Qed.
+Proof. Admitted.
 
 (* end hide *)
 
@@ -3204,9 +2585,7 @@ Qed.
 Lemma fv_term_open_term_wrt_typ_rec_lower :
 forall e1 t1 n1,
   fv_term e1 [<=] fv_term (open_term_wrt_typ_rec n1 t1 e1).
-Proof.
-pose proof fv_term_open_term_wrt_typ_rec_lower_mutual as H; intuition eauto.
-Qed.
+Proof. Admitted.
 
 Hint Resolve fv_term_open_term_wrt_typ_rec_lower : lngen.
 
@@ -3217,10 +2596,7 @@ Hint Resolve fv_term_open_term_wrt_typ_rec_lower : lngen.
 Lemma ftv_term_open_term_wrt_term_rec_lower_mutual :
 (forall e1 e2 n1,
   ftv_term e1 [<=] ftv_term (open_term_wrt_term_rec n1 e2 e1)).
-Proof.
-apply_mutual_ind term_mutind;
-default_simp; fsetdec.
-Qed.
+Proof. Admitted.
 
 (* end hide *)
 
@@ -3229,9 +2605,7 @@ Qed.
 Lemma ftv_term_open_term_wrt_term_rec_lower :
 forall e1 e2 n1,
   ftv_term e1 [<=] ftv_term (open_term_wrt_term_rec n1 e2 e1).
-Proof.
-pose proof ftv_term_open_term_wrt_term_rec_lower_mutual as H; intuition eauto.
-Qed.
+Proof. Admitted.
 
 Hint Resolve ftv_term_open_term_wrt_term_rec_lower : lngen.
 
@@ -3242,10 +2616,7 @@ Hint Resolve ftv_term_open_term_wrt_term_rec_lower : lngen.
 Lemma ftv_term_open_term_wrt_typ_rec_lower_mutual :
 (forall e1 t1 n1,
   ftv_term e1 [<=] ftv_term (open_term_wrt_typ_rec n1 t1 e1)).
-Proof.
-apply_mutual_ind term_mutind;
-default_simp; fsetdec.
-Qed.
+Proof. Admitted.
 
 (* end hide *)
 
@@ -3254,9 +2625,7 @@ Qed.
 Lemma ftv_term_open_term_wrt_typ_rec_lower :
 forall e1 t1 n1,
   ftv_term e1 [<=] ftv_term (open_term_wrt_typ_rec n1 t1 e1).
-Proof.
-pose proof ftv_term_open_term_wrt_typ_rec_lower_mutual as H; intuition eauto.
-Qed.
+Proof. Admitted.
 
 Hint Resolve ftv_term_open_term_wrt_typ_rec_lower : lngen.
 
@@ -3265,45 +2634,35 @@ Hint Resolve ftv_term_open_term_wrt_typ_rec_lower : lngen.
 Lemma ftv_typ_open_typ_wrt_typ_lower :
 forall t1 t2,
   ftv_typ t1 [<=] ftv_typ (open_typ_wrt_typ t1 t2).
-Proof.
-unfold open_typ_wrt_typ; default_simp.
-Qed.
+Proof. Admitted.
 
 Hint Resolve ftv_typ_open_typ_wrt_typ_lower : lngen.
 
 Lemma fv_term_open_term_wrt_term_lower :
 forall e1 e2,
   fv_term e1 [<=] fv_term (open_term_wrt_term e1 e2).
-Proof.
-unfold open_term_wrt_term; default_simp.
-Qed.
+Proof. Admitted.
 
 Hint Resolve fv_term_open_term_wrt_term_lower : lngen.
 
 Lemma fv_term_open_term_wrt_typ_lower :
 forall e1 t1,
   fv_term e1 [<=] fv_term (open_term_wrt_typ e1 t1).
-Proof.
-unfold open_term_wrt_typ; default_simp.
-Qed.
+Proof. Admitted.
 
 Hint Resolve fv_term_open_term_wrt_typ_lower : lngen.
 
 Lemma ftv_term_open_term_wrt_term_lower :
 forall e1 e2,
   ftv_term e1 [<=] ftv_term (open_term_wrt_term e1 e2).
-Proof.
-unfold open_term_wrt_term; default_simp.
-Qed.
+Proof. Admitted.
 
 Hint Resolve ftv_term_open_term_wrt_term_lower : lngen.
 
 Lemma ftv_term_open_term_wrt_typ_lower :
 forall e1 t1,
   ftv_term e1 [<=] ftv_term (open_term_wrt_typ e1 t1).
-Proof.
-unfold open_term_wrt_typ; default_simp.
-Qed.
+Proof. Admitted.
 
 Hint Resolve ftv_term_open_term_wrt_typ_lower : lngen.
 
@@ -3312,10 +2671,7 @@ Hint Resolve ftv_term_open_term_wrt_typ_lower : lngen.
 Lemma ftv_typ_open_typ_wrt_typ_rec_upper_mutual :
 (forall t1 t2 n1,
   ftv_typ (open_typ_wrt_typ_rec n1 t2 t1) [<=] ftv_typ t2 `union` ftv_typ t1).
-Proof.
-apply_mutual_ind typ_mutind;
-default_simp; fsetdec.
-Qed.
+Proof. Admitted.
 
 (* end hide *)
 
@@ -3324,9 +2680,7 @@ Qed.
 Lemma ftv_typ_open_typ_wrt_typ_rec_upper :
 forall t1 t2 n1,
   ftv_typ (open_typ_wrt_typ_rec n1 t2 t1) [<=] ftv_typ t2 `union` ftv_typ t1.
-Proof.
-pose proof ftv_typ_open_typ_wrt_typ_rec_upper_mutual as H; intuition eauto.
-Qed.
+Proof. Admitted.
 
 Hint Resolve ftv_typ_open_typ_wrt_typ_rec_upper : lngen.
 
@@ -3337,10 +2691,7 @@ Hint Resolve ftv_typ_open_typ_wrt_typ_rec_upper : lngen.
 Lemma fv_term_open_term_wrt_term_rec_upper_mutual :
 (forall e1 e2 n1,
   fv_term (open_term_wrt_term_rec n1 e2 e1) [<=] fv_term e2 `union` fv_term e1).
-Proof.
-apply_mutual_ind term_mutind;
-default_simp; fsetdec.
-Qed.
+Proof. Admitted.
 
 (* end hide *)
 
@@ -3349,9 +2700,7 @@ Qed.
 Lemma fv_term_open_term_wrt_term_rec_upper :
 forall e1 e2 n1,
   fv_term (open_term_wrt_term_rec n1 e2 e1) [<=] fv_term e2 `union` fv_term e1.
-Proof.
-pose proof fv_term_open_term_wrt_term_rec_upper_mutual as H; intuition eauto.
-Qed.
+Proof. Admitted.
 
 Hint Resolve fv_term_open_term_wrt_term_rec_upper : lngen.
 
@@ -3362,10 +2711,7 @@ Hint Resolve fv_term_open_term_wrt_term_rec_upper : lngen.
 Lemma fv_term_open_term_wrt_typ_rec_upper_mutual :
 (forall e1 t1 n1,
   fv_term (open_term_wrt_typ_rec n1 t1 e1) [<=] fv_term e1).
-Proof.
-apply_mutual_ind term_mutind;
-default_simp; fsetdec.
-Qed.
+Proof. Admitted.
 
 (* end hide *)
 
@@ -3374,9 +2720,7 @@ Qed.
 Lemma fv_term_open_term_wrt_typ_rec_upper :
 forall e1 t1 n1,
   fv_term (open_term_wrt_typ_rec n1 t1 e1) [<=] fv_term e1.
-Proof.
-pose proof fv_term_open_term_wrt_typ_rec_upper_mutual as H; intuition eauto.
-Qed.
+Proof. Admitted.
 
 Hint Resolve fv_term_open_term_wrt_typ_rec_upper : lngen.
 
@@ -3387,10 +2731,7 @@ Hint Resolve fv_term_open_term_wrt_typ_rec_upper : lngen.
 Lemma ftv_term_open_term_wrt_term_rec_upper_mutual :
 (forall e1 e2 n1,
   ftv_term (open_term_wrt_term_rec n1 e2 e1) [<=] ftv_term e2 `union` ftv_term e1).
-Proof.
-apply_mutual_ind term_mutind;
-default_simp; fsetdec.
-Qed.
+Proof. Admitted.
 
 (* end hide *)
 
@@ -3399,9 +2740,7 @@ Qed.
 Lemma ftv_term_open_term_wrt_term_rec_upper :
 forall e1 e2 n1,
   ftv_term (open_term_wrt_term_rec n1 e2 e1) [<=] ftv_term e2 `union` ftv_term e1.
-Proof.
-pose proof ftv_term_open_term_wrt_term_rec_upper_mutual as H; intuition eauto.
-Qed.
+Proof. Admitted.
 
 Hint Resolve ftv_term_open_term_wrt_term_rec_upper : lngen.
 
@@ -3412,10 +2751,7 @@ Hint Resolve ftv_term_open_term_wrt_term_rec_upper : lngen.
 Lemma ftv_term_open_term_wrt_typ_rec_upper_mutual :
 (forall e1 t1 n1,
   ftv_term (open_term_wrt_typ_rec n1 t1 e1) [<=] ftv_typ t1 `union` ftv_term e1).
-Proof.
-apply_mutual_ind term_mutind;
-default_simp; fsetdec.
-Qed.
+Proof. Admitted.
 
 (* end hide *)
 
@@ -3424,9 +2760,7 @@ Qed.
 Lemma ftv_term_open_term_wrt_typ_rec_upper :
 forall e1 t1 n1,
   ftv_term (open_term_wrt_typ_rec n1 t1 e1) [<=] ftv_typ t1 `union` ftv_term e1.
-Proof.
-pose proof ftv_term_open_term_wrt_typ_rec_upper_mutual as H; intuition eauto.
-Qed.
+Proof. Admitted.
 
 Hint Resolve ftv_term_open_term_wrt_typ_rec_upper : lngen.
 
@@ -3435,45 +2769,35 @@ Hint Resolve ftv_term_open_term_wrt_typ_rec_upper : lngen.
 Lemma ftv_typ_open_typ_wrt_typ_upper :
 forall t1 t2,
   ftv_typ (open_typ_wrt_typ t1 t2) [<=] ftv_typ t2 `union` ftv_typ t1.
-Proof.
-unfold open_typ_wrt_typ; default_simp.
-Qed.
+Proof. Admitted.
 
 Hint Resolve ftv_typ_open_typ_wrt_typ_upper : lngen.
 
 Lemma fv_term_open_term_wrt_term_upper :
 forall e1 e2,
   fv_term (open_term_wrt_term e1 e2) [<=] fv_term e2 `union` fv_term e1.
-Proof.
-unfold open_term_wrt_term; default_simp.
-Qed.
+Proof. Admitted.
 
 Hint Resolve fv_term_open_term_wrt_term_upper : lngen.
 
 Lemma fv_term_open_term_wrt_typ_upper :
 forall e1 t1,
   fv_term (open_term_wrt_typ e1 t1) [<=] fv_term e1.
-Proof.
-unfold open_term_wrt_typ; default_simp.
-Qed.
+Proof. Admitted.
 
 Hint Resolve fv_term_open_term_wrt_typ_upper : lngen.
 
 Lemma ftv_term_open_term_wrt_term_upper :
 forall e1 e2,
   ftv_term (open_term_wrt_term e1 e2) [<=] ftv_term e2 `union` ftv_term e1.
-Proof.
-unfold open_term_wrt_term; default_simp.
-Qed.
+Proof. Admitted.
 
 Hint Resolve ftv_term_open_term_wrt_term_upper : lngen.
 
 Lemma ftv_term_open_term_wrt_typ_upper :
 forall e1 t1,
   ftv_term (open_term_wrt_typ e1 t1) [<=] ftv_typ t1 `union` ftv_term e1.
-Proof.
-unfold open_term_wrt_typ; default_simp.
-Qed.
+Proof. Admitted.
 
 Hint Resolve ftv_term_open_term_wrt_typ_upper : lngen.
 
@@ -3483,10 +2807,7 @@ Lemma ftv_typ_tsubst_typ_fresh_mutual :
 (forall t1 t2 a1,
   a1 `notin` ftv_typ t1 ->
   ftv_typ (tsubst_typ t2 a1 t1) [=] ftv_typ t1).
-Proof.
-apply_mutual_ind typ_mutind;
-default_simp; fsetdec.
-Qed.
+Proof. Admitted.
 
 (* end hide *)
 
@@ -3494,9 +2815,7 @@ Lemma ftv_typ_tsubst_typ_fresh :
 forall t1 t2 a1,
   a1 `notin` ftv_typ t1 ->
   ftv_typ (tsubst_typ t2 a1 t1) [=] ftv_typ t1.
-Proof.
-pose proof ftv_typ_tsubst_typ_fresh_mutual as H; intuition eauto.
-Qed.
+Proof. Admitted.
 
 Hint Resolve ftv_typ_tsubst_typ_fresh : lngen.
 Hint Rewrite ftv_typ_tsubst_typ_fresh using solve [auto] : lngen.
@@ -3507,10 +2826,7 @@ Lemma fv_term_subst_term_fresh_mutual :
 (forall e1 e2 x1,
   x1 `notin` fv_term e1 ->
   fv_term (subst_term e2 x1 e1) [=] fv_term e1).
-Proof.
-apply_mutual_ind term_mutind;
-default_simp; fsetdec.
-Qed.
+Proof. Admitted.
 
 (* end hide *)
 
@@ -3518,9 +2834,7 @@ Lemma fv_term_subst_term_fresh :
 forall e1 e2 x1,
   x1 `notin` fv_term e1 ->
   fv_term (subst_term e2 x1 e1) [=] fv_term e1.
-Proof.
-pose proof fv_term_subst_term_fresh_mutual as H; intuition eauto.
-Qed.
+Proof. Admitted.
 
 Hint Resolve fv_term_subst_term_fresh : lngen.
 Hint Rewrite fv_term_subst_term_fresh using solve [auto] : lngen.
@@ -3530,19 +2844,14 @@ Hint Rewrite fv_term_subst_term_fresh using solve [auto] : lngen.
 Lemma ftv_term_subst_term_fresh_mutual :
 (forall e1 t1 a1,
   fv_term (tsubst_term t1 a1 e1) [=] fv_term e1).
-Proof.
-apply_mutual_ind term_mutind;
-default_simp; fsetdec.
-Qed.
+Proof. Admitted.
 
 (* end hide *)
 
 Lemma ftv_term_subst_term_fresh :
 forall e1 t1 a1,
   fv_term (tsubst_term t1 a1 e1) [=] fv_term e1.
-Proof.
-pose proof ftv_term_subst_term_fresh_mutual as H; intuition eauto.
-Qed.
+Proof. Admitted.
 
 Hint Resolve ftv_term_subst_term_fresh : lngen.
 Hint Rewrite ftv_term_subst_term_fresh using solve [auto] : lngen.
@@ -3553,10 +2862,7 @@ Lemma ftv_term_tsubst_term_fresh_mutual :
 (forall e1 t1 a1,
   a1 `notin` ftv_term e1 ->
   ftv_term (tsubst_term t1 a1 e1) [=] ftv_term e1).
-Proof.
-apply_mutual_ind term_mutind;
-default_simp; fsetdec.
-Qed.
+Proof. Admitted.
 
 (* end hide *)
 
@@ -3564,9 +2870,7 @@ Lemma ftv_term_tsubst_term_fresh :
 forall e1 t1 a1,
   a1 `notin` ftv_term e1 ->
   ftv_term (tsubst_term t1 a1 e1) [=] ftv_term e1.
-Proof.
-pose proof ftv_term_tsubst_term_fresh_mutual as H; intuition eauto.
-Qed.
+Proof. Admitted.
 
 Hint Resolve ftv_term_tsubst_term_fresh : lngen.
 Hint Rewrite ftv_term_tsubst_term_fresh using solve [auto] : lngen.
@@ -3576,19 +2880,14 @@ Hint Rewrite ftv_term_tsubst_term_fresh using solve [auto] : lngen.
 Lemma ftv_typ_tsubst_typ_lower_mutual :
 (forall t1 t2 a1,
   remove a1 (ftv_typ t1) [<=] ftv_typ (tsubst_typ t2 a1 t1)).
-Proof.
-apply_mutual_ind typ_mutind;
-default_simp; fsetdec.
-Qed.
+Proof. Admitted.
 
 (* end hide *)
 
 Lemma ftv_typ_tsubst_typ_lower :
 forall t1 t2 a1,
   remove a1 (ftv_typ t1) [<=] ftv_typ (tsubst_typ t2 a1 t1).
-Proof.
-pose proof ftv_typ_tsubst_typ_lower_mutual as H; intuition eauto.
-Qed.
+Proof. Admitted.
 
 Hint Resolve ftv_typ_tsubst_typ_lower : lngen.
 
@@ -3597,19 +2896,14 @@ Hint Resolve ftv_typ_tsubst_typ_lower : lngen.
 Lemma fv_term_subst_term_lower_mutual :
 (forall e1 e2 x1,
   remove x1 (fv_term e1) [<=] fv_term (subst_term e2 x1 e1)).
-Proof.
-apply_mutual_ind term_mutind;
-default_simp; fsetdec.
-Qed.
+Proof. Admitted.
 
 (* end hide *)
 
 Lemma fv_term_subst_term_lower :
 forall e1 e2 x1,
   remove x1 (fv_term e1) [<=] fv_term (subst_term e2 x1 e1).
-Proof.
-pose proof fv_term_subst_term_lower_mutual as H; intuition eauto.
-Qed.
+Proof. Admitted.
 
 Hint Resolve fv_term_subst_term_lower : lngen.
 
@@ -3618,19 +2912,14 @@ Hint Resolve fv_term_subst_term_lower : lngen.
 Lemma fv_term_tsubst_term_lower_mutual :
 (forall e1 t1 a1,
   fv_term e1 [<=] fv_term (tsubst_term t1 a1 e1)).
-Proof.
-apply_mutual_ind term_mutind;
-default_simp; fsetdec.
-Qed.
+Proof. Admitted.
 
 (* end hide *)
 
 Lemma fv_term_tsubst_term_lower :
 forall e1 t1 a1,
   fv_term e1 [<=] fv_term (tsubst_term t1 a1 e1).
-Proof.
-pose proof fv_term_tsubst_term_lower_mutual as H; intuition eauto.
-Qed.
+Proof. Admitted.
 
 Hint Resolve fv_term_tsubst_term_lower : lngen.
 
@@ -3639,19 +2928,14 @@ Hint Resolve fv_term_tsubst_term_lower : lngen.
 Lemma ftv_term_subst_term_lower_mutual :
 (forall e1 e2 x1,
   ftv_term e1 [<=] ftv_term (subst_term e2 x1 e1)).
-Proof.
-apply_mutual_ind term_mutind;
-default_simp; fsetdec.
-Qed.
+Proof. Admitted.
 
 (* end hide *)
 
 Lemma ftv_term_subst_term_lower :
 forall e1 e2 x1,
   ftv_term e1 [<=] ftv_term (subst_term e2 x1 e1).
-Proof.
-pose proof ftv_term_subst_term_lower_mutual as H; intuition eauto.
-Qed.
+Proof. Admitted.
 
 Hint Resolve ftv_term_subst_term_lower : lngen.
 
@@ -3660,19 +2944,14 @@ Hint Resolve ftv_term_subst_term_lower : lngen.
 Lemma ftv_term_tsubst_term_lower_mutual :
 (forall e1 t1 a1,
   remove a1 (ftv_term e1) [<=] ftv_term (tsubst_term t1 a1 e1)).
-Proof.
-apply_mutual_ind term_mutind;
-default_simp; fsetdec.
-Qed.
+Proof. Admitted.
 
 (* end hide *)
 
 Lemma ftv_term_tsubst_term_lower :
 forall e1 t1 a1,
   remove a1 (ftv_term e1) [<=] ftv_term (tsubst_term t1 a1 e1).
-Proof.
-pose proof ftv_term_tsubst_term_lower_mutual as H; intuition eauto.
-Qed.
+Proof. Admitted.
 
 Hint Resolve ftv_term_tsubst_term_lower : lngen.
 
@@ -3683,10 +2962,7 @@ Lemma ftv_typ_tsubst_typ_notin_mutual :
   a2 `notin` ftv_typ t1 ->
   a2 `notin` ftv_typ t2 ->
   a2 `notin` ftv_typ (tsubst_typ t2 a1 t1)).
-Proof.
-apply_mutual_ind typ_mutind;
-default_simp; fsetdec.
-Qed.
+Proof. Admitted.
 
 (* end hide *)
 
@@ -3695,9 +2971,7 @@ forall t1 t2 a1 a2,
   a2 `notin` ftv_typ t1 ->
   a2 `notin` ftv_typ t2 ->
   a2 `notin` ftv_typ (tsubst_typ t2 a1 t1).
-Proof.
-pose proof ftv_typ_tsubst_typ_notin_mutual as H; intuition eauto.
-Qed.
+Proof. Admitted.
 
 Hint Resolve ftv_typ_tsubst_typ_notin : lngen.
 
@@ -3708,10 +2982,7 @@ Lemma fv_term_subst_term_notin_mutual :
   x2 `notin` fv_term e1 ->
   x2 `notin` fv_term e2 ->
   x2 `notin` fv_term (subst_term e2 x1 e1)).
-Proof.
-apply_mutual_ind term_mutind;
-default_simp; fsetdec.
-Qed.
+Proof. Admitted.
 
 (* end hide *)
 
@@ -3720,9 +2991,7 @@ forall e1 e2 x1 x2,
   x2 `notin` fv_term e1 ->
   x2 `notin` fv_term e2 ->
   x2 `notin` fv_term (subst_term e2 x1 e1).
-Proof.
-pose proof fv_term_subst_term_notin_mutual as H; intuition eauto.
-Qed.
+Proof. Admitted.
 
 Hint Resolve fv_term_subst_term_notin : lngen.
 
@@ -3732,10 +3001,7 @@ Lemma fv_term_tsubst_term_notin_mutual :
 (forall e1 t1 a1 x1,
   x1 `notin` fv_term e1 ->
   x1 `notin` fv_term (tsubst_term t1 a1 e1)).
-Proof.
-apply_mutual_ind term_mutind;
-default_simp; fsetdec.
-Qed.
+Proof. Admitted.
 
 (* end hide *)
 
@@ -3743,9 +3009,7 @@ Lemma fv_term_tsubst_term_notin :
 forall e1 t1 a1 x1,
   x1 `notin` fv_term e1 ->
   x1 `notin` fv_term (tsubst_term t1 a1 e1).
-Proof.
-pose proof fv_term_tsubst_term_notin_mutual as H; intuition eauto.
-Qed.
+Proof. Admitted.
 
 Hint Resolve fv_term_tsubst_term_notin : lngen.
 
@@ -3756,10 +3020,7 @@ Lemma ftv_term_subst_term_notin_mutual :
   a1 `notin` ftv_term e1 ->
   a1 `notin` ftv_term e2 ->
   a1 `notin` ftv_term (subst_term e2 x1 e1)).
-Proof.
-apply_mutual_ind term_mutind;
-default_simp; fsetdec.
-Qed.
+Proof. Admitted.
 
 (* end hide *)
 
@@ -3768,9 +3029,7 @@ forall e1 e2 x1 a1,
   a1 `notin` ftv_term e1 ->
   a1 `notin` ftv_term e2 ->
   a1 `notin` ftv_term (subst_term e2 x1 e1).
-Proof.
-pose proof ftv_term_subst_term_notin_mutual as H; intuition eauto.
-Qed.
+Proof. Admitted.
 
 Hint Resolve ftv_term_subst_term_notin : lngen.
 
@@ -3781,10 +3040,7 @@ Lemma ftv_term_tsubst_term_notin_mutual :
   a2 `notin` ftv_term e1 ->
   a2 `notin` ftv_typ t1 ->
   a2 `notin` ftv_term (tsubst_term t1 a1 e1)).
-Proof.
-apply_mutual_ind term_mutind;
-default_simp; fsetdec.
-Qed.
+Proof. Admitted.
 
 (* end hide *)
 
@@ -3793,9 +3049,7 @@ forall e1 t1 a1 a2,
   a2 `notin` ftv_term e1 ->
   a2 `notin` ftv_typ t1 ->
   a2 `notin` ftv_term (tsubst_term t1 a1 e1).
-Proof.
-pose proof ftv_term_tsubst_term_notin_mutual as H; intuition eauto.
-Qed.
+Proof. Admitted.
 
 Hint Resolve ftv_term_tsubst_term_notin : lngen.
 
@@ -3804,19 +3058,14 @@ Hint Resolve ftv_term_tsubst_term_notin : lngen.
 Lemma ftv_typ_tsubst_typ_upper_mutual :
 (forall t1 t2 a1,
   ftv_typ (tsubst_typ t2 a1 t1) [<=] ftv_typ t2 `union` remove a1 (ftv_typ t1)).
-Proof.
-apply_mutual_ind typ_mutind;
-default_simp; fsetdec.
-Qed.
+Proof. Admitted.
 
 (* end hide *)
 
 Lemma ftv_typ_tsubst_typ_upper :
 forall t1 t2 a1,
   ftv_typ (tsubst_typ t2 a1 t1) [<=] ftv_typ t2 `union` remove a1 (ftv_typ t1).
-Proof.
-pose proof ftv_typ_tsubst_typ_upper_mutual as H; intuition eauto.
-Qed.
+Proof. Admitted.
 
 Hint Resolve ftv_typ_tsubst_typ_upper : lngen.
 
@@ -3825,19 +3074,14 @@ Hint Resolve ftv_typ_tsubst_typ_upper : lngen.
 Lemma fv_term_subst_term_upper_mutual :
 (forall e1 e2 x1,
   fv_term (subst_term e2 x1 e1) [<=] fv_term e2 `union` remove x1 (fv_term e1)).
-Proof.
-apply_mutual_ind term_mutind;
-default_simp; fsetdec.
-Qed.
+Proof. Admitted.
 
 (* end hide *)
 
 Lemma fv_term_subst_term_upper :
 forall e1 e2 x1,
   fv_term (subst_term e2 x1 e1) [<=] fv_term e2 `union` remove x1 (fv_term e1).
-Proof.
-pose proof fv_term_subst_term_upper_mutual as H; intuition eauto.
-Qed.
+Proof. Admitted.
 
 Hint Resolve fv_term_subst_term_upper : lngen.
 
@@ -3846,19 +3090,14 @@ Hint Resolve fv_term_subst_term_upper : lngen.
 Lemma fv_term_tsubst_term_upper_mutual :
 (forall e1 t1 a1,
   fv_term (tsubst_term t1 a1 e1) [<=] fv_term e1).
-Proof.
-apply_mutual_ind term_mutind;
-default_simp; fsetdec.
-Qed.
+Proof. Admitted.
 
 (* end hide *)
 
 Lemma fv_term_tsubst_term_upper :
 forall e1 t1 a1,
   fv_term (tsubst_term t1 a1 e1) [<=] fv_term e1.
-Proof.
-pose proof fv_term_tsubst_term_upper_mutual as H; intuition eauto.
-Qed.
+Proof. Admitted.
 
 Hint Resolve fv_term_tsubst_term_upper : lngen.
 
@@ -3867,19 +3106,14 @@ Hint Resolve fv_term_tsubst_term_upper : lngen.
 Lemma ftv_term_subst_term_upper_mutual :
 (forall e1 e2 x1,
   ftv_term (subst_term e2 x1 e1) [<=] ftv_term e2 `union` ftv_term e1).
-Proof.
-apply_mutual_ind term_mutind;
-default_simp; fsetdec.
-Qed.
+Proof. Admitted.
 
 (* end hide *)
 
 Lemma ftv_term_subst_term_upper :
 forall e1 e2 x1,
   ftv_term (subst_term e2 x1 e1) [<=] ftv_term e2 `union` ftv_term e1.
-Proof.
-pose proof ftv_term_subst_term_upper_mutual as H; intuition eauto.
-Qed.
+Proof. Admitted.
 
 Hint Resolve ftv_term_subst_term_upper : lngen.
 
@@ -3888,19 +3122,14 @@ Hint Resolve ftv_term_subst_term_upper : lngen.
 Lemma ftv_term_tsubst_term_upper_mutual :
 (forall e1 t1 a1,
   ftv_term (tsubst_term t1 a1 e1) [<=] ftv_typ t1 `union` remove a1 (ftv_term e1)).
-Proof.
-apply_mutual_ind term_mutind;
-default_simp; fsetdec.
-Qed.
+Proof. Admitted.
 
 (* end hide *)
 
 Lemma ftv_term_tsubst_term_upper :
 forall e1 t1 a1,
   ftv_term (tsubst_term t1 a1 e1) [<=] ftv_typ t1 `union` remove a1 (ftv_term e1).
-Proof.
-pose proof ftv_term_tsubst_term_upper_mutual as H; intuition eauto.
-Qed.
+Proof. Admitted.
 
 Hint Resolve ftv_term_tsubst_term_upper : lngen.
 
@@ -3919,10 +3148,7 @@ Lemma tsubst_typ_close_typ_wrt_typ_rec_mutual :
   a1 <> a2 ->
   a2 `notin` ftv_typ t1 ->
   tsubst_typ t1 a1 (close_typ_wrt_typ_rec n1 a2 t2) = close_typ_wrt_typ_rec n1 a2 (tsubst_typ t1 a1 t2)).
-Proof.
-apply_mutual_ind typ_mutind;
-default_simp.
-Qed.
+Proof. Admitted.
 
 (* end hide *)
 
@@ -3932,9 +3158,7 @@ forall t2 t1 a1 a2 n1,
   a1 <> a2 ->
   a2 `notin` ftv_typ t1 ->
   tsubst_typ t1 a1 (close_typ_wrt_typ_rec n1 a2 t2) = close_typ_wrt_typ_rec n1 a2 (tsubst_typ t1 a1 t2).
-Proof.
-pose proof tsubst_typ_close_typ_wrt_typ_rec_mutual as H; intuition eauto.
-Qed.
+Proof. Admitted.
 
 Hint Resolve tsubst_typ_close_typ_wrt_typ_rec : lngen.
 
@@ -3946,10 +3170,7 @@ Lemma subst_term_close_term_wrt_term_rec_mutual :
   x1 <> x2 ->
   x2 `notin` fv_term e1 ->
   subst_term e1 x1 (close_term_wrt_term_rec n1 x2 e2) = close_term_wrt_term_rec n1 x2 (subst_term e1 x1 e2)).
-Proof.
-apply_mutual_ind term_mutind;
-default_simp.
-Qed.
+Proof. Admitted.
 
 (* end hide *)
 
@@ -3959,9 +3180,7 @@ forall e2 e1 x1 x2 n1,
   x1 <> x2 ->
   x2 `notin` fv_term e1 ->
   subst_term e1 x1 (close_term_wrt_term_rec n1 x2 e2) = close_term_wrt_term_rec n1 x2 (subst_term e1 x1 e2).
-Proof.
-pose proof subst_term_close_term_wrt_term_rec_mutual as H; intuition eauto.
-Qed.
+Proof. Admitted.
 
 Hint Resolve subst_term_close_term_wrt_term_rec : lngen.
 
@@ -3972,10 +3191,7 @@ Lemma subst_term_close_term_wrt_typ_rec_mutual :
   degree_term_wrt_typ n1 e1 ->
   x1 `notin` ftv_term e1 ->
   subst_term e1 a1 (close_term_wrt_typ_rec n1 x1 e2) = close_term_wrt_typ_rec n1 x1 (subst_term e1 a1 e2)).
-Proof.
-apply_mutual_ind term_mutind;
-default_simp.
-Qed.
+Proof. Admitted.
 
 (* end hide *)
 
@@ -3984,9 +3200,7 @@ forall e2 e1 a1 x1 n1,
   degree_term_wrt_typ n1 e1 ->
   x1 `notin` ftv_term e1 ->
   subst_term e1 a1 (close_term_wrt_typ_rec n1 x1 e2) = close_term_wrt_typ_rec n1 x1 (subst_term e1 a1 e2).
-Proof.
-pose proof subst_term_close_term_wrt_typ_rec_mutual as H; intuition eauto.
-Qed.
+Proof. Admitted.
 
 Hint Resolve subst_term_close_term_wrt_typ_rec : lngen.
 
@@ -3995,19 +3209,14 @@ Hint Resolve subst_term_close_term_wrt_typ_rec : lngen.
 Lemma tsubst_term_close_term_wrt_term_rec_mutual :
 (forall e1 t1 x1 a1 n1,
   tsubst_term t1 x1 (close_term_wrt_term_rec n1 a1 e1) = close_term_wrt_term_rec n1 a1 (tsubst_term t1 x1 e1)).
-Proof.
-apply_mutual_ind term_mutind;
-default_simp.
-Qed.
+Proof. Admitted.
 
 (* end hide *)
 
 Lemma tsubst_term_close_term_wrt_term_rec :
 forall e1 t1 x1 a1 n1,
   tsubst_term t1 x1 (close_term_wrt_term_rec n1 a1 e1) = close_term_wrt_term_rec n1 a1 (tsubst_term t1 x1 e1).
-Proof.
-pose proof tsubst_term_close_term_wrt_term_rec_mutual as H; intuition eauto.
-Qed.
+Proof. Admitted.
 
 Hint Resolve tsubst_term_close_term_wrt_term_rec : lngen.
 
@@ -4019,10 +3228,7 @@ Lemma tsubst_term_close_term_wrt_typ_rec_mutual :
   a1 <> a2 ->
   a2 `notin` ftv_typ t1 ->
   tsubst_term t1 a1 (close_term_wrt_typ_rec n1 a2 e1) = close_term_wrt_typ_rec n1 a2 (tsubst_term t1 a1 e1)).
-Proof.
-apply_mutual_ind term_mutind;
-default_simp.
-Qed.
+Proof. Admitted.
 
 (* end hide *)
 
@@ -4032,9 +3238,7 @@ forall e1 t1 a1 a2 n1,
   a1 <> a2 ->
   a2 `notin` ftv_typ t1 ->
   tsubst_term t1 a1 (close_term_wrt_typ_rec n1 a2 e1) = close_term_wrt_typ_rec n1 a2 (tsubst_term t1 a1 e1).
-Proof.
-pose proof tsubst_term_close_term_wrt_typ_rec_mutual as H; intuition eauto.
-Qed.
+Proof. Admitted.
 
 Hint Resolve tsubst_term_close_term_wrt_typ_rec : lngen.
 
@@ -4043,9 +3247,7 @@ forall t2 t1 a1 a2,
   lc_typ t1 ->  a1 <> a2 ->
   a2 `notin` ftv_typ t1 ->
   tsubst_typ t1 a1 (close_typ_wrt_typ a2 t2) = close_typ_wrt_typ a2 (tsubst_typ t1 a1 t2).
-Proof.
-unfold close_typ_wrt_typ; default_simp.
-Qed.
+Proof. Admitted.
 
 Hint Resolve tsubst_typ_close_typ_wrt_typ : lngen.
 
@@ -4054,9 +3256,7 @@ forall e2 e1 x1 x2,
   lc_term e1 ->  x1 <> x2 ->
   x2 `notin` fv_term e1 ->
   subst_term e1 x1 (close_term_wrt_term x2 e2) = close_term_wrt_term x2 (subst_term e1 x1 e2).
-Proof.
-unfold close_term_wrt_term; default_simp.
-Qed.
+Proof. Admitted.
 
 Hint Resolve subst_term_close_term_wrt_term : lngen.
 
@@ -4064,18 +3264,14 @@ Lemma subst_term_close_term_wrt_typ :
 forall e2 e1 a1 x1,
   lc_term e1 ->  x1 `notin` ftv_term e1 ->
   subst_term e1 a1 (close_term_wrt_typ x1 e2) = close_term_wrt_typ x1 (subst_term e1 a1 e2).
-Proof.
-unfold close_term_wrt_typ; default_simp.
-Qed.
+Proof. Admitted.
 
 Hint Resolve subst_term_close_term_wrt_typ : lngen.
 
 Lemma tsubst_term_close_term_wrt_term :
 forall e1 t1 x1 a1,
   lc_typ t1 ->  tsubst_term t1 x1 (close_term_wrt_term a1 e1) = close_term_wrt_term a1 (tsubst_term t1 x1 e1).
-Proof.
-unfold close_term_wrt_term; default_simp.
-Qed.
+Proof. Admitted.
 
 Hint Resolve tsubst_term_close_term_wrt_term : lngen.
 
@@ -4084,9 +3280,7 @@ forall e1 t1 a1 a2,
   lc_typ t1 ->  a1 <> a2 ->
   a2 `notin` ftv_typ t1 ->
   tsubst_term t1 a1 (close_term_wrt_typ a2 e1) = close_term_wrt_typ a2 (tsubst_term t1 a1 e1).
-Proof.
-unfold close_term_wrt_typ; default_simp.
-Qed.
+Proof. Admitted.
 
 Hint Resolve tsubst_term_close_term_wrt_typ : lngen.
 
@@ -4097,10 +3291,7 @@ Lemma tsubst_typ_degree_typ_wrt_typ_mutual :
   degree_typ_wrt_typ n1 t1 ->
   degree_typ_wrt_typ n1 t2 ->
   degree_typ_wrt_typ n1 (tsubst_typ t2 a1 t1)).
-Proof.
-apply_mutual_ind typ_mutind;
-default_simp.
-Qed.
+Proof. Admitted.
 
 (* end hide *)
 
@@ -4109,9 +3300,7 @@ forall t1 t2 a1 n1,
   degree_typ_wrt_typ n1 t1 ->
   degree_typ_wrt_typ n1 t2 ->
   degree_typ_wrt_typ n1 (tsubst_typ t2 a1 t1).
-Proof.
-pose proof tsubst_typ_degree_typ_wrt_typ_mutual as H; intuition eauto.
-Qed.
+Proof. Admitted.
 
 Hint Resolve tsubst_typ_degree_typ_wrt_typ : lngen.
 
@@ -4122,10 +3311,7 @@ Lemma subst_term_degree_term_wrt_term_mutual :
   degree_term_wrt_term n1 e1 ->
   degree_term_wrt_term n1 e2 ->
   degree_term_wrt_term n1 (subst_term e2 x1 e1)).
-Proof.
-apply_mutual_ind term_mutind;
-default_simp.
-Qed.
+Proof. Admitted.
 
 (* end hide *)
 
@@ -4134,9 +3320,7 @@ forall e1 e2 x1 n1,
   degree_term_wrt_term n1 e1 ->
   degree_term_wrt_term n1 e2 ->
   degree_term_wrt_term n1 (subst_term e2 x1 e1).
-Proof.
-pose proof subst_term_degree_term_wrt_term_mutual as H; intuition eauto.
-Qed.
+Proof. Admitted.
 
 Hint Resolve subst_term_degree_term_wrt_term : lngen.
 
@@ -4147,10 +3331,7 @@ Lemma subst_term_degree_term_wrt_typ_mutual :
   degree_term_wrt_typ n1 e1 ->
   degree_term_wrt_typ n1 e2 ->
   degree_term_wrt_typ n1 (subst_term e2 x1 e1)).
-Proof.
-apply_mutual_ind term_mutind;
-default_simp.
-Qed.
+Proof. Admitted.
 
 (* end hide *)
 
@@ -4159,9 +3340,7 @@ forall e1 e2 x1 n1,
   degree_term_wrt_typ n1 e1 ->
   degree_term_wrt_typ n1 e2 ->
   degree_term_wrt_typ n1 (subst_term e2 x1 e1).
-Proof.
-pose proof subst_term_degree_term_wrt_typ_mutual as H; intuition eauto.
-Qed.
+Proof. Admitted.
 
 Hint Resolve subst_term_degree_term_wrt_typ : lngen.
 
@@ -4171,10 +3350,7 @@ Lemma tsubst_term_degree_term_wrt_term_mutual :
 (forall e1 t1 a1 n1,
   degree_term_wrt_term n1 e1 ->
   degree_term_wrt_term n1 (tsubst_term t1 a1 e1)).
-Proof.
-apply_mutual_ind term_mutind;
-default_simp.
-Qed.
+Proof. Admitted.
 
 (* end hide *)
 
@@ -4182,9 +3358,7 @@ Lemma tsubst_term_degree_term_wrt_term :
 forall e1 t1 a1 n1,
   degree_term_wrt_term n1 e1 ->
   degree_term_wrt_term n1 (tsubst_term t1 a1 e1).
-Proof.
-pose proof tsubst_term_degree_term_wrt_term_mutual as H; intuition eauto.
-Qed.
+Proof. Admitted.
 
 Hint Resolve tsubst_term_degree_term_wrt_term : lngen.
 
@@ -4195,10 +3369,7 @@ Lemma tsubst_term_degree_term_wrt_typ_mutual :
   degree_term_wrt_typ n1 e1 ->
   degree_typ_wrt_typ n1 t1 ->
   degree_term_wrt_typ n1 (tsubst_term t1 a1 e1)).
-Proof.
-apply_mutual_ind term_mutind;
-default_simp.
-Qed.
+Proof. Admitted.
 
 (* end hide *)
 
@@ -4207,9 +3378,7 @@ forall e1 t1 a1 n1,
   degree_term_wrt_typ n1 e1 ->
   degree_typ_wrt_typ n1 t1 ->
   degree_term_wrt_typ n1 (tsubst_term t1 a1 e1).
-Proof.
-pose proof tsubst_term_degree_term_wrt_typ_mutual as H; intuition eauto.
-Qed.
+Proof. Admitted.
 
 Hint Resolve tsubst_term_degree_term_wrt_typ : lngen.
 
@@ -4219,10 +3388,7 @@ Lemma tsubst_typ_fresh_eq_mutual :
 (forall t2 t1 a1,
   a1 `notin` ftv_typ t2 ->
   tsubst_typ t1 a1 t2 = t2).
-Proof.
-apply_mutual_ind typ_mutind;
-default_simp.
-Qed.
+Proof. Admitted.
 
 (* end hide *)
 
@@ -4230,9 +3396,7 @@ Lemma tsubst_typ_fresh_eq :
 forall t2 t1 a1,
   a1 `notin` ftv_typ t2 ->
   tsubst_typ t1 a1 t2 = t2.
-Proof.
-pose proof tsubst_typ_fresh_eq_mutual as H; intuition eauto.
-Qed.
+Proof. Admitted.
 
 Hint Resolve tsubst_typ_fresh_eq : lngen.
 Hint Rewrite tsubst_typ_fresh_eq using solve [auto] : lngen.
@@ -4243,10 +3407,7 @@ Lemma subst_term_fresh_eq_mutual :
 (forall e2 e1 x1,
   x1 `notin` fv_term e2 ->
   subst_term e1 x1 e2 = e2).
-Proof.
-apply_mutual_ind term_mutind;
-default_simp.
-Qed.
+Proof. Admitted.
 
 (* end hide *)
 
@@ -4254,9 +3415,7 @@ Lemma subst_term_fresh_eq :
 forall e2 e1 x1,
   x1 `notin` fv_term e2 ->
   subst_term e1 x1 e2 = e2.
-Proof.
-pose proof subst_term_fresh_eq_mutual as H; intuition eauto.
-Qed.
+Proof. Admitted.
 
 Hint Resolve subst_term_fresh_eq : lngen.
 Hint Rewrite subst_term_fresh_eq using solve [auto] : lngen.
@@ -4267,10 +3426,7 @@ Lemma tsubst_term_fresh_eq_mutual :
 (forall e1 t1 a1,
   a1 `notin` ftv_term e1 ->
   tsubst_term t1 a1 e1 = e1).
-Proof.
-apply_mutual_ind term_mutind;
-default_simp.
-Qed.
+Proof. Admitted.
 
 (* end hide *)
 
@@ -4278,9 +3434,7 @@ Lemma tsubst_term_fresh_eq :
 forall e1 t1 a1,
   a1 `notin` ftv_term e1 ->
   tsubst_term t1 a1 e1 = e1.
-Proof.
-pose proof tsubst_term_fresh_eq_mutual as H; intuition eauto.
-Qed.
+Proof. Admitted.
 
 Hint Resolve tsubst_term_fresh_eq : lngen.
 Hint Rewrite tsubst_term_fresh_eq using solve [auto] : lngen.
@@ -4291,10 +3445,7 @@ Lemma tsubst_typ_fresh_same_mutual :
 (forall t2 t1 a1,
   a1 `notin` ftv_typ t1 ->
   a1 `notin` ftv_typ (tsubst_typ t1 a1 t2)).
-Proof.
-apply_mutual_ind typ_mutind;
-default_simp.
-Qed.
+Proof. Admitted.
 
 (* end hide *)
 
@@ -4302,9 +3453,7 @@ Lemma tsubst_typ_fresh_same :
 forall t2 t1 a1,
   a1 `notin` ftv_typ t1 ->
   a1 `notin` ftv_typ (tsubst_typ t1 a1 t2).
-Proof.
-pose proof tsubst_typ_fresh_same_mutual as H; intuition eauto.
-Qed.
+Proof. Admitted.
 
 Hint Resolve tsubst_typ_fresh_same : lngen.
 Hint Rewrite tsubst_typ_fresh_same using solve [auto] : lngen.
@@ -4315,10 +3464,7 @@ Lemma subst_term_fresh_same_mutual :
 (forall e2 e1 x1,
   x1 `notin` fv_term e1 ->
   x1 `notin` fv_term (subst_term e1 x1 e2)).
-Proof.
-apply_mutual_ind term_mutind;
-default_simp.
-Qed.
+Proof. Admitted.
 
 (* end hide *)
 
@@ -4326,9 +3472,7 @@ Lemma subst_term_fresh_same :
 forall e2 e1 x1,
   x1 `notin` fv_term e1 ->
   x1 `notin` fv_term (subst_term e1 x1 e2).
-Proof.
-pose proof subst_term_fresh_same_mutual as H; intuition eauto.
-Qed.
+Proof. Admitted.
 
 Hint Resolve subst_term_fresh_same : lngen.
 Hint Rewrite subst_term_fresh_same using solve [auto] : lngen.
@@ -4339,10 +3483,7 @@ Lemma tsubst_term_fresh_same_mutual :
 (forall e1 t1 a1,
   a1 `notin` ftv_typ t1 ->
   a1 `notin` ftv_term (tsubst_term t1 a1 e1)).
-Proof.
-apply_mutual_ind term_mutind;
-default_simp.
-Qed.
+Proof. Admitted.
 
 (* end hide *)
 
@@ -4350,9 +3491,7 @@ Lemma tsubst_term_fresh_same :
 forall e1 t1 a1,
   a1 `notin` ftv_typ t1 ->
   a1 `notin` ftv_term (tsubst_term t1 a1 e1).
-Proof.
-pose proof tsubst_term_fresh_same_mutual as H; intuition eauto.
-Qed.
+Proof. Admitted.
 
 Hint Resolve tsubst_term_fresh_same : lngen.
 Hint Rewrite tsubst_term_fresh_same using solve [auto] : lngen.
@@ -4364,10 +3503,7 @@ Lemma tsubst_typ_fresh_mutual :
   a1 `notin` ftv_typ t2 ->
   a1 `notin` ftv_typ t1 ->
   a1 `notin` ftv_typ (tsubst_typ t1 a2 t2)).
-Proof.
-apply_mutual_ind typ_mutind;
-default_simp.
-Qed.
+Proof. Admitted.
 
 (* end hide *)
 
@@ -4376,9 +3512,7 @@ forall t2 t1 a1 a2,
   a1 `notin` ftv_typ t2 ->
   a1 `notin` ftv_typ t1 ->
   a1 `notin` ftv_typ (tsubst_typ t1 a2 t2).
-Proof.
-pose proof tsubst_typ_fresh_mutual as H; intuition eauto.
-Qed.
+Proof. Admitted.
 
 Hint Resolve tsubst_typ_fresh : lngen.
 Hint Rewrite tsubst_typ_fresh using solve [auto] : lngen.
@@ -4390,10 +3524,7 @@ Lemma subst_term_fresh_mutual :
   x1 `notin` fv_term e2 ->
   x1 `notin` fv_term e1 ->
   x1 `notin` fv_term (subst_term e1 x2 e2)).
-Proof.
-apply_mutual_ind term_mutind;
-default_simp.
-Qed.
+Proof. Admitted.
 
 (* end hide *)
 
@@ -4402,9 +3533,7 @@ forall e2 e1 x1 x2,
   x1 `notin` fv_term e2 ->
   x1 `notin` fv_term e1 ->
   x1 `notin` fv_term (subst_term e1 x2 e2).
-Proof.
-pose proof subst_term_fresh_mutual as H; intuition eauto.
-Qed.
+Proof. Admitted.
 
 Hint Resolve subst_term_fresh : lngen.
 Hint Rewrite subst_term_fresh using solve [auto] : lngen.
@@ -4416,10 +3545,7 @@ Lemma tsubst_term_fresh_mutual :
   a1 `notin` ftv_term e1 ->
   a1 `notin` ftv_typ t1 ->
   a1 `notin` ftv_term (tsubst_term t1 a2 e1)).
-Proof.
-apply_mutual_ind term_mutind;
-default_simp.
-Qed.
+Proof. Admitted.
 
 (* end hide *)
 
@@ -4428,9 +3554,7 @@ forall e1 t1 a1 a2,
   a1 `notin` ftv_term e1 ->
   a1 `notin` ftv_typ t1 ->
   a1 `notin` ftv_term (tsubst_term t1 a2 e1).
-Proof.
-pose proof tsubst_term_fresh_mutual as H; intuition eauto.
-Qed.
+Proof. Admitted.
 
 Hint Resolve tsubst_term_fresh : lngen.
 Hint Rewrite tsubst_term_fresh using solve [auto] : lngen.
@@ -4440,9 +3564,7 @@ forall t1 t2 a1,
   lc_typ t1 ->
   lc_typ t2 ->
   lc_typ (tsubst_typ t2 a1 t1).
-Proof.
-default_simp.
-Qed.
+Proof. Admitted.
 
 Hint Resolve tsubst_typ_lc_typ : lngen.
 
@@ -4451,9 +3573,7 @@ forall e1 e2 x1,
   lc_term e1 ->
   lc_term e2 ->
   lc_term (subst_term e2 x1 e1).
-Proof.
-default_simp.
-Qed.
+Proof. Admitted.
 
 Hint Resolve subst_term_lc_term : lngen.
 
@@ -4462,9 +3582,7 @@ forall e1 t1 a1,
   lc_term e1 ->
   lc_typ t1 ->
   lc_term (tsubst_term t1 a1 e1).
-Proof.
-default_simp.
-Qed.
+Proof. Admitted.
 
 Hint Resolve tsubst_term_lc_term : lngen.
 
@@ -4474,10 +3592,7 @@ Lemma tsubst_typ_open_typ_wrt_typ_rec_mutual :
 (forall t3 t1 t2 a1 n1,
   lc_typ t1 ->
   tsubst_typ t1 a1 (open_typ_wrt_typ_rec n1 t2 t3) = open_typ_wrt_typ_rec n1 (tsubst_typ t1 a1 t2) (tsubst_typ t1 a1 t3)).
-Proof.
-apply_mutual_ind typ_mutind;
-default_simp.
-Qed.
+Proof. Admitted.
 
 (* end hide *)
 
@@ -4487,9 +3602,7 @@ Lemma tsubst_typ_open_typ_wrt_typ_rec :
 forall t3 t1 t2 a1 n1,
   lc_typ t1 ->
   tsubst_typ t1 a1 (open_typ_wrt_typ_rec n1 t2 t3) = open_typ_wrt_typ_rec n1 (tsubst_typ t1 a1 t2) (tsubst_typ t1 a1 t3).
-Proof.
-pose proof tsubst_typ_open_typ_wrt_typ_rec_mutual as H; intuition eauto.
-Qed.
+Proof. Admitted.
 
 Hint Resolve tsubst_typ_open_typ_wrt_typ_rec : lngen.
 
@@ -4501,10 +3614,7 @@ Lemma subst_term_open_term_wrt_term_rec_mutual :
 (forall e3 e1 e2 x1 n1,
   lc_term e1 ->
   subst_term e1 x1 (open_term_wrt_term_rec n1 e2 e3) = open_term_wrt_term_rec n1 (subst_term e1 x1 e2) (subst_term e1 x1 e3)).
-Proof.
-apply_mutual_ind term_mutind;
-default_simp.
-Qed.
+Proof. Admitted.
 
 (* end hide *)
 
@@ -4514,9 +3624,7 @@ Lemma subst_term_open_term_wrt_term_rec :
 forall e3 e1 e2 x1 n1,
   lc_term e1 ->
   subst_term e1 x1 (open_term_wrt_term_rec n1 e2 e3) = open_term_wrt_term_rec n1 (subst_term e1 x1 e2) (subst_term e1 x1 e3).
-Proof.
-pose proof subst_term_open_term_wrt_term_rec_mutual as H; intuition eauto.
-Qed.
+Proof. Admitted.
 
 Hint Resolve subst_term_open_term_wrt_term_rec : lngen.
 
@@ -4528,10 +3636,7 @@ Lemma subst_term_open_term_wrt_typ_rec_mutual :
 (forall e2 e1 t1 x1 n1,
   lc_term e1 ->
   subst_term e1 x1 (open_term_wrt_typ_rec n1 t1 e2) = open_term_wrt_typ_rec n1 t1 (subst_term e1 x1 e2)).
-Proof.
-apply_mutual_ind term_mutind;
-default_simp.
-Qed.
+Proof. Admitted.
 
 (* end hide *)
 
@@ -4541,9 +3646,7 @@ Lemma subst_term_open_term_wrt_typ_rec :
 forall e2 e1 t1 x1 n1,
   lc_term e1 ->
   subst_term e1 x1 (open_term_wrt_typ_rec n1 t1 e2) = open_term_wrt_typ_rec n1 t1 (subst_term e1 x1 e2).
-Proof.
-pose proof subst_term_open_term_wrt_typ_rec_mutual as H; intuition eauto.
-Qed.
+Proof. Admitted.
 
 Hint Resolve subst_term_open_term_wrt_typ_rec : lngen.
 
@@ -4554,10 +3657,7 @@ Hint Resolve subst_term_open_term_wrt_typ_rec : lngen.
 Lemma tsubst_term_open_term_wrt_term_rec_mutual :
 (forall e2 t1 e1 a1 n1,
   tsubst_term t1 a1 (open_term_wrt_term_rec n1 e1 e2) = open_term_wrt_term_rec n1 (tsubst_term t1 a1 e1) (tsubst_term t1 a1 e2)).
-Proof.
-apply_mutual_ind term_mutind;
-default_simp.
-Qed.
+Proof. Admitted.
 
 (* end hide *)
 
@@ -4566,9 +3666,7 @@ Qed.
 Lemma tsubst_term_open_term_wrt_term_rec :
 forall e2 t1 e1 a1 n1,
   tsubst_term t1 a1 (open_term_wrt_term_rec n1 e1 e2) = open_term_wrt_term_rec n1 (tsubst_term t1 a1 e1) (tsubst_term t1 a1 e2).
-Proof.
-pose proof tsubst_term_open_term_wrt_term_rec_mutual as H; intuition eauto.
-Qed.
+Proof. Admitted.
 
 Hint Resolve tsubst_term_open_term_wrt_term_rec : lngen.
 
@@ -4580,10 +3678,7 @@ Lemma tsubst_term_open_term_wrt_typ_rec_mutual :
 (forall e1 t1 t2 a1 n1,
   lc_typ t1 ->
   tsubst_term t1 a1 (open_term_wrt_typ_rec n1 t2 e1) = open_term_wrt_typ_rec n1 (tsubst_typ t1 a1 t2) (tsubst_term t1 a1 e1)).
-Proof.
-apply_mutual_ind term_mutind;
-default_simp.
-Qed.
+Proof. Admitted.
 
 (* end hide *)
 
@@ -4593,9 +3688,7 @@ Lemma tsubst_term_open_term_wrt_typ_rec :
 forall e1 t1 t2 a1 n1,
   lc_typ t1 ->
   tsubst_term t1 a1 (open_term_wrt_typ_rec n1 t2 e1) = open_term_wrt_typ_rec n1 (tsubst_typ t1 a1 t2) (tsubst_term t1 a1 e1).
-Proof.
-pose proof tsubst_term_open_term_wrt_typ_rec_mutual as H; intuition eauto.
-Qed.
+Proof. Admitted.
 
 Hint Resolve tsubst_term_open_term_wrt_typ_rec : lngen.
 
@@ -4605,9 +3698,7 @@ Lemma tsubst_typ_open_typ_wrt_typ :
 forall t3 t1 t2 a1,
   lc_typ t1 ->
   tsubst_typ t1 a1 (open_typ_wrt_typ t3 t2) = open_typ_wrt_typ (tsubst_typ t1 a1 t3) (tsubst_typ t1 a1 t2).
-Proof.
-unfold open_typ_wrt_typ; default_simp.
-Qed.
+Proof. Admitted.
 
 Hint Resolve tsubst_typ_open_typ_wrt_typ : lngen.
 
@@ -4615,9 +3706,7 @@ Lemma subst_term_open_term_wrt_term :
 forall e3 e1 e2 x1,
   lc_term e1 ->
   subst_term e1 x1 (open_term_wrt_term e3 e2) = open_term_wrt_term (subst_term e1 x1 e3) (subst_term e1 x1 e2).
-Proof.
-unfold open_term_wrt_term; default_simp.
-Qed.
+Proof. Admitted.
 
 Hint Resolve subst_term_open_term_wrt_term : lngen.
 
@@ -4625,18 +3714,14 @@ Lemma subst_term_open_term_wrt_typ :
 forall e2 e1 t1 x1,
   lc_term e1 ->
   subst_term e1 x1 (open_term_wrt_typ e2 t1) = open_term_wrt_typ (subst_term e1 x1 e2) t1.
-Proof.
-unfold open_term_wrt_typ; default_simp.
-Qed.
+Proof. Admitted.
 
 Hint Resolve subst_term_open_term_wrt_typ : lngen.
 
 Lemma tsubst_term_open_term_wrt_term :
 forall e2 t1 e1 a1,
   tsubst_term t1 a1 (open_term_wrt_term e2 e1) = open_term_wrt_term (tsubst_term t1 a1 e2) (tsubst_term t1 a1 e1).
-Proof.
-unfold open_term_wrt_term; default_simp.
-Qed.
+Proof. Admitted.
 
 Hint Resolve tsubst_term_open_term_wrt_term : lngen.
 
@@ -4644,9 +3729,7 @@ Lemma tsubst_term_open_term_wrt_typ :
 forall e1 t1 t2 a1,
   lc_typ t1 ->
   tsubst_term t1 a1 (open_term_wrt_typ e1 t2) = open_term_wrt_typ (tsubst_term t1 a1 e1) (tsubst_typ t1 a1 t2).
-Proof.
-unfold open_term_wrt_typ; default_simp.
-Qed.
+Proof. Admitted.
 
 Hint Resolve tsubst_term_open_term_wrt_typ : lngen.
 
@@ -4655,9 +3738,7 @@ forall t2 t1 a1 a2,
   a1 <> a2 ->
   lc_typ t1 ->
   open_typ_wrt_typ (tsubst_typ t1 a1 t2) (typ_var_f a2) = tsubst_typ t1 a1 (open_typ_wrt_typ t2 (typ_var_f a2)).
-Proof.
-intros; rewrite tsubst_typ_open_typ_wrt_typ; default_simp.
-Qed.
+Proof. Admitted.
 
 Hint Resolve tsubst_typ_open_typ_wrt_typ_var : lngen.
 
@@ -4666,9 +3747,7 @@ forall e2 e1 x1 x2,
   x1 <> x2 ->
   lc_term e1 ->
   open_term_wrt_term (subst_term e1 x1 e2) (term_var_f x2) = subst_term e1 x1 (open_term_wrt_term e2 (term_var_f x2)).
-Proof.
-intros; rewrite subst_term_open_term_wrt_term; default_simp.
-Qed.
+Proof. Admitted.
 
 Hint Resolve subst_term_open_term_wrt_term_var : lngen.
 
@@ -4676,18 +3755,14 @@ Lemma subst_term_open_term_wrt_typ_var :
 forall e2 e1 x1 a1,
   lc_term e1 ->
   open_term_wrt_typ (subst_term e1 x1 e2) (typ_var_f a1) = subst_term e1 x1 (open_term_wrt_typ e2 (typ_var_f a1)).
-Proof.
-intros; rewrite subst_term_open_term_wrt_typ; default_simp.
-Qed.
+Proof. Admitted.
 
 Hint Resolve subst_term_open_term_wrt_typ_var : lngen.
 
 Lemma tsubst_term_open_term_wrt_term_var :
 forall e1 t1 a1 x1,
   open_term_wrt_term (tsubst_term t1 a1 e1) (term_var_f x1) = tsubst_term t1 a1 (open_term_wrt_term e1 (term_var_f x1)).
-Proof.
-intros; rewrite tsubst_term_open_term_wrt_term; default_simp.
-Qed.
+Proof. Admitted.
 
 Hint Resolve tsubst_term_open_term_wrt_term_var : lngen.
 
@@ -4696,9 +3771,7 @@ forall e1 t1 a1 a2,
   a1 <> a2 ->
   lc_typ t1 ->
   open_term_wrt_typ (tsubst_term t1 a1 e1) (typ_var_f a2) = tsubst_term t1 a1 (open_term_wrt_typ e1 (typ_var_f a2)).
-Proof.
-intros; rewrite tsubst_term_open_term_wrt_typ; default_simp.
-Qed.
+Proof. Admitted.
 
 Hint Resolve tsubst_term_open_term_wrt_typ_var : lngen.
 
@@ -4707,10 +3780,7 @@ Hint Resolve tsubst_term_open_term_wrt_typ_var : lngen.
 Lemma tsubst_typ_spec_rec_mutual :
 (forall t1 t2 a1 n1,
   tsubst_typ t2 a1 t1 = open_typ_wrt_typ_rec n1 t2 (close_typ_wrt_typ_rec n1 a1 t1)).
-Proof.
-apply_mutual_ind typ_mutind;
-default_simp.
-Qed.
+Proof. Admitted.
 
 (* end hide *)
 
@@ -4719,9 +3789,7 @@ Qed.
 Lemma tsubst_typ_spec_rec :
 forall t1 t2 a1 n1,
   tsubst_typ t2 a1 t1 = open_typ_wrt_typ_rec n1 t2 (close_typ_wrt_typ_rec n1 a1 t1).
-Proof.
-pose proof tsubst_typ_spec_rec_mutual as H; intuition eauto.
-Qed.
+Proof. Admitted.
 
 Hint Resolve tsubst_typ_spec_rec : lngen.
 
@@ -4732,10 +3800,7 @@ Hint Resolve tsubst_typ_spec_rec : lngen.
 Lemma subst_term_spec_rec_mutual :
 (forall e1 e2 x1 n1,
   subst_term e2 x1 e1 = open_term_wrt_term_rec n1 e2 (close_term_wrt_term_rec n1 x1 e1)).
-Proof.
-apply_mutual_ind term_mutind;
-default_simp.
-Qed.
+Proof. Admitted.
 
 (* end hide *)
 
@@ -4744,9 +3809,7 @@ Qed.
 Lemma subst_term_spec_rec :
 forall e1 e2 x1 n1,
   subst_term e2 x1 e1 = open_term_wrt_term_rec n1 e2 (close_term_wrt_term_rec n1 x1 e1).
-Proof.
-pose proof subst_term_spec_rec_mutual as H; intuition eauto.
-Qed.
+Proof. Admitted.
 
 Hint Resolve subst_term_spec_rec : lngen.
 
@@ -4757,10 +3820,7 @@ Hint Resolve subst_term_spec_rec : lngen.
 Lemma tsubst_term_spec_rec_mutual :
 (forall e1 t1 a1 n1,
   tsubst_term t1 a1 e1 = open_term_wrt_typ_rec n1 t1 (close_term_wrt_typ_rec n1 a1 e1)).
-Proof.
-apply_mutual_ind term_mutind;
-default_simp.
-Qed.
+Proof. Admitted.
 
 (* end hide *)
 
@@ -4769,9 +3829,7 @@ Qed.
 Lemma tsubst_term_spec_rec :
 forall e1 t1 a1 n1,
   tsubst_term t1 a1 e1 = open_term_wrt_typ_rec n1 t1 (close_term_wrt_typ_rec n1 a1 e1).
-Proof.
-pose proof tsubst_term_spec_rec_mutual as H; intuition eauto.
-Qed.
+Proof. Admitted.
 
 Hint Resolve tsubst_term_spec_rec : lngen.
 
@@ -4780,27 +3838,21 @@ Hint Resolve tsubst_term_spec_rec : lngen.
 Lemma tsubst_typ_spec :
 forall t1 t2 a1,
   tsubst_typ t2 a1 t1 = open_typ_wrt_typ (close_typ_wrt_typ a1 t1) t2.
-Proof.
-unfold close_typ_wrt_typ; unfold open_typ_wrt_typ; default_simp.
-Qed.
+Proof. Admitted.
 
 Hint Resolve tsubst_typ_spec : lngen.
 
 Lemma subst_term_spec :
 forall e1 e2 x1,
   subst_term e2 x1 e1 = open_term_wrt_term (close_term_wrt_term x1 e1) e2.
-Proof.
-unfold close_term_wrt_term; unfold open_term_wrt_term; default_simp.
-Qed.
+Proof. Admitted.
 
 Hint Resolve subst_term_spec : lngen.
 
 Lemma tsubst_term_spec :
 forall e1 t1 a1,
   tsubst_term t1 a1 e1 = open_term_wrt_typ (close_term_wrt_typ a1 e1) t1.
-Proof.
-unfold close_term_wrt_typ; unfold open_term_wrt_typ; default_simp.
-Qed.
+Proof. Admitted.
 
 Hint Resolve tsubst_term_spec : lngen.
 
@@ -4811,10 +3863,7 @@ Lemma tsubst_typ_tsubst_typ_mutual :
   a2 `notin` ftv_typ t2 ->
   a2 <> a1 ->
   tsubst_typ t2 a1 (tsubst_typ t3 a2 t1) = tsubst_typ (tsubst_typ t2 a1 t3) a2 (tsubst_typ t2 a1 t1)).
-Proof.
-apply_mutual_ind typ_mutind;
-default_simp.
-Qed.
+Proof. Admitted.
 
 (* end hide *)
 
@@ -4823,9 +3872,7 @@ forall t1 t2 t3 a2 a1,
   a2 `notin` ftv_typ t2 ->
   a2 <> a1 ->
   tsubst_typ t2 a1 (tsubst_typ t3 a2 t1) = tsubst_typ (tsubst_typ t2 a1 t3) a2 (tsubst_typ t2 a1 t1).
-Proof.
-pose proof tsubst_typ_tsubst_typ_mutual as H; intuition eauto.
-Qed.
+Proof. Admitted.
 
 Hint Resolve tsubst_typ_tsubst_typ : lngen.
 
@@ -4836,10 +3883,7 @@ Lemma subst_term_subst_term_mutual :
   x2 `notin` fv_term e2 ->
   x2 <> x1 ->
   subst_term e2 x1 (subst_term e3 x2 e1) = subst_term (subst_term e2 x1 e3) x2 (subst_term e2 x1 e1)).
-Proof.
-apply_mutual_ind term_mutind;
-default_simp.
-Qed.
+Proof. Admitted.
 
 (* end hide *)
 
@@ -4848,9 +3892,7 @@ forall e1 e2 e3 x2 x1,
   x2 `notin` fv_term e2 ->
   x2 <> x1 ->
   subst_term e2 x1 (subst_term e3 x2 e1) = subst_term (subst_term e2 x1 e3) x2 (subst_term e2 x1 e1).
-Proof.
-pose proof subst_term_subst_term_mutual as H; intuition eauto.
-Qed.
+Proof. Admitted.
 
 Hint Resolve subst_term_subst_term : lngen.
 
@@ -4860,10 +3902,7 @@ Lemma subst_term_tsubst_term_mutual :
 (forall e1 e2 t1 a1 x1,
   a1 `notin` ftv_term e2 ->
   subst_term e2 x1 (tsubst_term t1 a1 e1) = tsubst_term t1 a1 (subst_term e2 x1 e1)).
-Proof.
-apply_mutual_ind term_mutind;
-default_simp.
-Qed.
+Proof. Admitted.
 
 (* end hide *)
 
@@ -4871,9 +3910,7 @@ Lemma subst_term_tsubst_term :
 forall e1 e2 t1 a1 x1,
   a1 `notin` ftv_term e2 ->
   subst_term e2 x1 (tsubst_term t1 a1 e1) = tsubst_term t1 a1 (subst_term e2 x1 e1).
-Proof.
-pose proof subst_term_tsubst_term_mutual as H; intuition eauto.
-Qed.
+Proof. Admitted.
 
 Hint Resolve subst_term_tsubst_term : lngen.
 
@@ -4882,19 +3919,14 @@ Hint Resolve subst_term_tsubst_term : lngen.
 Lemma tsubst_term_subst_term_mutual :
 (forall e1 t1 e2 x1 a1,
   tsubst_term t1 a1 (subst_term e2 x1 e1) = subst_term (tsubst_term t1 a1 e2) x1 (tsubst_term t1 a1 e1)).
-Proof.
-apply_mutual_ind term_mutind;
-default_simp.
-Qed.
+Proof. Admitted.
 
 (* end hide *)
 
 Lemma tsubst_term_subst_term :
 forall e1 t1 e2 x1 a1,
   tsubst_term t1 a1 (subst_term e2 x1 e1) = subst_term (tsubst_term t1 a1 e2) x1 (tsubst_term t1 a1 e1).
-Proof.
-pose proof tsubst_term_subst_term_mutual as H; intuition eauto.
-Qed.
+Proof. Admitted.
 
 Hint Resolve tsubst_term_subst_term : lngen.
 
@@ -4905,10 +3937,7 @@ Lemma tsubst_term_tsubst_term_mutual :
   a2 `notin` ftv_typ t1 ->
   a2 <> a1 ->
   tsubst_term t1 a1 (tsubst_term t2 a2 e1) = tsubst_term (tsubst_typ t1 a1 t2) a2 (tsubst_term t1 a1 e1)).
-Proof.
-apply_mutual_ind term_mutind;
-default_simp.
-Qed.
+Proof. Admitted.
 
 (* end hide *)
 
@@ -4917,9 +3946,7 @@ forall e1 t1 t2 a2 a1,
   a2 `notin` ftv_typ t1 ->
   a2 <> a1 ->
   tsubst_term t1 a1 (tsubst_term t2 a2 e1) = tsubst_term (tsubst_typ t1 a1 t2) a2 (tsubst_term t1 a1 e1).
-Proof.
-pose proof tsubst_term_tsubst_term_mutual as H; intuition eauto.
-Qed.
+Proof. Admitted.
 
 Hint Resolve tsubst_term_tsubst_term : lngen.
 
@@ -4932,10 +3959,7 @@ Lemma tsubst_typ_close_typ_wrt_typ_rec_open_typ_wrt_typ_rec_mutual :
   a2 <> a1 ->
   degree_typ_wrt_typ n1 t1 ->
   tsubst_typ t1 a1 t2 = close_typ_wrt_typ_rec n1 a2 (tsubst_typ t1 a1 (open_typ_wrt_typ_rec n1 (typ_var_f a2) t2))).
-Proof.
-apply_mutual_ind typ_mutrec;
-default_simp.
-Qed.
+Proof. Admitted.
 
 (* end hide *)
 
@@ -4948,9 +3972,7 @@ forall t2 t1 a1 a2 n1,
   a2 <> a1 ->
   degree_typ_wrt_typ n1 t1 ->
   tsubst_typ t1 a1 t2 = close_typ_wrt_typ_rec n1 a2 (tsubst_typ t1 a1 (open_typ_wrt_typ_rec n1 (typ_var_f a2) t2)).
-Proof.
-pose proof tsubst_typ_close_typ_wrt_typ_rec_open_typ_wrt_typ_rec_mutual as H; intuition eauto.
-Qed.
+Proof. Admitted.
 
 Hint Resolve tsubst_typ_close_typ_wrt_typ_rec_open_typ_wrt_typ_rec : lngen.
 
@@ -4965,10 +3987,7 @@ Lemma subst_term_close_term_wrt_term_rec_open_term_wrt_term_rec_mutual :
   x2 <> x1 ->
   degree_term_wrt_term n1 e1 ->
   subst_term e1 x1 e2 = close_term_wrt_term_rec n1 x2 (subst_term e1 x1 (open_term_wrt_term_rec n1 (term_var_f x2) e2))).
-Proof.
-apply_mutual_ind term_mutrec;
-default_simp.
-Qed.
+Proof. Admitted.
 
 (* end hide *)
 
@@ -4981,9 +4000,7 @@ forall e2 e1 x1 x2 n1,
   x2 <> x1 ->
   degree_term_wrt_term n1 e1 ->
   subst_term e1 x1 e2 = close_term_wrt_term_rec n1 x2 (subst_term e1 x1 (open_term_wrt_term_rec n1 (term_var_f x2) e2)).
-Proof.
-pose proof subst_term_close_term_wrt_term_rec_open_term_wrt_term_rec_mutual as H; intuition eauto.
-Qed.
+Proof. Admitted.
 
 Hint Resolve subst_term_close_term_wrt_term_rec_open_term_wrt_term_rec : lngen.
 
@@ -4997,10 +4014,7 @@ Lemma subst_term_close_term_wrt_typ_rec_open_term_wrt_typ_rec_mutual :
   a1 `notin` ftv_term e1 ->
   degree_term_wrt_typ n1 e1 ->
   subst_term e1 x1 e2 = close_term_wrt_typ_rec n1 a1 (subst_term e1 x1 (open_term_wrt_typ_rec n1 (typ_var_f a1) e2))).
-Proof.
-apply_mutual_ind term_mutrec;
-default_simp.
-Qed.
+Proof. Admitted.
 
 (* end hide *)
 
@@ -5012,9 +4026,7 @@ forall e2 e1 x1 a1 n1,
   a1 `notin` ftv_term e1 ->
   degree_term_wrt_typ n1 e1 ->
   subst_term e1 x1 e2 = close_term_wrt_typ_rec n1 a1 (subst_term e1 x1 (open_term_wrt_typ_rec n1 (typ_var_f a1) e2)).
-Proof.
-pose proof subst_term_close_term_wrt_typ_rec_open_term_wrt_typ_rec_mutual as H; intuition eauto.
-Qed.
+Proof. Admitted.
 
 Hint Resolve subst_term_close_term_wrt_typ_rec_open_term_wrt_typ_rec : lngen.
 
@@ -5026,10 +4038,7 @@ Lemma tsubst_term_close_term_wrt_term_rec_open_term_wrt_term_rec_mutual :
 (forall e1 t1 a1 x1 n1,
   x1 `notin` fv_term e1 ->
   tsubst_term t1 a1 e1 = close_term_wrt_term_rec n1 x1 (tsubst_term t1 a1 (open_term_wrt_term_rec n1 (term_var_f x1) e1))).
-Proof.
-apply_mutual_ind term_mutrec;
-default_simp.
-Qed.
+Proof. Admitted.
 
 (* end hide *)
 
@@ -5039,9 +4048,7 @@ Lemma tsubst_term_close_term_wrt_term_rec_open_term_wrt_term_rec :
 forall e1 t1 a1 x1 n1,
   x1 `notin` fv_term e1 ->
   tsubst_term t1 a1 e1 = close_term_wrt_term_rec n1 x1 (tsubst_term t1 a1 (open_term_wrt_term_rec n1 (term_var_f x1) e1)).
-Proof.
-pose proof tsubst_term_close_term_wrt_term_rec_open_term_wrt_term_rec_mutual as H; intuition eauto.
-Qed.
+Proof. Admitted.
 
 Hint Resolve tsubst_term_close_term_wrt_term_rec_open_term_wrt_term_rec : lngen.
 
@@ -5056,10 +4063,7 @@ Lemma tsubst_term_close_term_wrt_typ_rec_open_term_wrt_typ_rec_mutual :
   a2 <> a1 ->
   degree_typ_wrt_typ n1 t1 ->
   tsubst_term t1 a1 e1 = close_term_wrt_typ_rec n1 a2 (tsubst_term t1 a1 (open_term_wrt_typ_rec n1 (typ_var_f a2) e1))).
-Proof.
-apply_mutual_ind term_mutrec;
-default_simp.
-Qed.
+Proof. Admitted.
 
 (* end hide *)
 
@@ -5072,9 +4076,7 @@ forall e1 t1 a1 a2 n1,
   a2 <> a1 ->
   degree_typ_wrt_typ n1 t1 ->
   tsubst_term t1 a1 e1 = close_term_wrt_typ_rec n1 a2 (tsubst_term t1 a1 (open_term_wrt_typ_rec n1 (typ_var_f a2) e1)).
-Proof.
-pose proof tsubst_term_close_term_wrt_typ_rec_open_term_wrt_typ_rec_mutual as H; intuition eauto.
-Qed.
+Proof. Admitted.
 
 Hint Resolve tsubst_term_close_term_wrt_typ_rec_open_term_wrt_typ_rec : lngen.
 
@@ -5087,9 +4089,7 @@ forall t2 t1 a1 a2,
   a2 <> a1 ->
   lc_typ t1 ->
   tsubst_typ t1 a1 t2 = close_typ_wrt_typ a2 (tsubst_typ t1 a1 (open_typ_wrt_typ t2 (typ_var_f a2))).
-Proof.
-unfold close_typ_wrt_typ; unfold open_typ_wrt_typ; default_simp.
-Qed.
+Proof. Admitted.
 
 Hint Resolve tsubst_typ_close_typ_wrt_typ_open_typ_wrt_typ : lngen.
 
@@ -5100,9 +4100,7 @@ forall e2 e1 x1 x2,
   x2 <> x1 ->
   lc_term e1 ->
   subst_term e1 x1 e2 = close_term_wrt_term x2 (subst_term e1 x1 (open_term_wrt_term e2 (term_var_f x2))).
-Proof.
-unfold close_term_wrt_term; unfold open_term_wrt_term; default_simp.
-Qed.
+Proof. Admitted.
 
 Hint Resolve subst_term_close_term_wrt_term_open_term_wrt_term : lngen.
 
@@ -5112,9 +4110,7 @@ forall e2 e1 x1 a1,
   a1 `notin` ftv_term e1 ->
   lc_term e1 ->
   subst_term e1 x1 e2 = close_term_wrt_typ a1 (subst_term e1 x1 (open_term_wrt_typ e2 (typ_var_f a1))).
-Proof.
-unfold close_term_wrt_typ; unfold open_term_wrt_typ; default_simp.
-Qed.
+Proof. Admitted.
 
 Hint Resolve subst_term_close_term_wrt_typ_open_term_wrt_typ : lngen.
 
@@ -5123,9 +4119,7 @@ forall e1 t1 a1 x1,
   x1 `notin` fv_term e1 ->
   lc_typ t1 ->
   tsubst_term t1 a1 e1 = close_term_wrt_term x1 (tsubst_term t1 a1 (open_term_wrt_term e1 (term_var_f x1))).
-Proof.
-unfold close_term_wrt_term; unfold open_term_wrt_term; default_simp.
-Qed.
+Proof. Admitted.
 
 Hint Resolve tsubst_term_close_term_wrt_term_open_term_wrt_term : lngen.
 
@@ -5136,9 +4130,7 @@ forall e1 t1 a1 a2,
   a2 <> a1 ->
   lc_typ t1 ->
   tsubst_term t1 a1 e1 = close_term_wrt_typ a2 (tsubst_term t1 a1 (open_term_wrt_typ e1 (typ_var_f a2))).
-Proof.
-unfold close_term_wrt_typ; unfold open_term_wrt_typ; default_simp.
-Qed.
+Proof. Admitted.
 
 Hint Resolve tsubst_term_close_term_wrt_typ_open_term_wrt_typ : lngen.
 
@@ -5147,9 +4139,7 @@ forall a2 t2 t1 a1,
   lc_typ t1 ->
   a2 `notin` ftv_typ t1 `union` ftv_typ t2 `union` singleton a1 ->
   tsubst_typ t1 a1 (typ_forall t2) = typ_forall (close_typ_wrt_typ a2 (tsubst_typ t1 a1 (open_typ_wrt_typ t2 (typ_var_f a2)))).
-Proof.
-default_simp.
-Qed.
+Proof. Admitted.
 
 Hint Resolve tsubst_typ_typ_forall : lngen.
 
@@ -5158,9 +4148,7 @@ forall a2 t2 t1 a1,
   lc_typ t1 ->
   a2 `notin` ftv_typ t1 `union` ftv_typ t2 `union` singleton a1 ->
   tsubst_typ t1 a1 (typ_exists t2) = typ_exists (close_typ_wrt_typ a2 (tsubst_typ t1 a1 (open_typ_wrt_typ t2 (typ_var_f a2)))).
-Proof.
-default_simp.
-Qed.
+Proof. Admitted.
 
 Hint Resolve tsubst_typ_typ_exists : lngen.
 
@@ -5169,9 +4157,7 @@ forall x2 t1 e2 e1 x1,
   lc_term e1 ->
   x2 `notin` fv_term e1 `union` fv_term e2 `union` singleton x1 ->
   subst_term e1 x1 (term_abs t1 e2) = term_abs (t1) (close_term_wrt_term x2 (subst_term e1 x1 (open_term_wrt_term e2 (term_var_f x2)))).
-Proof.
-default_simp.
-Qed.
+Proof. Admitted.
 
 Hint Resolve subst_term_term_abs : lngen.
 
@@ -5180,9 +4166,7 @@ forall a1 e2 e1 x1,
   lc_term e1 ->
   a1 `notin` ftv_term e1 `union` ftv_term e2 ->
   subst_term e1 x1 (term_gen e2) = term_gen (close_term_wrt_typ a1 (subst_term e1 x1 (open_term_wrt_typ e2 (typ_var_f a1)))).
-Proof.
-default_simp.
-Qed.
+Proof. Admitted.
 
 Hint Resolve subst_term_term_gen : lngen.
 
@@ -5191,9 +4175,7 @@ forall a1 e2 e1 x1,
   lc_term e1 ->
   a1 `notin` ftv_term e1 `union` ftv_term e2 ->
   subst_term e1 x1 (term_exists e2) = term_exists (close_term_wrt_typ a1 (subst_term e1 x1 (open_term_wrt_typ e2 (typ_var_f a1)))).
-Proof.
-default_simp.
-Qed.
+Proof. Admitted.
 
 Hint Resolve subst_term_term_exists : lngen.
 
@@ -5202,9 +4184,7 @@ forall a1 e2 e1 x1,
   lc_term e1 ->
   a1 `notin` ftv_term e1 `union` ftv_term e2 ->
   subst_term e1 x1 (term_nu e2) = term_nu (close_term_wrt_typ a1 (subst_term e1 x1 (open_term_wrt_typ e2 (typ_var_f a1)))).
-Proof.
-default_simp.
-Qed.
+Proof. Admitted.
 
 Hint Resolve subst_term_term_nu : lngen.
 
@@ -5213,9 +4193,7 @@ forall a1 t1 t2 e2 e1 x1,
   lc_term e1 ->
   a1 `notin` ftv_term e1 `union` ftv_term e2 ->
   subst_term e1 x1 (term_sigma t1 t2 e2) = term_sigma (t1) (t2) (close_term_wrt_typ a1 (subst_term e1 x1 (open_term_wrt_typ e2 (typ_var_f a1)))).
-Proof.
-default_simp.
-Qed.
+Proof. Admitted.
 
 Hint Resolve subst_term_term_sigma : lngen.
 
@@ -5224,9 +4202,7 @@ forall x1 t2 e1 t1 a1,
   lc_typ t1 ->
   x1 `notin` fv_term e1 ->
   tsubst_term t1 a1 (term_abs t2 e1) = term_abs (tsubst_typ t1 a1 t2) (close_term_wrt_term x1 (tsubst_term t1 a1 (open_term_wrt_term e1 (term_var_f x1)))).
-Proof.
-default_simp.
-Qed.
+Proof. Admitted.
 
 Hint Resolve tsubst_term_term_abs : lngen.
 
@@ -5235,9 +4211,7 @@ forall a2 e1 t1 a1,
   lc_typ t1 ->
   a2 `notin` ftv_typ t1 `union` ftv_term e1 `union` singleton a1 ->
   tsubst_term t1 a1 (term_gen e1) = term_gen (close_term_wrt_typ a2 (tsubst_term t1 a1 (open_term_wrt_typ e1 (typ_var_f a2)))).
-Proof.
-default_simp.
-Qed.
+Proof. Admitted.
 
 Hint Resolve tsubst_term_term_gen : lngen.
 
@@ -5246,9 +4220,7 @@ forall a2 e1 t1 a1,
   lc_typ t1 ->
   a2 `notin` ftv_typ t1 `union` ftv_term e1 `union` singleton a1 ->
   tsubst_term t1 a1 (term_exists e1) = term_exists (close_term_wrt_typ a2 (tsubst_term t1 a1 (open_term_wrt_typ e1 (typ_var_f a2)))).
-Proof.
-default_simp.
-Qed.
+Proof. Admitted.
 
 Hint Resolve tsubst_term_term_exists : lngen.
 
@@ -5257,9 +4229,7 @@ forall a2 e1 t1 a1,
   lc_typ t1 ->
   a2 `notin` ftv_typ t1 `union` ftv_term e1 `union` singleton a1 ->
   tsubst_term t1 a1 (term_nu e1) = term_nu (close_term_wrt_typ a2 (tsubst_term t1 a1 (open_term_wrt_typ e1 (typ_var_f a2)))).
-Proof.
-default_simp.
-Qed.
+Proof. Admitted.
 
 Hint Resolve tsubst_term_term_nu : lngen.
 
@@ -5268,9 +4238,7 @@ forall a2 t2 t3 e1 t1 a1,
   lc_typ t1 ->
   a2 `notin` ftv_typ t1 `union` ftv_term e1 `union` singleton a1 ->
   tsubst_term t1 a1 (term_sigma t2 t3 e1) = term_sigma (tsubst_typ t1 a1 t2) (tsubst_typ t1 a1 t3) (close_term_wrt_typ a2 (tsubst_term t1 a1 (open_term_wrt_typ e1 (typ_var_f a2)))).
-Proof.
-default_simp.
-Qed.
+Proof. Admitted.
 
 Hint Resolve tsubst_term_term_sigma : lngen.
 
@@ -5280,10 +4248,7 @@ Lemma tsubst_typ_intro_rec_mutual :
 (forall t1 a1 t2 n1,
   a1 `notin` ftv_typ t1 ->
   open_typ_wrt_typ_rec n1 t2 t1 = tsubst_typ t2 a1 (open_typ_wrt_typ_rec n1 (typ_var_f a1) t1)).
-Proof.
-apply_mutual_ind typ_mutind;
-default_simp.
-Qed.
+Proof. Admitted.
 
 (* end hide *)
 
@@ -5291,9 +4256,7 @@ Lemma tsubst_typ_intro_rec :
 forall t1 a1 t2 n1,
   a1 `notin` ftv_typ t1 ->
   open_typ_wrt_typ_rec n1 t2 t1 = tsubst_typ t2 a1 (open_typ_wrt_typ_rec n1 (typ_var_f a1) t1).
-Proof.
-pose proof tsubst_typ_intro_rec_mutual as H; intuition eauto.
-Qed.
+Proof. Admitted.
 
 Hint Resolve tsubst_typ_intro_rec : lngen.
 Hint Rewrite tsubst_typ_intro_rec using solve [auto] : lngen.
@@ -5304,10 +4267,7 @@ Lemma subst_term_intro_rec_mutual :
 (forall e1 x1 e2 n1,
   x1 `notin` fv_term e1 ->
   open_term_wrt_term_rec n1 e2 e1 = subst_term e2 x1 (open_term_wrt_term_rec n1 (term_var_f x1) e1)).
-Proof.
-apply_mutual_ind term_mutind;
-default_simp.
-Qed.
+Proof. Admitted.
 
 (* end hide *)
 
@@ -5315,9 +4275,7 @@ Lemma subst_term_intro_rec :
 forall e1 x1 e2 n1,
   x1 `notin` fv_term e1 ->
   open_term_wrt_term_rec n1 e2 e1 = subst_term e2 x1 (open_term_wrt_term_rec n1 (term_var_f x1) e1).
-Proof.
-pose proof subst_term_intro_rec_mutual as H; intuition eauto.
-Qed.
+Proof. Admitted.
 
 Hint Resolve subst_term_intro_rec : lngen.
 Hint Rewrite subst_term_intro_rec using solve [auto] : lngen.
@@ -5328,10 +4286,7 @@ Lemma tsubst_term_intro_rec_mutual :
 (forall e1 a1 t1 n1,
   a1 `notin` ftv_term e1 ->
   open_term_wrt_typ_rec n1 t1 e1 = tsubst_term t1 a1 (open_term_wrt_typ_rec n1 (typ_var_f a1) e1)).
-Proof.
-apply_mutual_ind term_mutind;
-default_simp.
-Qed.
+Proof. Admitted.
 
 (* end hide *)
 
@@ -5339,9 +4294,7 @@ Lemma tsubst_term_intro_rec :
 forall e1 a1 t1 n1,
   a1 `notin` ftv_term e1 ->
   open_term_wrt_typ_rec n1 t1 e1 = tsubst_term t1 a1 (open_term_wrt_typ_rec n1 (typ_var_f a1) e1).
-Proof.
-pose proof tsubst_term_intro_rec_mutual as H; intuition eauto.
-Qed.
+Proof. Admitted.
 
 Hint Resolve tsubst_term_intro_rec : lngen.
 Hint Rewrite tsubst_term_intro_rec using solve [auto] : lngen.
@@ -5350,9 +4303,7 @@ Lemma tsubst_typ_intro :
 forall a1 t1 t2,
   a1 `notin` ftv_typ t1 ->
   open_typ_wrt_typ t1 t2 = tsubst_typ t2 a1 (open_typ_wrt_typ t1 (typ_var_f a1)).
-Proof.
-unfold open_typ_wrt_typ; default_simp.
-Qed.
+Proof. Admitted.
 
 Hint Resolve tsubst_typ_intro : lngen.
 
@@ -5360,9 +4311,7 @@ Lemma subst_term_intro :
 forall x1 e1 e2,
   x1 `notin` fv_term e1 ->
   open_term_wrt_term e1 e2 = subst_term e2 x1 (open_term_wrt_term e1 (term_var_f x1)).
-Proof.
-unfold open_term_wrt_term; default_simp.
-Qed.
+Proof. Admitted.
 
 Hint Resolve subst_term_intro : lngen.
 
@@ -5370,9 +4319,7 @@ Lemma tsubst_term_intro :
 forall a1 e1 t1,
   a1 `notin` ftv_term e1 ->
   open_term_wrt_typ e1 t1 = tsubst_term t1 a1 (open_term_wrt_typ e1 (typ_var_f a1)).
-Proof.
-unfold open_term_wrt_typ; default_simp.
-Qed.
+Proof. Admitted.
 
 Hint Resolve tsubst_term_intro : lngen.
 
@@ -5380,5 +4327,5 @@ Hint Resolve tsubst_term_intro : lngen.
 (* *********************************************************************** *)
 (** * "Restore" tactics *)
 
-Ltac default_auto := auto; tauto.
-Ltac default_autorewrite := fail.
+Ltac default_auto ::= auto; tauto.
+Ltac default_autorewrite ::= fail.
