FzipCore/FzipCore_init.v
@@ -1,0 +1,56 @@
+Add LoadPath "../metatheory".
+Require Export Relations.
+Require Export FzipCore_inf.
+Require Export Utf8.
+Require Export Coq.Program.Equality.
+
+(** Notations *)
+(*
+Notation "[ e2 / x ] e1" := (subst_term e2 x e1) (at level 67).
+Notation "[ y → x ] e" := (subst_term (term_var_f y) x e) (at level 67).
+*)
+Notation "e1 ^^ e2" := (open_term_wrt_term e1 e2) (at level 67).
+Notation "e ^ x" := (e ^^ (term_var_f x)).
+Notation "e1 '⇝' e2" := (red1 e1 e2) (at level 68).
+Notation "e1 '⇝⋆' e2" := (clos_refl_trans _ red1 e1 e2) (at level 68).
+Notation "G '⊢' t 'ok'" := (wftyp G t) (at level 67).
+Notation "G '⊢' 'ok'" := (wfenv G) (at level 67).
+Notation "G '⊢' e ':' t" := (wfterm G e t) (at level 67).
+Notation "x '∉' L" := (x `notin` L) (at level 70).
+Notation "x '∈' L" := (x `in` L) (at level 70) : set_hs_scope.
+Notation "E '∪' F" := (E `union` F) (at level 65, right associativity, format "E '∪' '/' F") : set_hs_scope.
+
+(** Tactics *)
+Tactic Notation "absurdity" "with" tactic(tac) :=
+  assert False by tac; contradiction.
+Ltac absurdity := absurdity with auto.
+Ltac size_absurd size t :=
+  assert (1 <= size t) by auto with lngen; absurdity with omega.
+Ltac size_term_absurd t := size_absurd size_term t.
+
+(** env_map *)
+Definition tag_map {A B : Set} (f : A → B) (t : @tag A) :=
+  match t with
+    | U => U
+    | E => E
+    | T a => T (f a)
+    | Eq a => Eq (f a)
+  end.
+Hint Unfold tag_map.
+
+Definition env_map {A : Set} (f : typ → A) (env : typing_env) :=
+  map (tag_map f) env.
+Hint Unfold env_map.
+
+(** Additional lemmas *)
+Lemma var_subst : forall e x, subst_term e x (term_var_f x) = e.
+Proof.
+intros e x; simpl; destruct (x == x); congruence.
+Qed.
+Hint Rewrite var_subst : lngen.
+
+Lemma tvar_tsubst : forall t a, tsubst_typ t a (typ_var_f a) = t.
+Proof.
+intros t a; simpl; destruct (a == a); congruence.
+Qed.
+Hint Rewrite tvar_tsubst : lngen.
