FzipCore/FzipCore_soundness.v
@@ -1,0 +1,1004 @@
+Add LoadPath "../metatheory".
+Require Export FzipCore_init.
+
+Ltac gather_atoms ::=
+  let A := gather_atoms_with (fun x : vars => x) in
+  let B := gather_atoms_with (fun x : var => {{ x }}) in
+  let C := gather_atoms_with (fun x : typing_env => dom x) in
+  let D1 := gather_atoms_with (fun x => fv_term x) in
+  let D2 := gather_atoms_with (fun x => ftv_typ x) in
+  let D3 := gather_atoms_with (fun x => ftv_term x) in
+  constr:(A \u B \u C \u D1 \u D2 \u D3).
+
+(** Mutual induction principles *)
+Scheme val_mut_ind_aux  := Induction for val  Sort Prop
+with   result_mut_ind_aux := Induction for result Sort Prop.
+Combined Scheme val_result_mut_ind from val_mut_ind_aux, result_mut_ind_aux.
+
+Scheme wfenv_mut_ind_aux := Induction for wfenv Sort Prop
+with   wftyp_mut_ind_aux := Induction for wftyp Sort Prop.
+Combined Scheme wfenv_wftyp_mut_ind from
+  wfenv_mut_ind_aux, wftyp_mut_ind_aux.
+
+(** Administrative lemmas *)
+Lemma val_result_regular :
+  (forall v, val v → lc_term v)
+  ∧ (forall p, result p → lc_term p).
+Proof.
+apply val_result_mut_ind; eauto.
+Case "val_exists".
+  intros; subst.
+  pick fresh b; pick fresh a.
+  apply (lc_term_exists_exists b).
+  unfold open_term_wrt_typ; simpl.
+  apply (lc_term_sigma_exists a); auto.
+    apply l; auto.
+  eapply (H b a); auto; reflexivity.
+Qed.
+
+Lemma val_regular : forall v, val v → lc_term v.
+Proof.
+intros; destruct val_result_regular as [H1 _]; auto.
+Qed.
+
+Lemma result_regular : forall p, result p → lc_term p.
+Proof.
+intros; destruct val_result_regular as [_ H2]; auto.
+Qed.
+Hint Resolve val_regular result_regular.
+
+Lemma red0_regular1 : forall e e', red0 e e' → lc_term e.
+Proof.
+intros e e' H. destruct H; auto.
+Case "nu_sigma".
+  pick fresh b; pick fresh a.
+  apply (lc_term_nu_exists b).
+  unfold open_term_wrt_typ; simpl.
+  apply (lc_term_sigma_exists a); auto.
+  apply H; auto.
+  apply result_regular.
+  eapply (H2 b a); auto; reflexivity.
+Qed.
+
+Lemma red0_regular2 : forall e e', red0 e e' → lc_term e'.
+Proof.
+intros e e' H; destruct H;
+try solve [apply val_regular in H; inversion H; subst; auto];
+auto with lngen.
+Case "beta_v". eauto with lngen.
+Case "beta_t".
+  pick fresh a.
+  assert (lc_term (open_term_wrt_typ e (typ_var_f a))) by auto.
+  apply tsubst_term_lc_term
+    with (t1 := typ_var_f b) (a1 := a) in H0; auto.
+  rewrite tsubst_term_open_term_wrt_typ in H0; auto.
+  autorewrite with lngen in H0; auto.
+Case "nu_sigma".
+  pick fresh b; pick fresh a.
+  erewrite (H3 b a); auto.
+  apply tsubst_term_lc_term; auto.
+  apply result_regular.
+  eapply (H2 b a); auto;
+  unfold open_term_wrt_typ; simpl; reflexivity.
+  reflexivity.
+Case "coerce_coerce".
+  inversion H0; subst; try congruence; auto with lngen.
+Case "sigma_appL".
+  pick fresh a.
+  apply (lc_term_sigma_exists a); auto.
+  apply result_regular in H; inversion H; subst; auto.
+  unfold open_term_wrt_typ; simpl.
+  constructor.
+    apply result_regular in H; inversion H; subst. apply H7.
+    rewrite <- (H1 a) in H0; auto.
+Case "sigma_appR".
+  pick fresh a.
+  apply (lc_term_sigma_exists a); auto.
+  apply result_regular in H0; inversion H0; subst; auto.
+  unfold open_term_wrt_typ; simpl.
+  constructor.
+    rewrite <- (H1 a) in H; auto.
+    apply result_regular in H0; inversion H0; subst. apply H7.
+Case "sigma_pairL".
+  pick fresh a.
+  apply (lc_term_sigma_exists a); auto.
+  apply result_regular in H; inversion H; subst; auto.
+  unfold open_term_wrt_typ; simpl.
+  constructor.
+    apply result_regular in H; inversion H; subst. apply H7.
+    rewrite <- (H1 a) in H0; auto.
+Case "sigma_pairR".
+  pick fresh a.
+  apply (lc_term_sigma_exists a); auto.
+  apply result_regular in H0; inversion H0; subst; auto.
+  unfold open_term_wrt_typ; simpl.
+  constructor.
+    rewrite <- (H1 a) in H; auto.
+    apply result_regular in H0; inversion H0; subst. apply H7.
+Case "sigma_fst".
+  pick fresh a.
+  apply result_regular in H; inversion H; subst.
+  apply (lc_term_sigma_exists a); auto.
+  unfold open_term_wrt_typ; simpl.
+  constructor; apply H5.
+Case "sigma_snd".
+  pick fresh a.
+  apply result_regular in H; inversion H; subst.
+  apply (lc_term_sigma_exists a); auto.
+  unfold open_term_wrt_typ; simpl.
+  constructor; apply H5.
+Case "Sigma_inst".
+  pick fresh a.
+  apply result_regular in H0; inversion H0; subst.
+  apply (lc_term_sigma_exists a); auto.
+  unfold open_term_wrt_typ; simpl.
+  constructor.
+    apply H7.
+    rewrite <- (H1 a) in H; auto.
+Case "sigma_open".
+  pick fresh a.
+  apply result_regular in H; inversion H; subst.
+  apply (lc_term_sigma_exists a); auto.
+  unfold open_term_wrt_typ; simpl.
+  constructor; auto. apply H5.
+Case "sigma_sigma".
+  pick fresh a2; pick fresh a1.
+  apply result_regular in H; inversion H; subst.
+  apply (lc_term_sigma_exists a2); auto.
+  rewrite (H3 a2); auto.
+    assert
+      (lc_term
+        (open_term_wrt_typ
+          (term_sigma (typ_var_f b2) t2 e)
+          (typ_var_f a2))) as H11 by auto;
+      inversion H11; subst; auto.
+  unfold open_term_wrt_typ; simpl.
+  apply (lc_term_sigma_exists a1); auto.
+  rewrite (H2 a2) in H9; auto.
+  assert (open_term_wrt_typ_rec 1 (typ_var_f a2) e'
+  = open_term_wrt_typ_rec 1 (typ_var_f a1) e) as Heq.
+    apply (H4 a1 a2); auto.
+    unfold open_term_wrt_typ; simpl; rewrite (H3 a1); auto.
+    unfold open_term_wrt_typ; simpl; rewrite (H2 a2); auto.
+  rewrite Heq; clear Heq.
+  assert
+    (lc_term (open_term_wrt_typ (term_sigma (typ_var_f b2) t2 e) (typ_var_f a1))) as H11 by auto.
+  unfold open_term_wrt_typ in H11; simpl in H11; inversion H11; subst.
+  auto.
+Qed.
+Hint Resolve red0_regular1 red0_regular2.
+
+Lemma red1_regular1 : forall e e', e ⇝ e' → lc_term e.
+Proof.
+intros e e' H. induction H; eauto.
+Qed.
+
+Lemma red1_regular2 : forall e e', e ⇝ e' → lc_term e'.
+Proof.
+intros e e' H; induction H; eauto.
+Qed.
+Hint Resolve red1_regular1 red1_regular2.
+
+Lemma wftyp_regular : forall Γ τ, wftyp Γ τ → lc_typ τ.
+Proof.
+intros Γ τ H.
+induction H; eauto.
+Qed.
+Hint Resolve wftyp_regular.
+
+Lemma wfenv_wftyp_aux :
+  (forall Γ, wfenv Γ → forall Γ₁ x b τ, Γ = x ~ b ++ Γ₁ ->
+    (b = T τ ∨ b = Eq τ) → wftyp Γ₁ τ) ∧
+  (forall Γ τ, wftyp Γ τ → wfenv Γ).
+Proof.
+apply wfenv_wftyp_mut_ind; intros; eauto.
+inversion H.
+inversion H0; destruct H1; congruence.
+inversion H0; destruct H1; congruence.
+inversion H0; destruct H1; congruence.
+inversion H0; destruct H1; congruence.
+pick fresh a; assert (a ~ U ++ G ⊢ ok) by auto; inversion H0; subst; auto.
+pick fresh a; assert (a ~ U ++ G ⊢ ok) by auto; inversion H0; subst; auto.
+Qed.
+
+Lemma wfenv_wftyp_T :
+forall Γ₁ Γ₂ x τ, wfenv (Γ₁ ++ x ~ T τ ++ Γ₂) → wftyp Γ₂ τ.
+Proof.
+destruct wfenv_wftyp_aux as [H1 H2].
+intros Γ₁ Γ₂ x τ H0.
+generalize dependent Γ₂.
+induction Γ₁; intros; simpl_env in H0; eauto.
+inversion H0; subst; simpl_env in H5; eauto.
+Qed.
+
+Lemma wfenv_wftyp_Eq :
+forall Γ₁ Γ₂ x τ, wfenv (Γ₁ ++ x ~ Eq τ ++ Γ₂) → wftyp Γ₂ τ.
+Proof.
+destruct wfenv_wftyp_aux as [H1 H2].
+intros Γ₁ Γ₂ x τ H0.
+generalize dependent Γ₂.
+induction Γ₁; intros; simpl_env in H0; eauto.
+inversion H0; subst; simpl_env in H5; eauto.
+Qed.
+Hint Resolve wfenv_wftyp_T wfenv_wftyp_Eq.
+
+
+Lemma wftyp_wfenv : forall Γ τ, wftyp Γ τ → wfenv Γ.
+Proof.
+destruct wfenv_wftyp_aux; auto.
+Qed.
+Hint Resolve wftyp_wfenv.
+
+Lemma wfenv_wftyp_uniq_aux :
+  (forall Γ, wfenv Γ → uniq Γ) ∧ (forall Γ τ, wftyp Γ τ → uniq Γ).
+Proof.
+apply wfenv_wftyp_mut_ind; intros; auto.
+pick fresh a. assert (uniq (a ~ U ++ G)) by auto. destruct_uniq; auto.
+pick fresh a. assert (uniq (a ~ U ++ G)) by auto. destruct_uniq; auto.
+Qed.
+
+Lemma wfenv_uniq : forall Γ, wfenv Γ → uniq Γ.
+Proof.
+destruct wfenv_wftyp_uniq_aux; auto.
+Qed.
+Hint Resolve wfenv_uniq.
+
+Lemma wftyp_uniq :  forall Γ τ, wftyp Γ τ → uniq Γ.
+Proof.
+eauto.
+Qed.
+Hint Resolve wftyp_uniq.
+
+(** Lemmas about [wfenv] and [wftyp] *)
+Lemma wfenv_wftyp_weakening :
+(forall Γ, wfenv Γ → forall Γ₁ Γ₂ Γ₃, Γ = Γ₁ ++ Γ₃ → wfenv (Γ₂ ++ Γ₃) → disjoint Γ₁ Γ₂ → wfenv (Γ₁ ++ Γ₂ ++ Γ₃))
+∧
+(forall Γ τ, wftyp Γ τ → forall Γ₁ Γ₂ Γ₃, Γ = Γ₁ ++ Γ₃ → wfenv (Γ₂ ++ Γ₃) → disjoint Γ₁ Γ₂ → wftyp (Γ₁ ++ Γ₂ ++ Γ₃) τ).
+Proof.
+apply wfenv_wftyp_mut_ind; intros; auto.
+Case "wfenv_empty".
+destruct Γ₁. destruct Γ₃. simpl_env in *; auto.
+simpl in H; inversion H.
+simpl in H; inversion H.
+Case "wfenv_cons_T".
+destruct Γ₁; simpl_env in *.
+destruct Γ₃; simpl_env in *; auto.
+inversion H0; subst.
+apply wfenv_cons_T.
+simpl in H2; apply disjoint_cons_1 in H2; auto.
+apply H; auto.
+simpl in H2; apply disjoint_cons_2 in H2; auto.
+Case "wfenv_cons_U".
+destruct Γ₁; simpl_env in *.
+destruct Γ₃; simpl_env in *; auto.
+inversion H0; subst.
+apply wfenv_cons_U.
+simpl in H2; apply disjoint_cons_1 in H2; auto.
+apply H; auto.
+simpl in H2; apply disjoint_cons_2 in H2; auto.
+Case "wfenv_cons_E".
+destruct Γ₁; simpl_env in *.
+destruct Γ₃; simpl_env in *; auto.
+inversion H0; subst.
+apply wfenv_cons_E.
+simpl in H2; apply disjoint_cons_1 in H2; auto.
+apply H; auto.
+simpl in H2; apply disjoint_cons_2 in H2; auto.
+Case "wfenv_cons_Eq".
+destruct Γ₁; simpl_env in *.
+destruct Γ₃; simpl_env in *; auto.
+inversion H0; subst.
+apply wfenv_cons_Eq.
+simpl in H2; apply disjoint_cons_1 in H2; auto.
+apply H; auto.
+simpl in H2; apply disjoint_cons_2 in H2; auto.
+Case "wftyp_var".
+subst G.
+  destruct o. auto.
+  destruct H0. auto.
+  destruct H0. apply wftyp_var; auto; right; right; eauto.
+Case "wftyp_forall".
+subst G; apply wftyp_forall with (L := L ∪ dom Γ₂); intros.
+rewrite_env ((a~U ++ Γ₁) ++ Γ₂ ++ Γ₃); apply H; eauto.
+Case "wftyp_exists".
+subst G; apply wftyp_exists with (L := L ∪ dom Γ₂); intros.
+rewrite_env ((a~U ++ Γ₁) ++ Γ₂ ++ Γ₃); apply H; eauto.
+Qed.
+
+Lemma wfenv_weakening :
+forall Γ₁ Γ₂ Γ₃, wfenv (Γ₁ ++ Γ₃) → wfenv (Γ₂ ++ Γ₃) → disjoint Γ₁ Γ₂ → wfenv (Γ₁ ++ Γ₂ ++ Γ₃).
+Proof.
+destruct wfenv_wftyp_weakening as [H1 H2].
+intros; apply (H1 (Γ₁ ++ Γ₃)); auto.
+Qed.
+
+Lemma wftyp_weakening :
+forall Γ₁ Γ₂ Γ₃ τ, wftyp (Γ₁ ++ Γ₃) τ → wfenv (Γ₂ ++ Γ₃) → disjoint Γ₁ Γ₂ → wftyp (Γ₁ ++ Γ₂ ++ Γ₃) τ.
+Proof.
+destruct wfenv_wftyp_weakening as [H1 H2].
+intros. apply (H2 (Γ₁ ++ Γ₃)); auto.
+Qed.
+
+Lemma wfenv_wftyp_T2 :
+forall Γ x τ, wfenv Γ → binds x (T τ) Γ → wftyp Γ τ.
+Proof.
+intro Γ; induction Γ; intros.
+analyze_binds H0.
+destruct a; destruct t; simpl_env in *; analyze_binds H0.
+Case "T =".
+replace t with τ in * by congruence.
+rewrite_env (nil ++ a ~ T τ ++ Γ).
+inversion H; subst.
+apply wftyp_weakening; auto.
+Case "T ≠".
+rewrite_env (nil ++ a ~ T t ++ Γ).
+apply wftyp_weakening; auto. simpl.
+inversion H; subst. eapply IHΓ; eauto.
+Case "U".
+rewrite_env (nil ++ a ~ U ++ Γ).
+apply wftyp_weakening; auto.
+inversion H; subst. eapply IHΓ; eauto.
+Case "E".
+rewrite_env (nil ++ a ~ E ++ Γ).
+apply wftyp_weakening; auto.
+inversion H; subst. eapply IHΓ; eauto.
+Case "Eq".
+rewrite_env (nil ++ a ~ Eq t ++ Γ).
+apply wftyp_weakening; auto. simpl.
+inversion H; subst. eapply IHΓ; eauto.
+Qed.
+
+Lemma wfenv_wftyp_Eq2 :
+forall Γ x τ, wfenv Γ → binds x (Eq τ) Γ → wftyp Γ τ.
+Proof.
+intro Γ; induction Γ; intros.
+analyze_binds H0.
+destruct a; destruct t; simpl_env in *; analyze_binds H0.
+Case "T".
+rewrite_env (nil ++ a ~ T t ++ Γ).
+apply wftyp_weakening; auto. simpl.
+inversion H; subst. eapply IHΓ; eauto.
+Case "U".
+rewrite_env (nil ++ a ~ U ++ Γ).
+apply wftyp_weakening; auto.
+inversion H; subst. eapply IHΓ; eauto.
+Case "E".
+rewrite_env (nil ++ a ~ E ++ Γ).
+apply wftyp_weakening; auto.
+inversion H; subst. eapply IHΓ; eauto.
+Case "Eq =".
+replace t with τ in * by congruence.
+rewrite_env (nil ++ a ~ Eq τ ++ Γ).
+inversion H; subst.
+apply wftyp_weakening; auto.
+Case "Eq ≠".
+rewrite_env (nil ++ a ~ Eq t ++ Γ).
+apply wftyp_weakening; auto. simpl.
+inversion H; subst. eapply IHΓ; eauto.
+Qed.
+Hint Resolve wfenv_wftyp_T2 wfenv_wftyp_Eq2.
+
+Lemma wfenv_wftyp_T3 :
+forall Γ x τ, wfenv (x ~ T τ ++ Γ) → wftyp Γ τ.
+Proof.
+intros Γ x τ H; inversion H; subst; auto.
+Qed.
+
+Lemma wfenv_wftyp_Eq3 :
+forall Γ x τ, wfenv (x ~ Eq τ ++ Γ) → wftyp Γ τ.
+Proof.
+intros Γ x τ H; inversion H; subst; auto.
+Qed.
+Hint Resolve wfenv_wftyp_T3 wfenv_wftyp_Eq3.
+
+Lemma wfenv_regular_T :
+forall Γ x τ, wfenv Γ → binds x (T τ) Γ → lc_typ τ.
+Proof.
+intros. induction H; analyze_binds H0.
+replace t with τ in * by congruence; eauto.
+eauto.
+eauto.
+Qed.
+
+Lemma wfenv_regular_Eq :
+forall Γ x τ, wfenv Γ → binds x (Eq τ) Γ → lc_typ τ.
+Proof.
+intros. induction H; analyze_binds H0.
+eauto.
+replace t with τ in * by congruence; eauto.
+eauto.
+Qed.
+Hint Resolve wfenv_regular_T wfenv_regular_Eq.
+
+Lemma wftyp_regular_T2 : forall Γ x τ τ',
+  wftyp (x ~ T τ ++ Γ) τ' → lc_typ τ.
+Proof.
+intros Γ x τ τ' H. eauto.
+Qed.
+
+Lemma wftyp_regular_Eq2 : forall Γ x τ τ',
+  wftyp (x ~ Eq τ ++ Γ) τ' → lc_typ τ.
+Proof.
+intros Γ x τ τ' H. eauto.
+Qed.
+Hint Resolve wftyp_regular_T2 wftyp_regular_Eq2.
+
+Lemma wfenv_wftyp_subst :
+  (forall Γ, wfenv Γ → forall Γ₁ Γ₂ x τ, Γ = Γ₁ ++ x ~ (T τ) ++ Γ₂ → wfenv (Γ₁ ++ Γ₂)) ∧
+  (forall Γ τ, wftyp Γ τ → forall Γ₁ Γ₂ x τ', Γ = Γ₁ ++ x ~ (T τ') ++ Γ₂ → wftyp (Γ₁ ++ Γ₂) τ).
+Proof.
+apply wfenv_wftyp_mut_ind; intros.
+Case "wfenv_empty".
+assert (binds x (T τ) nil). rewrite H; auto. analyze_binds H0.
+Case "wfenv_T".
+destruct Γ₁; simpl_env in *.
+inversion H0; subst; eauto.
+destruct p; destruct t; inversion H0; subst; simpl_env in *;
+constructor; eauto.
+Case "wfenv_cons_U".
+destruct Γ₁; simpl_env in *.
+inversion H0; subst; eauto.
+destruct p; destruct t; inversion H0; subst; simpl_env in *;
+constructor; eauto.
+Case "wfenv_cons_E".
+destruct Γ₁; simpl_env in *.
+inversion H0; subst; eauto.
+destruct p; destruct t; inversion H0; subst; simpl_env in *;
+constructor; eauto.
+Case "wfenv_Eq".
+destruct Γ₁; simpl_env in *.
+inversion H0; subst; eauto.
+destruct p; destruct t; inversion H0; subst; simpl_env in *;
+constructor; eauto.
+Case "wftyp_var".
+subst G. constructor; eauto.
+  destruct o. analyze_binds H0.
+  destruct H0. analyze_binds H0.
+  destruct H0. analyze_binds H0; eauto.
+Case "wftyp_arrow".
+subst G. constructor; eauto.
+Case "wftyp_prod".
+subst G. constructor; eauto.
+Case "wftyp_forall".
+subst G. econstructor; intros.
+rewrite_env (([(a, U)] ++ Γ₁) ++ Γ₂). eapply H; simpl_env; eauto.
+Case "wftyp_exists".
+subst G. econstructor; intros.
+rewrite_env (([(a, U)] ++ Γ₁) ++ Γ₂). eapply H; simpl_env; eauto.
+Qed.
+
+Lemma wfenv_subst :
+forall Γ₁ Γ₂ x τ, wfenv (Γ₁ ++ x ~ (T τ) ++ Γ₂) → wfenv (Γ₁ ++ Γ₂).
+Proof.
+destruct wfenv_wftyp_subst as [H1 H2].
+intros Γ₁ Γ₂ x τ H. eapply H1; eauto.
+Qed.
+Hint Resolve wfenv_subst.
+
+Lemma wftyp_subst :
+forall Γ₁ Γ₂ τ x τ', wftyp (Γ₁ ++ x ~ (T τ') ++ Γ₂) τ → wftyp (Γ₁ ++ Γ₂) τ.
+Proof.
+destruct wfenv_wftyp_subst as [H1 H2].
+intros. eapply H2; eauto.
+Qed.
+Hint Resolve wftyp_subst.
+
+Lemma wfenv_wftyp_tsubst :
+  (forall Γ, wfenv Γ → forall Γ₁ Γ₂ a τ, Γ = Γ₁ ++ a ~ U ++ Γ₂ → wftyp Γ₂ τ → wfenv ((env_map (tsubst_typ τ a) Γ₁) ++ Γ₂)) ∧
+  (forall Γ τ, wftyp Γ τ → forall Γ₁ Γ₂ a τ', Γ = Γ₁ ++ a ~ U ++ Γ₂ → wftyp Γ₂ τ' → wftyp ((env_map (tsubst_typ τ' a) Γ₁) ++ Γ₂) (tsubst_typ τ' a τ)).
+Proof.
+apply wfenv_wftyp_mut_ind; intros.
+Case "wfenv_empty".
+assert (binds a (@U typ) nil). rewrite H; auto. analyze_binds H1.
+Case "wfenv_cons_T".
+destruct Γ₁; simpl_env in *.
+inversion H0; subst; eauto.
+destruct p; destruct t; inversion H0; subst; simpl_env in *;
+simpl; simpl_env; constructor.
+unfold env_map; auto. eapply H; auto.
+unfold env_map; auto. eapply H; auto.
+unfold env_map; auto. eapply H; auto.
+unfold env_map; auto. eapply H; auto.
+unfold env_map; auto. eapply H; auto.
+unfold env_map; auto. eapply H; auto.
+Case "wfenv_cons_U".
+destruct Γ₁; simpl_env in *.
+inversion H0; subst; eauto.
+destruct p; destruct t; inversion H0; subst; simpl_env in *.
+simpl; simpl_env; constructor. unfold env_map; auto. eapply H; auto.
+Case "wfenv_cons_E".
+destruct Γ₁; simpl_env in *.
+inversion H0; subst; eauto.
+destruct p; destruct t; inversion H0; subst; simpl_env in *.
+simpl; simpl_env; constructor. unfold env_map; auto. eapply H; auto.
+Case "wfenv_cons_Eq".
+destruct Γ₁; simpl_env in *.
+inversion H0; subst; eauto.
+destruct p; destruct t; inversion H0; subst; simpl_env in *;
+simpl; simpl_env; constructor.
+unfold env_map; auto. eapply H; auto.
+unfold env_map; auto. eapply H; auto.
+unfold env_map; auto. eapply H; auto.
+unfold env_map; auto. eapply H; auto.
+unfold env_map; auto. eapply H; auto.
+unfold env_map; auto. eapply H; auto.
+Case "wftyp_var".
+subst G. simpl.
+destruct (a == a0); subst.
+rewrite_env (nil ++ env_map (tsubst_typ τ' a0) Γ₁ ++ Γ₂); apply wftyp_weakening; auto.
+constructor; auto.
+destruct o.
+analyze_binds H0;
+replace (@U typ) with (tag_map (tsubst_typ τ' a0) U) by reflexivity;
+unfold env_map; auto.
+destruct H0.
+analyze_binds H0;
+replace (@E typ) with (tag_map (tsubst_typ τ' a0) E) by reflexivity;
+unfold env_map; auto.
+destruct H0.
+right; right. analyze_binds H0; eauto.
+exists (tsubst_typ τ' a0 x).
+replace (Eq (tsubst_typ τ' a0 x)) with (tag_map (tsubst_typ τ' a0) (Eq x)) by reflexivity;
+unfold env_map; auto.
+Case "wftyp_arrow".
+subst G. simpl; constructor; auto.
+Case "wftyp_prod".
+subst G. simpl; constructor; auto.
+Case "wftyp_forall".
+subst G. simpl; apply wftyp_forall with (L := L ∪ {{a}}); intros.
+rewrite_env (([(a0, U)] ++ env_map (tsubst_typ τ' a) Γ₁) ++ Γ₂).
+replace ([(a0, U)] ++ env_map (tsubst_typ τ' a) Γ₁) with (env_map (tsubst_typ τ' a) ([(a0, U)] ++ Γ₁)) by reflexivity.
+replace (typ_var_f a0) with (tsubst_typ τ' a (typ_var_f a0)).
+rewrite <- tsubst_typ_open_typ_wrt_typ.
+eapply H; simpl_env; eauto. eauto.
+autorewrite with lngen; auto.
+Case "wftyp_exists".
+subst G. simpl; apply wftyp_exists with (L := L ∪ {{a}}); intros.
+rewrite_env (([(a0, U)] ++ env_map (tsubst_typ τ' a) Γ₁) ++ Γ₂).
+replace ([(a0, U)] ++ env_map (tsubst_typ τ' a) Γ₁) with (env_map (tsubst_typ τ' a) ([(a0, U)] ++ Γ₁)) by reflexivity.
+replace (typ_var_f a0) with (tsubst_typ τ' a (typ_var_f a0)).
+rewrite <- tsubst_typ_open_typ_wrt_typ.
+eapply H; simpl_env; eauto. eauto.
+autorewrite with lngen; auto.
+Qed.
+
+Lemma wfenv_tsubst :
+  forall Γ₁ Γ₂ a τ, wfenv (Γ₁ ++ a ~ U ++ Γ₂) → wftyp Γ₂ τ →
+    wfenv (env_map (tsubst_typ τ a) Γ₁ ++ Γ₂).
+Proof.
+destruct wfenv_wftyp_tsubst as [H1 H2].
+intros Γ₁ Γ₂ x τ H. eapply H1; eauto.
+Qed.
+Hint Resolve wfenv_tsubst.
+
+Lemma wftyp_tsubst :
+forall Γ₁ Γ₂ τ a τ', wftyp (Γ₁ ++ a ~ U ++ Γ₂) τ →
+wftyp Γ₂ τ' → wftyp (env_map (tsubst_typ τ' a) Γ₁ ++ Γ₂) (tsubst_typ τ' a τ).
+Proof.
+destruct wfenv_wftyp_tsubst as [H1 H2].
+intros. eapply H2; eauto.
+Qed.
+Hint Resolve wftyp_tsubst.
+
+Lemma wftyp_fv : forall Γ τ, wftyp Γ τ → ftv_typ τ [<=] dom Γ.
+Proof.
+intros Γ τ H. induction H; simpl in *; try fsetdec.
+Case "var".
+assert (a ∈ dom G).
+  destruct H; eauto. destruct H; eauto. destruct H; eauto.
+fsetdec.
+Case "forall".
+pick fresh a.
+assert (ftv_typ (open_typ_wrt_typ t (typ_var_f a))[<=]add a (dom G)) by auto.
+assert (ftv_typ t [<=] ftv_typ (open_typ_wrt_typ t (typ_var_f a))); auto with lngen.
+fsetdec.
+Case "exists".
+pick fresh a.
+assert (ftv_typ (open_typ_wrt_typ t (typ_var_f a))[<=]add a (dom G)) by auto.
+assert (ftv_typ t [<=] ftv_typ (open_typ_wrt_typ t (typ_var_f a))); auto with lngen.
+fsetdec.
+Qed.
+Hint Resolve wftyp_fv.
+
+(** Lemmas about [zip] *)
+
+ICI
+
+(** Lemmas about [wfterm] *)
+Lemma wfterm_wfenv : forall Γ e τ,
+  wfterm Γ e τ → wfenv Γ.
+Proof.
+intros Γ e τ H.
+induction H; auto.
+pick fresh x; assert (wfenv ([(x, T t1)] ++ G)) by auto; inversion H1; subst; eauto.
+pick fresh a; assert (wfenv ([(a, None)] ++ G)) by auto; inversion H1; subst; eauto.
+Qed.
+Hint Resolve wfterm_wfenv.
+
+Lemma wfterm_wftyp : forall Γ e τ,
+  wfterm Γ e τ → wftyp Γ τ.
+Proof.
+intros Γ e τ H.
+induction H.
+Case "var". eapply wfenv_wftyp2; eauto.
+Case "app". inversion IHwfterm1; subst; auto.
+Case "abs". pick fresh x. assert ([(x, T t1)] ++ G ⊢ t2 ok) by auto.
+assert (wfenv ([(x, T t1)] ++ G)) by eauto.
+inversion H2; subst.
+constructor; auto. rewrite_env (nil ++ G). eauto.
+Case "inst". inversion IHwfterm; subst.
+inversion IHwfterm; subst.
+pick fresh a. rewrite tsubst_typ_intro with (a1 := a); auto.
+rewrite_env (env_map (tsubst_typ t a) nil ++ G).
+apply wftyp_tsubst; simpl_env; auto.
+Case "gen".
+apply wftyp_forall with (L := L); auto.
+Qed.
+Hint Resolve wfterm_wftyp.
+
+Lemma wfterm_regular2 : forall Γ e τ,
+  wfterm Γ e τ → lc_typ τ.
+Proof.
+intros Γ e τ H; induction H; eauto.
+Qed.
+Hint Resolve wfterm_regular2.
+
+Lemma wfterm_regular1 : forall Γ e τ,
+  wfterm Γ e τ → lc_term e.
+Proof.
+intros Γ e τ H; induction H; auto.
+pick fresh x.
+apply lc_term_abs_exists with (x1 := x).
+apply wfenv_regular with (Γ := [(x, T t1)] ++ G) (x := x); eauto.
+auto.
+eauto.
+Qed.
+Hint Resolve wfterm_regular1.
+
+Lemma wfterm_env_uniq : forall Γ e τ,
+  wfterm Γ e τ → uniq Γ.
+Proof.
+intros Γ e τ H. eauto.
+Qed.
+Hint Resolve wfterm_env_uniq.
+
+(** Lemmas about values *)
+Lemma value_is_normal_aux :
+  (forall v, pval v → ~ exists e, v ⇝ e) ∧
+  (forall v, val v → ~ exists e, v ⇝ e).
+Proof.
+apply pval_val_mut_ind; intros; intros [e0 Hred]; inversion Hred; subst; eauto.
+inversion H.
+inversion H1; subst. inversion p.
+inversion H0; subst. inversion p.
+inversion H0.
+pick fresh x. eapply H; eauto.
+inversion H0.
+pick fresh a. eapply H; eauto.
+Qed.
+
+Lemma value_is_normal : forall v, val v → ~ exists e, v ⇝ e.
+Proof.
+destruct value_is_normal_aux as [_ Th]. intuition auto.
+Qed.
+
+(** Renaming lemmas *)
+Lemma pval_val_renaming : forall x y,
+  (forall v, pval v → pval (subst_term (term_var_f y) x v)) ∧
+  (forall v, val v → val (subst_term (term_var_f y) x v)).
+Proof.
+intros x y.
+apply pval_val_mut_ind; intros; simpl; auto.
+Case "var". destruct (x0 == x); auto.
+Case "abs". pick fresh z and apply val_abs; auto.
+  rewrite subst_term_open_term_wrt_term_var; auto.
+Case "gen". pick fresh a and apply val_gen; auto.
+  rewrite subst_term_open_term_wrt_typ_var; auto.
+Qed.
+
+Lemma val_renaming : forall x y v,
+  val v → val (subst_term (term_var_f y) x v).
+Proof.
+intros x y v H. destruct (pval_val_renaming x y); auto.
+Qed.
+Hint Resolve val_renaming.
+
+Lemma pval_val_trenaming : forall a b,
+  (forall v, pval v → pval (tsubst_term (typ_var_f b) a v)) ∧
+  (forall v, val v → val (tsubst_term (typ_var_f b) a v)).
+Proof.
+intros a b.
+apply pval_val_mut_ind; intros; simpl; auto with lngen.
+Case "abs". pick fresh z and apply val_abs; auto with lngen.
+  rewrite tsubst_term_open_term_wrt_term_var; auto.
+Case "gen". pick fresh c and apply val_gen; auto.
+  rewrite tsubst_term_open_term_wrt_typ_var; auto.
+Qed.
+
+Lemma val_trenaming : forall a b v,
+  val v → val (tsubst_term (typ_var_f b) a v).
+Proof.
+intros a b v H. destruct (pval_val_trenaming a b); auto.
+Qed.
+Hint Resolve val_trenaming.
+
+(** Lemmas about red0, red1 *)
+Lemma red0_subst : forall x e'' e e', lc_term e'' → red0 e e' →
+  red0 (subst_term e'' x e) (subst_term e'' x e').
+Proof.
+intros x e'' e e' Hlc H.
+inversion H; subst; simpl.
+rewrite subst_term_open_term_wrt_term; auto. apply red0_beta; auto with lngen.
+assert (lc_term (subst_term e'' x (term_abs t e1))) by auto with lngen; auto.
+rewrite subst_term_open_term_wrt_typ; auto. apply red0_beta_t; auto with lngen.
+assert (lc_term (subst_term e'' x (term_gen e0))) by auto with lngen; auto.
+Qed.
+Hint Resolve red0_subst.
+
+Lemma red1_subst : forall x e'' e e', lc_term e'' → e ⇝ e' →
+  (subst_term e'' x e) ⇝ (subst_term e'' x e').
+Proof.
+intros x e'' e e' Hlc H.
+induction H; subst; simpl; auto with lngen.
+apply red1_abs with (L := L `union` {{x}}); auto; intros z Hz.
+replace (term_var_f z) with (subst_term e'' x (term_var_f z)) by auto with lngen.
+repeat rewrite <- subst_term_open_term_wrt_term; eauto.
+apply red1_gen with (L := L `union` {{x}}); intros a Ha.
+repeat rewrite <- subst_term_open_term_wrt_typ; eauto.
+Qed.
+Hint Resolve red1_subst.
+
+Lemma red1_open : forall L e'' e e',
+  lc_term e'' →
+  (forall x, x ∉ L → e ^ x ⇝ e' ^ x) →
+  e ^^ e'' ⇝ e' ^^ e''.
+Proof.
+intros L e'' e e' Hlc H.
+pick fresh x.
+rewrite subst_term_intro with (x1 := x) (e1 := e); auto.
+rewrite subst_term_intro with (x1 := x) (e1 := e'); auto.
+Qed.
+Hint Resolve red1_open.
+
+Lemma red0_tsubst : forall a τ e e', lc_typ τ → red0 e e' →
+  red0 (tsubst_term τ a e) (tsubst_term τ a e').
+Proof.
+intros a τ e e' Hlc H.
+inversion H; subst; simpl.
+rewrite tsubst_term_open_term_wrt_term; auto. apply red0_beta; auto with lngen.
+assert (lc_term (tsubst_term τ a (term_abs t e1))) by auto with lngen; auto.
+rewrite tsubst_term_open_term_wrt_typ; auto. apply red0_beta_t; auto with lngen.
+assert (lc_term (tsubst_term τ a (term_gen e0))) by auto with lngen; auto.
+Qed.
+Hint Resolve red0_tsubst.
+
+Lemma red1_tsubst : forall a τ e e', lc_typ τ → e ⇝ e' →
+  (tsubst_term τ a e) ⇝ (tsubst_term τ a e').
+Proof.
+intros a τ e e' Hlc H.
+induction H; subst; simpl; auto with lngen.
+apply red1_abs with (L := L `union` {{a}}); auto with lngen ; intros z Hz.
+replace (term_var_f z) with (tsubst_term τ a (term_var_f z)) by reflexivity.
+repeat rewrite <- tsubst_term_open_term_wrt_term; eauto.
+apply red1_gen with (L := L `union` {{a}}); intros b Hb.
+replace (typ_var_f b) with (tsubst_typ τ a (typ_var_f b)) by auto with lngen.
+repeat rewrite <- tsubst_term_open_term_wrt_typ; eauto.
+Qed.
+Hint Resolve red1_tsubst.
+
+Lemma red1_topen : forall L τ e e',
+  lc_typ τ →
+  (forall a, a ∉ L → open_term_wrt_typ e (typ_var_f a) ⇝ open_term_wrt_typ e' (typ_var_f a)) →
+  open_term_wrt_typ e τ ⇝ open_term_wrt_typ e' τ.
+Proof.
+intros L τ e e' Hlc H.
+pick fresh a.
+rewrite tsubst_term_intro with (a1 := a) (e1 := e); auto.
+rewrite tsubst_term_intro with (a1 := a) (e1 := e'); auto.
+Qed.
+Hint Resolve red1_topen.
+
+(*
+(* Lemmas about wfterm *)
+Lemma wfterm_fv : forall Γ e τ,
+  wfterm Γ e τ → fv_term e [<=] dom Γ.
+Proof.
+intros Γ e τ H. induction H; simpl fv_term in *.
+assert (x ∈ dom G) by eauto; fsetdec.
+fsetdec.
+pick fresh x. assert (fv_term (e ^ x) [<=] dom (x ~ t1 ++ G)) by auto.
+assert (fv_term e [<=] fv_term (e ^ x)) by auto with lngen.
+assert (fv_term e [<=] {{x}} ∪ dom G). simpl in *; fsetdec.
+fsetdec.
+Qed.
+*)
+
+Lemma wfterm_uniqueness : forall Γ e τ τ',
+  wfterm Γ e τ → wfterm Γ e τ' → τ = τ'.
+Proof.
+intros Γ e τ τ' H1 H2. generalize dependent τ'.
+induction H1; intros τ' H2; inversion H2; subst.
+Case "var".
+assert (T t = T τ'). eapply binds_unique; eauto. congruence.
+Case "app".
+assert (typ_arrow t2 t1 = typ_arrow t3 τ') by auto; congruence.
+Case "abs".
+pick fresh x; assert (t2 = t3) by eauto; congruence.
+Case "inst".
+assert (typ_forall t' = typ_forall t'0) by auto; congruence.
+Case "gen".
+pick fresh a. assert (open_typ_wrt_typ t (typ_var_f a) = open_typ_wrt_typ t0 (typ_var_f a)) by auto.
+f_equal; eapply open_typ_wrt_typ_inj; eauto.
+Qed.
+
+(*
+Lemma wfterm_strengthening : forall Γ₁ Γ₂ x τ τ' e,
+  x ∉ fv_term e →
+  wfterm (Γ₁ ++ x ~ τ' ++ Γ₂) e τ →
+  wfterm (Γ₁ ++ Γ₂) e τ.
+Proof.
+intros Γ₁ Γ₂ x τ τ' e Hx He.
+dependent induction He; simpl in Hx.
+Case "var".
+constructor. solve_uniq. analyze_binds_uniq H0.
+Case "app".
+econstructor; eauto.
+Case "abs".
+apply wfterm_abs with (L := L `union` {{x}}); intros.
+rewrite_env (([(x0, t1)] ++ Γ₁) ++ Γ₂).
+eapply H0 with (x1 := x); auto.
+assert (fv_term (e ^ x0) [<=] fv_term (term_var_f x0) ∪ fv_term e) as H2
+ by auto with lngen.
+simpl in H2; fsetdec.
+simpl_env; eauto.
+Qed.
+*)
+
+(** Major lemmas about [wfterm] *)
+Lemma wfterm_weakening : forall Γ₁ Γ₂ Γ₃ e τ,
+  wfterm (Γ₁ ++ Γ₃) e τ →
+  wfenv (Γ₂ ++ Γ₃) →
+  disjoint Γ₁ Γ₂ →
+  wfterm (Γ₁ ++ Γ₂ ++ Γ₃) e τ.
+Proof.
+intros Γ₁ Γ₂ Γ₃ e τ H. dependent induction H; intros; eauto.
+Case "var".
+constructor. auto using wfenv_weakening. analyze_binds H0.
+Case "abs". pick fresh x and apply wfterm_abs.
+rewrite_env (([(x, T t1)] ++ Γ₁) ++ Γ₂ ++ Γ₃).
+apply H0; simpl_env; auto.
+Case "inst". constructor. auto using wftyp_weakening. eauto.
+Case "gen". pick fresh a and apply wfterm_gen.
+rewrite_env (([(a, None)] ++ Γ₁) ++ Γ₂ ++ Γ₃).
+apply H0; simpl_env; auto.
+Qed.
+
+Lemma wfterm_subst : forall Γ₁ Γ₂ x τ₁ τ₂ e₁ e₂,
+  wfterm (Γ₁ ++ x ~ T τ₂ ++ Γ₂) e₁ τ₁ →
+  wfterm Γ₂ e₂ τ₂ →
+  wfterm (Γ₁ ++ Γ₂) (subst_term e₂ x e₁) τ₁.
+Proof with eauto.
+intros Γ₁ Γ₂ x τ₁ τ₂ e₁ e₂ H. dependent induction H; intro; simpl...
+Case "var".
+  destruct (x == x0); subst.
+  SCase "x = x0".
+    analyze_binds_uniq H0; apply wfterm_weakening with (Γ₁ := nil); auto.
+    replace t with τ₂ by congruence; auto.
+    eapply wfenv_subst; eauto.
+  SCase "x <> x0".
+    analyze_binds_uniq H0...
+Case "abs".
+  pick fresh z and apply wfterm_abs.
+  rewrite_env ((z ~ T t1 ++ Γ₁) ++ Γ₂).
+  rewrite subst_term_open_term_wrt_term_var...
+  apply H0 with (τ₂0 := τ₂)...
+Case "gen".
+  pick fresh a and apply wfterm_gen.
+  rewrite_env ((a ~ None ++ Γ₁) ++ Γ₂).
+  rewrite subst_term_open_term_wrt_typ_var...
+  apply H0 with (τ₂0 := τ₂)...
+Qed.
+
+Lemma wfterm_tsubst : forall Γ₁ Γ₂ a τ₁ e₁ τ₂,
+  wfterm (Γ₁ ++ a ~ None ++ Γ₂) e₁ τ₁ →
+  wftyp Γ₂ τ₂ →
+  wfterm (env_map (tsubst_typ τ₂ a) Γ₁ ++ Γ₂) (tsubst_term τ₂ a e₁) (tsubst_typ τ₂ a τ₁).
+Proof with eauto.
+intros Γ₁ Γ₂ a τ₁ e₁ τ₂ H. dependent induction H; intro; simpl...
+Case "var".
+constructor. auto using wfenv_tsubst.
+replace (T (tsubst_typ τ₂ a t)) with (tag_map (tsubst_typ τ₂ a) (T t)) by reflexivity.
+unfold env_map. analyze_binds H0.
+simpl.
+assert (a ∉ ftv_typ t).
+  assert (ftv_typ t [<=] dom Γ₂) by eauto.
+  assert (uniq (Γ₁ ++ [(a, None)] ++ Γ₂)) by auto.
+  destruct_uniq. fsetdec.
+autorewrite with lngen; auto.
+Case "app".
+econstructor.
+eapply IHwfterm1; auto.
+eapply IHwfterm2; auto.
+Case "abs".
+  pick fresh z and apply wfterm_abs.
+  rewrite_env (env_map (tsubst_typ τ₂ a) ([(z, T t1)] ++ Γ₁) ++ Γ₂).
+  rewrite tsubst_term_open_term_wrt_term_var...
+Case "inst".
+  rewrite tsubst_typ_open_typ_wrt_typ...
+  constructor; auto. apply IHwfterm; auto.
+Case "gen".
+  pick fresh b and apply wfterm_gen.
+  rewrite_env (env_map (tsubst_typ τ₂ a) ([(b, None)] ++ Γ₁) ++ Γ₂).
+  rewrite tsubst_term_open_term_wrt_typ_var...
+  rewrite tsubst_typ_open_typ_wrt_typ_var...
+Qed.
+
+(** Soundness *)
+Theorem subject_reduction : forall Γ e e' τ,
+  wfterm Γ e τ → e ⇝ e' → wfterm Γ e' τ.
+Proof with eauto.
+  intros Γ e e' τ H. generalize dependent e'.
+  dependent induction H.
+  Case "var".
+    intros e' J; inversion J; subst; inversion H1.
+  Case "app".
+    intros e' J; inversion J; subst...
+    inversion H; subst; inversion H1; subst.
+    pick fresh z.
+    rewrite (subst_term_intro z)...
+    eapply wfterm_subst with (Γ₁ := nil); simpl_env...
+  Case "abs".
+    intros e' J; inversion J; subst.
+    inversion H1.
+    pick fresh z and apply wfterm_abs...
+  Case "inst".
+    intros e' J; inversion J; subst; auto.
+    inversion H1; subst.
+    inversion H0; subst.
+    pick fresh a.
+    rewrite (tsubst_term_intro a)...
+    rewrite (tsubst_typ_intro a)...
+    rewrite_env (env_map (tsubst_typ t a) nil ++ G).
+    eapply wfterm_tsubst; simpl_env...
+  Case "gen".
+    intros e' J; inversion J; subst.
+    inversion H1.
+    pick fresh a and apply wfterm_gen...
+Qed.
+
+Theorem progress : forall Γ e τ,
+  wfterm Γ e τ →
+  (exists e', e ⇝ e') ∨ val e.
+Proof with eauto.
+  intros Γ e τ H.
+  dependent induction H; simpl...
+  Case "typing_app".
+    destruct IHwfterm1 as [[e1' ?] | ?]...
+    destruct IHwfterm2 as [[e2' ?] | ?]...
+    destruct e1; simpl in H1; inversion H1; subst; try solve [inversion H]; eauto 7.
+  Case "abs".
+    pick fresh z. edestruct (H0 z) as [[e1 ?] | ?]...
+    left.
+      exists (term_abs t1 (close_term_wrt_term z e1)).
+      apply red1_abs with (L := L `union` {{z}}); intros...
+      rewrite <- subst_term_spec.
+      rewrite (subst_term_intro z)...
+    right.
+      apply val_abs with (L := L `union` {{z}}); intros...
+      rewrite (subst_term_intro z)...
+  Case "inst".
+    destruct IHwfterm as [[e' ? ] | ? ]...
+    destruct e; simpl in H1; inversion H1; subst; eauto.
+    inversion H0.
+    eauto 7.
+  Case "gen".
+    pick fresh a. edestruct (H0 a) as [[e1 ?] | ?]...
+    left.
+      exists (term_gen (close_term_wrt_typ a e1)).
+      apply red1_gen with (L := L `union` {{a}}); intros.
+      rewrite <- tsubst_term_spec.
+      rewrite (tsubst_term_intro a)...
+    right.
+      apply val_gen with (L := L `union` {{a}}); intros.
+      rewrite (tsubst_term_intro a)...
+Qed.
